@prefix owl: <http://www.w3.org/2002/07/owl#> .
@prefix xsd: <http://www.w3.org/2001/XMLSchema#> .
@prefix : <http://www.purl.org/mentalhealth/references#> .
@prefix schema: <http://schema.org/> .
@prefix dcterms: <http://purl.org/dc/terms/> .
@prefix mhdb: <http://www.purl.org/mentalhealth#> .
@prefix rdfs: <http://www.w3.org/2000/01/rdf-schema#> .
@prefix rdf: <http://www.w3.org/1999/02/22-rdf-syntax-ns#> .
@prefix dbpedia-owl: <http://dbpedia.org/ontology> .
@prefix bibo: <http://purl.org/ontology/bibo> .
@prefix fabio: <http://purl.org/spar/fabio> .
@prefix disco: <http://rdf-vocabulary.ddialliance.org/discovery.html> .
@base <http://www.purl.org/mentalhealth/references> .
<http://www.purl.org/mentalhealth/references> rdf:type owl:Ontology ;
    owl:versionIRI <http://www.purl.org/mentalhealth/references/0.3.0> ;
    owl:versionInfo "0.3.0"^^rdfs:Literal ;
    rdfs:label "mental health database — References"^^rdfs:Literal ;
    rdfs:comment """

================================================================================
		Mental Health Database (MHDB)
================================================================================
This mental health database interrelates information about mental health-related
(1) signs, symptoms, and disorders from the DSM-5, 
(2) questions from questionnaires, 
(3) cognitive tasks, 
(4) behaviors, cognitive domains, measures, and sensors,  
(5) projects and technologies, and 
(6) relevant references.
The database is licensed under the terms of the Creative Commons BY license.
Current information can be found on the website, https://matter.childmind.org.

================================================================================
		References
================================================================================

"""@en .

mhdb:ReferenceType rdfs:label """ReferenceType"""@en ;
	rdf:type rdf:Class .

mhdb:Informant rdfs:label """Informant"""@en ;
	rdf:type rdf:Class .

mhdb:AgeGroup rdfs:label """AgeGroup"""@en ;
	rdf:type rdf:Class .

mhdb:StudyOrClinic rdfs:label """StudyOrClinic"""@en ;
	rdf:type rdf:Class .

mhdb:Domain rdfs:label """Domain"""@en ;
	rdf:type rdf:Class .

mhdb:hasReferenceType rdfs:label """hasReferenceType"""@en ;
	rdf:type rdf:Property ;
	rdfs:domain dcterms:source ;
	rdfs:range mhdb:ReferenceType .

mhdb:hasInformant rdfs:label """hasInformant"""@en ;
	rdf:type rdf:Property ;
	rdfs:range mhdb:Informant .

mhdb:hasAgeGroup rdfs:label """hasAgeGroup"""@en ;
	rdf:type rdf:Property ;
	rdfs:range mhdb:AgeGroup .

mhdb:hasStudyOrClinic rdfs:label """hasStudyOrClinic"""@en ;
	rdf:type rdf:Property ;
	rdfs:range mhdb:StudyOrClinic .

mhdb:hasAbbreviation rdfs:label """hasAbbreviation"""@en ;
	rdf:type rdf:Property ;
	rdfs:range dbpedia-owl:abbreviation .

mhdb:hasNumberOfQuestions rdfs:label """hasNumberOfQuestions"""@en ;
	rdf:type rdf:Property .

mhdb:takesMinutesToComplete rdfs:label """takesMinutesToComplete"""@en ;
	rdf:type rdf:Property .

mhdb:usedByStudyOrClinic rdfs:label """usedByStudyOrClinic"""@en ;
	rdf:type rdf:Property ;
	rdfs:range mhdb:StudyOrClinic .

mhdb:isAboutDomain rdfs:label """isAboutDomain"""@en ;
	rdf:type rdf:Property ;
	rdfs:range mhdb:Domain .

mhdb:isForInformant rdfs:label """isForInformant"""@en ;
	rdf:type rdf:Property ;
	rdfs:range mhdb:Informant .

mhdb:isForAgeGroup rdfs:label """isForAgeGroup"""@en ;
	rdf:type rdf:Property ;
	rdfs:range mhdb:AgeGroup .

<https://depts.washington.edu/dbpeds/Screening%20Tools/DSM-5(ASD.Guidelines)Feb2013.pdf> rdfs:label """DSM-5 Autism Spectrum Disorder: Guidelines and Criteria exemplars (Laura Carpenter)"""@en ;
	rdf:type dcterms:source ;
	schema:WebSite <https://depts.washington.edu/dbpeds/Screening%20Tools/DSM-5(ASD.Guidelines)Feb2013.pdf> ;
	mhdb:hasReferenceType schema:WebSite .

<https://www.cdc.gov/childrensmentalhealth/ocd.html> rdfs:label """CDC Obsessive-Compulsive Disorder"""@en ;
	rdf:type dcterms:source ;
	schema:WebSite <https://www.cdc.gov/childrensmentalhealth/ocd.html> ;
	mhdb:hasReferenceType schema:WebSite .

<https://www.cdc.gov/ncbddd/tourette/ocd.html> rdfs:label """CDC Diagnosing Obsessive -Compulsive Disorder"""@en ;
	rdf:type dcterms:source ;
	schema:WebSite <https://www.cdc.gov/ncbddd/tourette/ocd.html> ;
	mhdb:hasReferenceType schema:WebSite .

<https://www.urmc.rochester.edu/encyclopedia/content.aspx?contenttypeid=90&contentid=P02582> rdfs:label """University of Rochester / Encyclopedia / Separation Anxiety Disorder"""@en ;
	rdf:type dcterms:source ;
	schema:WebSite <https://www.urmc.rochester.edu/encyclopedia/content.aspx?contenttypeid=90&contentid=P02582> ;
	mhdb:hasReferenceType schema:WebSite ;
	mhdb:isAboutDomain mhdb:anxiety .

<https://www.nimh.nih.gov/health/publications/social-anxiety-disorder-more-than-just-shyness/index.shtml> rdfs:label """National Institute of Mental health: Social Anxiety Disorder"""@en ;
	rdf:type dcterms:source ;
	schema:WebSite <https://www.nimh.nih.gov/health/publications/social-anxiety-disorder-more-than-just-shyness/index.shtml> ;
	mhdb:hasReferenceType schema:WebSite ;
	mhdb:isAboutDomain mhdb:anxiety .

<https://www.nimh.nih.gov/health/topics/anxiety-disorders/index.shtml> rdfs:label """National Institute of Mental health: Anxiety Disorder"""@en ;
	rdf:type dcterms:source ;
	schema:WebSite <https://www.nimh.nih.gov/health/topics/anxiety-disorders/index.shtml> ;
	mhdb:hasReferenceType schema:WebSite ;
	mhdb:isAboutDomain mhdb:anxiety .

<http://dsm.psychiatryonline.org/doi/book/10.1176/appi.books.9780890425596> rdfs:label """Diagnostic and Statistical Manual 5"""@en ;
	rdf:type dcterms:source ;
	mhdb:hasAbbreviation mhdb:DSM-5 ;
	schema:WebSite <http://dsm.psychiatryonline.org/doi/book/10.1176/appi.books.9780890425596> ;
	mhdb:hasReferenceType mhdb:nosology_manual .

mhdb:CMI_Life_Events_Questionnaire rdfs:label """CMI Life Events Questionnaire"""@en ;
	rdf:type dcterms:source ;
	mhdb:hasReferenceType disco:Questionnaire ;
	mhdb:usedByStudyOrClinic mhdb:Child_Mind_Institute ;
	mhdb:isAboutDomain mhdb:background_information .

mhdb:CMI_Symptom_Checklist-Parent rdfs:label """CMI Symptom Checklist - Parent"""@en ;
	rdf:type dcterms:source ;
	rdfs:comment """The Child Mind Institute Symptom Checker is used to assess general psychiatric symptoms of individuals."""@en ;
	mhdb:takesMinutesToComplete "5"^^xsd:nonNegativeInteger ;
	mhdb:hasReferenceType disco:Questionnaire ;
	mhdb:usedByStudyOrClinic mhdb:Healthy_Brain_Network ;
	mhdb:usedByStudyOrClinic mhdb:Child_Mind_Institute ;
	mhdb:isAboutDomain mhdb:psychotic_behavior ;
	mhdb:isAboutDomain mhdb:behavior ;
	mhdb:isAboutDomain mhdb:atypical_behavior ;
	mhdb:isForInformant mhdb:parent-report ;
	mhdb:isForAgeGroup mhdb:children .

mhdb:CMI_Symptom_Self_Checklist rdfs:label """CMI Symptom Self Checklist"""@en ;
	rdf:type dcterms:source ;
	mhdb:hasReferenceType disco:Questionnaire ;
	mhdb:usedByStudyOrClinic mhdb:Child_Mind_Institute ;
	mhdb:isAboutDomain mhdb:psychotic_behavior ;
	mhdb:isAboutDomain mhdb:atypical_behavior ;
	mhdb:isForInformant mhdb:self-report .

mhdb:Sutter-Eyberg_School_Behavior_Inventory_Revised rdfs:label """Sutter-Eyberg School Behavior Inventory Revised"""@en ;
	rdf:type dcterms:source ;
	mhdb:hasAbbreviation mhdb:SESBI-R ;
	mhdb:hasReferenceType disco:Questionnaire ;
	mhdb:usedByStudyOrClinic mhdb:Child_Mind_Institute ;
	mhdb:usedByStudyOrClinic mhdb:Nathan_Kline_Institute .

mhdb:SNAP-4_Parent_questionnaire rdfs:label """SNAP-4 Parent questionnaire"""@en ;
	rdf:type dcterms:source ;
	mhdb:hasAbbreviation mhdb:SNAP ;
	mhdb:hasReferenceType disco:Questionnaire ;
	mhdb:usedByStudyOrClinic mhdb:Child_Mind_Institute ;
	mhdb:usedByStudyOrClinic mhdb:Nathan_Kline_Institute ;
	mhdb:isForInformant mhdb:parent-report .

mhdb:Eyberg_Child_Behavior_Inventory rdfs:label """Eyberg Child Behavior Inventory"""@en ;
	rdf:type dcterms:source ;
	mhdb:hasAbbreviation mhdb:ECBI ;
	mhdb:hasReferenceType disco:Questionnaire ;
	mhdb:usedByStudyOrClinic mhdb:Child_Mind_Institute ;
	mhdb:usedByStudyOrClinic mhdb:Nathan_Kline_Institute .

mhdb:The_Conners_ADHD_Rating_Scale_3-Parent_Short_Form rdfs:label """The Conners ADHD Rating Scale 3 - Parent Short Form"""@en ;
	rdf:type dcterms:source ;
	mhdb:hasReferenceType disco:Questionnaire ;
	mhdb:usedByStudyOrClinic mhdb:Nathan_Kline_Institute ;
	mhdb:isAboutDomain mhdb:oppositionality ;
	mhdb:isAboutDomain mhdb:social_interaction ;
	mhdb:isAboutDomain mhdb:executive_functions ;
	mhdb:isAboutDomain mhdb:hyperactivity ;
	mhdb:isAboutDomain mhdb:attention ;
	mhdb:isAboutDomain mhdb:aggression ;
	mhdb:isForInformant mhdb:parent-report .

mhdb:Child_Behaviour_Checklist_for_ages_15-5 rdfs:label """Child Behaviour Checklist for ages 1.5-5"""@en ;
	rdf:type dcterms:source ;
	mhdb:hasAbbreviation mhdb:CBCL_Age_15-5 ;
	mhdb:hasReferenceType disco:Questionnaire ;
	mhdb:usedByStudyOrClinic mhdb:Child_Mind_Institute .

mhdb:Child_Behaviour_Checklist_Teachers_Report_Form_for_ages_6-18 rdfs:label """Child Behaviour Checklist Teacher's Report Form for ages 6-18"""@en ;
	rdf:type dcterms:source ;
	mhdb:hasAbbreviation mhdb:CBCL-TRF_Age_6-18 ;
	rdfs:comment """The CBCL is a device by which parents or other individuals who know the child well rate a child's problem behaviors and competencies. The CBCL can also be used to measure a child's change in behavior over time or following a treatment. It consists of 118 items related to behavior problems, which are scored on a 3-point scale ranging from not true to often true of the child. There are also 20 social competency items used to obtain parents’ reports of the amount and quality of their child’s participation in sports, hobbies, games, activities, organizations, jobs and chores, friendships, how well the child gets along with others and plays and works by him/herself, and school functioning."""@en ;
	mhdb:takesMinutesToComplete "20"^^xsd:nonNegativeInteger ;
	mhdb:hasReferenceType disco:Questionnaire ;
	mhdb:usedByStudyOrClinic mhdb:Healthy_Brain_Network ;
	mhdb:isAboutDomain mhdb:impulsivity ;
	mhdb:isAboutDomain mhdb:anxiety ;
	mhdb:isAboutDomain mhdb:social_interaction ;
	mhdb:isAboutDomain mhdb:substance_use ;
	mhdb:isAboutDomain mhdb:psychotic_behavior ;
	mhdb:isAboutDomain mhdb:risk_taking ;
	mhdb:isAboutDomain mhdb:behavior ;
	mhdb:isAboutDomain mhdb:atypical_behavior ;
	mhdb:isAboutDomain mhdb:personality_traits ;
	mhdb:isAboutDomain mhdb:somatic_complaints ;
	mhdb:isAboutDomain mhdb:addiction ;
	mhdb:isForInformant mhdb:teacher-report ;
	dcterms:isReferencedBy mhdb:Achenbach_T_M_1991_Integrative_Guide_to_the_1991_CBCL4-18_YSR_and_TRF_Profiles_Burlington_VT_University_of_Vermont_Department_of_Psychology .

mhdb:Child_Behavior_Checklist_Age_6-18 rdfs:label """Child Behavior Checklist: Age 6-18"""@en ;
	rdf:type dcterms:source ;
	mhdb:hasAbbreviation mhdb:CBCL_Age_6-18 ;
	rdfs:comment """The CBCL is a device by which parents or other individuals who know the child well rate a child's problem behaviors and competencies. The CBCL can also be used to measure a child's change in behavior over time or following a treatment. It consists of 118 items related to behavior problems, which are scored on a 3-point scale ranging from not true to often true of the child. There are also 20 social competency items used to obtain parents’ reports of the amount and quality of their child’s participation in sports, hobbies, games, activities, organizations, jobs and chores, friendships, how well the child gets along with others and plays and works by him/herself, and school functioning."""@en ;
	mhdb:takesMinutesToComplete "20"^^xsd:nonNegativeInteger ;
	mhdb:hasReferenceType disco:Questionnaire ;
	mhdb:usedByStudyOrClinic mhdb:Healthy_Brain_Network ;
	mhdb:usedByStudyOrClinic mhdb:Nathan_Kline_Institute ;
	mhdb:isAboutDomain mhdb:anxiety ;
	mhdb:isAboutDomain mhdb:social_interaction ;
	mhdb:isAboutDomain mhdb:substance_use ;
	mhdb:isAboutDomain mhdb:psychotic_behavior ;
	mhdb:isAboutDomain mhdb:risk_taking ;
	mhdb:isAboutDomain mhdb:behavior ;
	mhdb:isAboutDomain mhdb:atypical_behavior ;
	mhdb:isAboutDomain mhdb:personality_traits ;
	mhdb:isAboutDomain mhdb:somatic_complaints ;
	mhdb:isAboutDomain mhdb:addiction ;
	mhdb:isForInformant mhdb:parent-report ;
	dcterms:isReferencedBy mhdb:Achenbach_T_M_1991_Integrative_Guide_to_the_1991_CBCL4-18_YSR_and_TRF_Profiles_Burlington_VT_University_of_Vermont_Department_of_Psychology .

mhdb:Adult_Self_Report_Age_18-59 rdfs:label """Adult Self Report: Age 18-59"""@en ;
	rdf:type dcterms:source ;
	mhdb:hasAbbreviation mhdb:ASR ;
	rdfs:comment """The ASR is a self-administered instrument that examines diverse aspects of adaptive functioning and problems."""@en ;
	mhdb:takesMinutesToComplete "10"^^xsd:nonNegativeInteger ;
	mhdb:hasReferenceType disco:Questionnaire ;
	mhdb:usedByStudyOrClinic mhdb:Healthy_Brain_Network ;
	mhdb:usedByStudyOrClinic mhdb:Nathan_Kline_Institute ;
	mhdb:isAboutDomain mhdb:social_interaction ;
	mhdb:isAboutDomain mhdb:antisocial_personality ;
	mhdb:isAboutDomain mhdb:anxiety ;
	mhdb:isAboutDomain mhdb:psychotic_behavior ;
	mhdb:isAboutDomain mhdb:risk_taking ;
	mhdb:isAboutDomain mhdb:avoidant_personality ;
	mhdb:isAboutDomain mhdb:atypical_behavior ;
	mhdb:isAboutDomain mhdb:mood ;
	mhdb:isAboutDomain mhdb:somatic_complaints ;
	mhdb:isAboutDomain mhdb:oppositionality ;
	mhdb:isAboutDomain mhdb:impulsivity ;
	mhdb:isAboutDomain mhdb:depression ;
	mhdb:isAboutDomain mhdb:executive_functions ;
	mhdb:isAboutDomain mhdb:behavior ;
	mhdb:isAboutDomain mhdb:hyperactivity ;
	mhdb:isAboutDomain mhdb:aggression ;
	mhdb:isAboutDomain mhdb:addiction ;
	mhdb:isAboutDomain mhdb:cognitive_functioning ;
	mhdb:isAboutDomain mhdb:substance_use ;
	mhdb:isAboutDomain mhdb:personality_traits ;
	mhdb:isAboutDomain mhdb:attention ;
	mhdb:isForInformant mhdb:self-report ;
	mhdb:isForAgeGroup mhdb:adults ;
	dcterms:isReferencedBy mhdb:Achenbach_T_Rescorla_L_2003_Manual_for_the_ASEBA_Adult_Forms__Profiles_Burlington_VT_University_of_Vermont_Research_Center_for_Children_Youth_and_Families .

mhdb:Youth_Self_Report rdfs:label """Youth Self Report"""@en ;
	rdf:type dcterms:source ;
	mhdb:hasAbbreviation mhdb:YSR ;
	rdfs:comment """The YSR is a self-administered instrument in which youth (ages 11-18) rate themselves for how true each item is now or has been during the past 6 months, using the same 3-point scale as the CBCL 6-18 and the TRF. YSR also has 14 socially desirable items that most youths endorse about themselves."""@en ;
	mhdb:takesMinutesToComplete "10"^^xsd:nonNegativeInteger ;
	mhdb:hasReferenceType disco:Questionnaire ;
	mhdb:usedByStudyOrClinic mhdb:Healthy_Brain_Network ;
	mhdb:usedByStudyOrClinic mhdb:Nathan_Kline_Institute ;
	mhdb:isAboutDomain mhdb:oppositionality ;
	mhdb:isAboutDomain mhdb:impulsivity ;
	mhdb:isAboutDomain mhdb:depression ;
	mhdb:isAboutDomain mhdb:social_interaction ;
	mhdb:isAboutDomain mhdb:substance_use ;
	mhdb:isAboutDomain mhdb:cognitive_functioning ;
	mhdb:isAboutDomain mhdb:personality_traits ;
	mhdb:isAboutDomain mhdb:psychotic_behavior ;
	mhdb:isAboutDomain mhdb:executive_functions ;
	mhdb:isAboutDomain mhdb:behavior ;
	mhdb:isAboutDomain mhdb:risk_taking ;
	mhdb:isAboutDomain mhdb:atypical_behavior ;
	mhdb:isAboutDomain mhdb:mood ;
	mhdb:isAboutDomain mhdb:hyperactivity ;
	mhdb:isAboutDomain mhdb:somatic_complaints ;
	mhdb:isAboutDomain mhdb:attention ;
	mhdb:isAboutDomain mhdb:aggression ;
	mhdb:isAboutDomain mhdb:addiction ;
	mhdb:isForInformant mhdb:self-report ;
	dcterms:isReferencedBy mhdb:Achenbach_T_M_1991_Manual_for_the_Youth_Self-Report_and_1991_profile_Burlington_VT_University_of_Vermont_Department_of_Psychiatry .

mhdb:Child_Behaviour_Checklist_Caregiver_and_teacher-15-5 rdfs:label """Child Behaviour Checklist Caregiver and teacher - 1.5-5"""@en ;
	rdf:type dcterms:source ;
	mhdb:hasReferenceType disco:Questionnaire ;
	mhdb:usedByStudyOrClinic mhdb:Nathan_Kline_Institute ;
	mhdb:isForInformant mhdb:teacher-report ;
	mhdb:isForInformant mhdb:caregiver-report ;
	mhdb:isForAgeGroup mhdb:children .

mhdb:Childrens_Yale-Brown_Obsessive_Compulsive_Scale rdfs:label """Children's Yale-Brown Obsessive Compulsive Scale"""@en ;
	rdf:type dcterms:source ;
	mhdb:hasAbbreviation mhdb:CY-BOCS ;
	rdfs:comment """The Y-BOCS is a semi-structured clinician rated instrument to assess the severity of obsessive-compulsive disorder (OCD) symptoms that is administered as part of the KSADS interview, if indicated."""@en ;
	mhdb:takesMinutesToComplete "10"^^xsd:nonNegativeInteger ;
	mhdb:hasReferenceType disco:Questionnaire ;
	mhdb:usedByStudyOrClinic mhdb:Nathan_Kline_Institute ;
	mhdb:isAboutDomain mhdb:psychotic_behavior ;
	mhdb:isAboutDomain mhdb:behavior ;
	mhdb:isAboutDomain mhdb:atypical_behavior ;
	mhdb:isForInformant mhdb:self-report ;
	dcterms:isReferencedBy mhdb:Storch_E_A_Larson_M_J_Goodman_W_K_Rasmussen_S_A_Price_L_H__Murphy_T_K_2010 .

mhdb:Screen_for_Child_Anxiety_Related_Disorders-Child_Version rdfs:label """Screen for Child Anxiety Related Disorders - Child Version"""@en ;
	rdf:type dcterms:source ;
	mhdb:hasAbbreviation mhdb:SCARED-C ;
	rdfs:comment """The SCARED is a child and parent self-report instrument used to screen for childhood anxiety disorders including general anxiety disorder, separation anxiety disorder, panic disorder, and social phobia. In addition, it assesses symptoms related to school phobias."""@en ;
	mhdb:takesMinutesToComplete "10"^^xsd:nonNegativeInteger ;
	mhdb:hasReferenceType disco:Questionnaire ;
	mhdb:usedByStudyOrClinic mhdb:Child_Mind_Institute ;
	mhdb:isAboutDomain mhdb:anxiety ;
	mhdb:isForInformant mhdb:self-report ;
	mhdb:isForAgeGroup mhdb:children ;
	dcterms:isReferencedBy mhdb:Birmaher_B_Brent_D_A_Chiappetta_L_Bridge_J_Monga_S__Baugher_M_1999 .

mhdb:Screen_for_Child_Anxiety_Related_Disorders-Parent_report rdfs:label """Screen for Child Anxiety Related Disorders - Parent report"""@en ;
	rdf:type dcterms:source ;
	mhdb:hasAbbreviation mhdb:SCARED-P ;
	mhdb:hasReferenceType disco:Questionnaire ;
	mhdb:usedByStudyOrClinic mhdb:Healthy_Brain_Network ;
	mhdb:isAboutDomain mhdb:anxiety ;
	mhdb:isForInformant mhdb:parent-report ;
	mhdb:isForAgeGroup mhdb:children .

mhdb:Becks_Depression_Inventory-2 rdfs:label """Beck's Depression Inventory - 2"""@en ;
	rdf:type dcterms:source ;
	mhdb:hasAbbreviation mhdb:BDI ;
	rdfs:comment """The BDI-II is a 21-question multiple-choice self-report inventory, one of the most widely used instruments for measuring the severity of depression."""@en ;
	mhdb:takesMinutesToComplete "10"^^xsd:nonNegativeInteger ;
	mhdb:hasReferenceType disco:Questionnaire ;
	mhdb:usedByStudyOrClinic mhdb:Healthy_Brain_Network ;
	mhdb:usedByStudyOrClinic mhdb:Nathan_Kline_Institute ;
	mhdb:isAboutDomain mhdb:depression ;
	mhdb:isAboutDomain mhdb:mood ;
	mhdb:isForInformant mhdb:self-report .

mhdb:Columbia_Suicide_Severity_Rating_Scale rdfs:label """Columbia Suicide Severity Rating Scale"""@en ;
	rdf:type dcterms:source ;
	mhdb:hasAbbreviation mhdb:C-SSRS ;
	rdfs:comment """The Columbia Suicide Severity Rating Scale is a 6-item scale used to assess the severity of suicidal thoughts and behaviors. It is administered by a clinician as an interview, only to those participants who screen positive for suicidal thoughts or behaviors."""@en ;
	mhdb:takesMinutesToComplete "5"^^xsd:nonNegativeInteger ;
	mhdb:hasReferenceType disco:Questionnaire ;
	mhdb:usedByStudyOrClinic mhdb:Healthy_Brain_Network ;
	mhdb:isAboutDomain mhdb:suicidal_ideation ;
	mhdb:isAboutDomain mhdb:depression ;
	mhdb:isAboutDomain mhdb:mood ;
	mhdb:isForInformant mhdb:self-report ;
	dcterms:isReferencedBy mhdb:Posner_K_Brown_GK_Stanley_B_Brent_DA_Yershova_KV_Oquendo_MA_Currier_GW_Melvin_G_Greenhill_L_Shen_S__Mann_JJ_The_Columbia-Suicide_Severity_Rating_Scale_Initial_Validity_and_Internal_Consistency_Findings_From_Three_Multisite_Studies_With_Adolescents_and_Adults_American_Journal_of_Psychiatry_2011_1681266-1277 .

mhdb:Adult_Suicidal_Ideation_Questionnaire rdfs:label """Adult Suicidal Ideation Questionnaire"""@en ;
	rdf:type dcterms:source ;
	mhdb:hasAbbreviation mhdb:ASIQ ;
	mhdb:hasReferenceType disco:Questionnaire ;
	mhdb:usedByStudyOrClinic mhdb:Child_Mind_Institute ;
	mhdb:isAboutDomain mhdb:suicidal_ideation ;
	mhdb:isForInformant mhdb:self-report ;
	mhdb:isForAgeGroup mhdb:adults .

mhdb:Childrens_Depression_Inventory rdfs:label """Children's Depression Inventory"""@en ;
	rdf:type dcterms:source ;
	mhdb:hasAbbreviation mhdb:CDI ;
	rdfs:comment """The Children’s Depression Inventory is a 27 item, self-report measure of symptoms of depression among children and adolescents. The CDI assesses a range of depressive symptoms, including disturbed mood, impaired hedonic capacity, vegetative functions, self-evaluation, and interpersonal behaviors."""@en ;
	mhdb:takesMinutesToComplete "15"^^xsd:nonNegativeInteger ;
	mhdb:hasReferenceType disco:Questionnaire ;
	mhdb:usedByStudyOrClinic mhdb:Healthy_Brain_Network ;
	mhdb:usedByStudyOrClinic mhdb:Nathan_Kline_Institute ;
	mhdb:isAboutDomain mhdb:depression ;
	mhdb:isAboutDomain mhdb:mood ;
	mhdb:isForInformant mhdb:self-report ;
	mhdb:isForAgeGroup mhdb:children ;
	dcterms:isReferencedBy mhdb:Kovacs_M_1985_The_Childrens_Depression_Inventory_CDI_Psychopharmacology_Bulletin_214_995-998 .

mhdb:Suicidal_Ideation_Questionnaire rdfs:label """Suicidal Ideation Questionnaire"""@en ;
	rdf:type dcterms:source ;
	mhdb:hasAbbreviation mhdb:SIQ ;
	mhdb:hasReferenceType disco:Questionnaire ;
	mhdb:usedByStudyOrClinic mhdb:Child_Mind_Institute ;
	mhdb:isAboutDomain mhdb:suicidal_ideation .

mhdb:Difficulties_in_Emotion_Regulation_Scale rdfs:label """Difficulties in Emotion Regulation Scale"""@en ;
	rdf:type dcterms:source ;
	mhdb:hasAbbreviation mhdb:DERS ;
	mhdb:hasReferenceType disco:Questionnaire ;
	mhdb:usedByStudyOrClinic mhdb:Nathan_Kline_Institute ;
	mhdb:isAboutDomain mhdb:emotion .

mhdb:State_Trait_Anxiety_Inventory rdfs:label """State Trait Anxiety Inventory"""@en ;
	rdf:type dcterms:source ;
	mhdb:hasAbbreviation mhdb:STAI ;
	rdfs:comment """The STAI is used to measure anxiety in adults. A version is available for children. Helps distinguish feelings of anxiety from depression. The STAI Form clearly differentiates between the temporary condition of “state anxiety” verses the more general and long standing quality of ”trait anxiety.” The STAI has forty questions with a range of four possible responses to each (Likert scale)."""@en ;
	mhdb:takesMinutesToComplete "10"^^xsd:nonNegativeInteger ;
	mhdb:hasReferenceType disco:Questionnaire ;
	mhdb:usedByStudyOrClinic mhdb:Healthy_Brain_Network ;
	mhdb:usedByStudyOrClinic mhdb:Nathan_Kline_Institute ;
	mhdb:isAboutDomain mhdb:anxiety ;
	mhdb:isForInformant mhdb:self-report ;
	dcterms:isReferencedBy mhdb:Spielberger_C_D_Gorsuch_RL_and_Lushene_RE_1970_Manual_for_the_State-Trait_Anxiety_Inventory_Palo_Alto_CA_Consulting_Psychologists_Press .

mhdb:Mood_and_Feelings_Questionnaire_Parent_Report rdfs:label """Mood and Feelings Questionnaire Parent Report"""@en ;
	rdf:type dcterms:source ;
	mhdb:hasAbbreviation mhdb:MFQ-P ;
	rdfs:comment """The MFQ consists of a series of descriptive phrases regarding how the subject has been feeling or acting recently. Codings reflect whether the phrase was descriptive of the subject most of the time, sometimes, or not at all in the past two weeks."""@en ;
	mhdb:takesMinutesToComplete "10"^^xsd:nonNegativeInteger ;
	mhdb:hasReferenceType disco:Questionnaire ;
	mhdb:usedByStudyOrClinic mhdb:Healthy_Brain_Network ;
	mhdb:isAboutDomain mhdb:depression ;
	mhdb:isAboutDomain mhdb:mood ;
	mhdb:isForInformant mhdb:parent-report ;
	dcterms:isReferencedBy mhdb:Angold_A_Costello_E_J_Messer_S_C_Pickles_A_Winder_F__Silver_D_1995_The_development_of_a_short_questionnaire_for_use_in_epidemiological_studies_of_depression_in_children_and_adolescents_International_Journal_of_Methods_in_Psychiatric_Research_5_237-249 .

mhdb:Mood_and_Feelings_Questionnaire_Self_Report rdfs:label """Mood and Feelings Questionnaire Self Report"""@en ;
	rdf:type dcterms:source ;
	mhdb:hasAbbreviation mhdb:MFQ-SR ;
	rdfs:comment """The MFQ consists of a series of descriptive phrases regarding how the subject has been feeling or acting recently. Codings reflect whether the phrase was descriptive of the subject most of the time, sometimes, or not at all in the past two weeks."""@en ;
	mhdb:takesMinutesToComplete "10"^^xsd:nonNegativeInteger ;
	mhdb:hasReferenceType disco:Questionnaire ;
	mhdb:usedByStudyOrClinic mhdb:Healthy_Brain_Network ;
	mhdb:isAboutDomain mhdb:depression ;
	mhdb:isAboutDomain mhdb:mood ;
	mhdb:isForInformant mhdb:self-report ;
	dcterms:isReferencedBy mhdb:Angold_A_Costello_E_J_Messer_S_C_Pickles_A_Winder_F__Silver_D_1995_The_development_of_a_short_questionnaire_for_use_in_epidemiological_studies_of_depression_in_children_and_adolescents_International_Journal_of_Methods_in_Psychiatric_Research_5_237-249 .

mhdb:Affective_Reactivity_Index___Self_Report rdfs:label """Affective Reactivity Index –  Self Report"""@en ;
	rdf:type dcterms:source ;
	mhdb:hasAbbreviation mhdb:ARI-S ;
	rdfs:comment """The ARI-S is a concise scale for the dimensional assessment of irritability."""@en ;
	mhdb:takesMinutesToComplete "5-7"^^xsd:string ;
	mhdb:hasReferenceType disco:Questionnaire ;
	mhdb:usedByStudyOrClinic mhdb:Healthy_Brain_Network ;
	mhdb:isAboutDomain mhdb:oppositionality ;
	mhdb:isAboutDomain mhdb:aggression ;
	mhdb:isAboutDomain mhdb:personality_traits ;
	mhdb:isForInformant mhdb:self-report .

mhdb:Strengths_and_Weaknesses_Assessment_of_Normal_Behavior rdfs:label """Strengths and Weaknesses Assessment of Normal Behavior"""@en ;
	rdf:type dcterms:source ;
	mhdb:hasAbbreviation mhdb:SWAN ;
	rdfs:comment """The SWAN ADHD Rating Scale is an instrument that uses observer ratings to help assess attention deficit/hyperactivity disorder (ADHD) and evaluate problem behavior in children and adolescents."""@en ;
	mhdb:hasReferenceType disco:Questionnaire ;
	mhdb:usedByStudyOrClinic mhdb:Healthy_Brain_Network ;
	mhdb:usedByStudyOrClinic mhdb:Nathan_Kline_Institute ;
	mhdb:isAboutDomain mhdb:hyperactivity ;
	mhdb:isAboutDomain mhdb:executive_functions ;
	mhdb:isAboutDomain mhdb:cognitive_functioning ;
	mhdb:isAboutDomain mhdb:attention ;
	mhdb:isForInformant mhdb:parent-report ;
	dcterms:isReferencedBy mhdb:Swanson_J_Schuck_S_Mann_M_Carlson_C_Hartman_K_Sergeant_J____McCleary_R_2001_The_SWAN_rating_scale .

mhdb:Inventory_of_Callous_and_Unemotional_Traits___Parent_Report rdfs:label """Inventory of Callous and Unemotional Traits  – Parent Report"""@en ;
	rdf:type dcterms:source ;
	mhdb:hasAbbreviation mhdb:ICU-P ;
	rdfs:comment """The Inventory of Callous-Unemotional Traits (ICUT) is a copyright protected 24-item questionnaire designed to provide a comprehensive assessment of callous and unemotional traits.  These traits have proven to be important for designating a distinct subgroup group of antisocial and aggressive youth. The ICUT has three subscales: Callousness, Uncaring, and Unemotional."""@en ;
	mhdb:takesMinutesToComplete "10-15"^^xsd:string ;
	mhdb:hasReferenceType disco:Questionnaire ;
	mhdb:usedByStudyOrClinic mhdb:Healthy_Brain_Network ;
	mhdb:usedByStudyOrClinic mhdb:Nathan_Kline_Institute ;
	mhdb:isAboutDomain mhdb:personality_traits ;
	mhdb:isForInformant mhdb:parent-report ;
	dcterms:isReferencedBy mhdb:Essau_CA_Sasagawa_S__Frick_PJ_2006_Callous-unemotional_traits_in_a_community_sample_of_adolescents_Assessment_132_454-469 .

mhdb:Autism_Spectrum_Screening_Questionnaire rdfs:label """Autism Spectrum Screening Questionnaire"""@en ;
	rdf:type dcterms:source ;
	mhdb:hasAbbreviation mhdb:ASSQ ;
	rdfs:comment """The ASSQ is a 27-item checklist for completion by lay informants when assessing symptoms characteristic of Asperger's Syndrome or high-functioning autism spectrum disorders."""@en ;
	mhdb:takesMinutesToComplete "15"^^xsd:nonNegativeInteger ;
	mhdb:hasReferenceType disco:Questionnaire ;
	mhdb:usedByStudyOrClinic mhdb:Healthy_Brain_Network ;
	mhdb:usedByStudyOrClinic mhdb:Nathan_Kline_Institute ;
	mhdb:isAboutDomain mhdb:restrictive_behaviors ;
	mhdb:isAboutDomain mhdb:repetitive_behaviors ;
	mhdb:isAboutDomain mhdb:motor_clumsiness ;
	mhdb:isForInformant mhdb:parent-report .

mhdb:Social_Communication_Questionnaire rdfs:label """Social Communication Questionnaire"""@en ;
	rdf:type dcterms:source ;
	mhdb:hasAbbreviation mhdb:SCQ ;
	rdfs:comment """The SCQ consists of forty yes-or-no questions, which a parent can complete in around ten minutes. It is brief and easy to understand, yet provides valuable information on a child’s body movements, use of language or gestures, and style of interacting. There are two versions of the SCQ. Usually, the SCQ is used as a screening instrument to help identify which children may have an autism spectrum disorder. It is not meant to provide a detailed diagnosis, but to indicate whether a child needs a more careful and in-depth evaluation."""@en ;
	mhdb:takesMinutesToComplete "10"^^xsd:nonNegativeInteger ;
	mhdb:hasReferenceType disco:Questionnaire ;
	mhdb:usedByStudyOrClinic mhdb:Healthy_Brain_Network ;
	mhdb:isAboutDomain mhdb:social_interaction ;
	mhdb:isForInformant mhdb:parent-report ;
	dcterms:isReferencedBy mhdb:Chandler_S_Charman_T_Baird_G_et_al_2007_Validation_of_the_Social_Communication_Questionnaire_in_a_population_cohort_of_children_with_autism_spectrum_disorders_Journal_of_the_American_Academy_of_Child_and_Adolescent_Psychiatry_46_1324_-1332 .

mhdb:Social_Responsiveness_Scale-2 rdfs:label """Social Responsiveness Scale-2"""@en ;
	rdf:type dcterms:source ;
	mhdb:hasAbbreviation mhdb:SRS-2 ;
	rdfs:comment """The second edition of the widely administered Social Responsiveness Scale (SRS-2; Constantino & Gruber, 2012) maintains continuity with the original instrument as an efficient quantitative measure of the various dimensions of interpersonal behavior, communication, and repetitive/stereotypic behavior characteristic of autism spectrum disorders (ASD)."""@en ;
	mhdb:takesMinutesToComplete "15"^^xsd:nonNegativeInteger ;
	mhdb:hasReferenceType disco:Questionnaire ;
	mhdb:usedByStudyOrClinic mhdb:Healthy_Brain_Network ;
	mhdb:isAboutDomain mhdb:social_interaction ;
	mhdb:isForInformant mhdb:parent-report ;
	dcterms:isReferencedBy mhdb:Constantino_JN_Davis_SA_Todd_RD_Schindler_MK_Gross_MM_Brophy_SL_et_al_2003_Validation_of_a_brief_quantitative_measure_of_autistic_traits_comparison_of_the_Social_Responsiveness_Scale_with_the_Autism_Diagnostic_Interview-Revised_Journal_of_Autism_Developmental_Disorders_33_427-433 .

mhdb:Columbia_Impairment_Scale-Self_Report_Version rdfs:label """Columbia Impairment Scale - Self Report Version"""@en ;
	rdf:type dcterms:source ;
	mhdb:hasAbbreviation mhdb:CIS-SR ;
	rdfs:comment """The CIS is a 13 item parent report scale that assesses global functioning in domains of interpersonal relations, psychopathology, school performance, use of leisure time; monitors progress after 6 months of treatment."""@en ;
	mhdb:hasReferenceType disco:Questionnaire ;
	mhdb:usedByStudyOrClinic mhdb:Healthy_Brain_Network ;
	mhdb:isAboutDomain mhdb:general_impairment ;
	mhdb:isForInformant mhdb:self-report ;
	dcterms:isReferencedBy mhdb:Bird_H_R_Shaffer_D_Fisher_P__Gould_M_S_1993_The_Columbia_Impairment_Scale_CIS_Pilot_findings_on_a_measure_of_global_impairment_for_children_and_adolescents_International_Journal_of_Methods_in_Psychiatric_Research .

mhdb:WHO_Disability_Assessment_Schedule_Parent_Report rdfs:label """WHO Disability Assessment Schedule Parent Report"""@en ;
	rdf:type dcterms:source ;
	mhdb:hasAbbreviation mhdb:WHODAS-P ;
	rdfs:comment """The WHODAS is a generic assessment instrument for health and disability. It assesses function across domains of cognition, mobility, self-care, getting along, life activities, and participation."""@en ;
	mhdb:takesMinutesToComplete "5"^^xsd:nonNegativeInteger ;
	mhdb:hasReferenceType disco:Questionnaire ;
	mhdb:usedByStudyOrClinic mhdb:Healthy_Brain_Network ;
	mhdb:isAboutDomain mhdb:general_impairment ;
	mhdb:isForInformant mhdb:parent-report ;
	dcterms:isReferencedBy mhdb:Gold_Liza_H_DSM-5_and_the_assessment_of_functioning_the_World_Health_Organization_Disability_Assessment_Schedule_20_WHODAS_20_Journal_of_the_American_Academy_of_Psychiatry_and_the_Law_Online_422_2014_173-181 .

mhdb:Manual_for_the_ASEBA_School-Age_forms__profiles rdfs:label """Manual for the ASEBA School-Age forms & profiles"""@en ;
	rdf:type dcterms:source ;
	mhdb:hasReferenceType mhdb:questionnaire_manual .

mhdb:Adverse_Childhood_Experience_Scale rdfs:label """Adverse Childhood Experience Scale"""@en ;
	rdf:type dcterms:source ;
	mhdb:hasAbbreviation mhdb:ACES ;
	rdfs:comment """Adverse childhood experiences (ACEs) include verbal, physical, or sexual abuse, as well as family dysfunction (e.g., an incarcerated, mentally ill, or substance-abusing family member; domestic violence; or absence of a parent because of divorce or separation). ACEs have been linked to a range of adverse health outcomes in adulthood, including substance abuse, depression, cardiovascular disease, diabetes, cancer, and premature mortality."""@en ;
	mhdb:takesMinutesToComplete "10"^^xsd:nonNegativeInteger ;
	mhdb:hasReferenceType disco:Questionnaire ;
	mhdb:usedByStudyOrClinic mhdb:Healthy_Brain_Network ;
	mhdb:isAboutDomain mhdb:trauma ;
	mhdb:isAboutDomain mhdb:mood ;
	mhdb:isForInformant mhdb:self-report ;
	dcterms:isReferencedBy mhdb:Felitti_VJ_Anda_RF_Nordenberg_D_et_al_Relationship_of_childhood_abuse_and_household_dysfunction_to_many_of_the_leading_causes_of_death_in_adults_The_adverse_childhood_experiences_ACE_study_Am_J_Prev_Med_199814245--58_PMID_9635069 .

mhdb:Alabama_Parenting_Questionnaire__Parent_Report rdfs:label """Alabama Parenting Questionnaire – Parent Report"""@en ;
	rdf:type dcterms:source ;
	mhdb:hasAbbreviation mhdb:APQ-P ;
	rdfs:comment """The APQ measures is a 42 item questionnaire measuring five domains of parenting that are relevant to the etiology and treatment of child externalizing problems: positive involvement, supervision/monitoring, use of positive discipline, consistency in the use of such discipline, and use of corporal punishment."""@en ;
	mhdb:takesMinutesToComplete "15"^^xsd:nonNegativeInteger ;
	mhdb:hasReferenceType disco:Questionnaire ;
	mhdb:usedByStudyOrClinic mhdb:Healthy_Brain_Network ;
	mhdb:isAboutDomain mhdb:corporal_punishment ;
	mhdb:isAboutDomain mhdb:supervisionmonitoring ;
	mhdb:isAboutDomain mhdb:distress_tolerance ;
	mhdb:isAboutDomain mhdb:use_of_consistency_of_positive_discipline ;
	mhdb:isAboutDomain mhdb:positive_involvement ;
	mhdb:isForInformant mhdb:parent-report .

mhdb:Alabama_Parenting_Questionnaire_Self-Report rdfs:label """Alabama Parenting Questionnaire Self-Report"""@en ;
	rdf:type dcterms:source ;
	mhdb:hasAbbreviation mhdb:APQ ;
	rdfs:comment """The APQ measures is a 42 item questionnaire measuring five domains of parenting that are relevant to the etiology and treatment of child externalizing problems: positive involvement, supervision/monitoring, use of positive discipline, consistency in the use of such discipline, and use of corporal punishment."""@en ;
	mhdb:takesMinutesToComplete "15"^^xsd:nonNegativeInteger ;
	mhdb:hasReferenceType disco:Questionnaire ;
	mhdb:usedByStudyOrClinic mhdb:Healthy_Brain_Network ;
	mhdb:isAboutDomain mhdb:corporal_punishment ;
	mhdb:isAboutDomain mhdb:supervisionmonitoring ;
	mhdb:isAboutDomain mhdb:distress_tolerance ;
	mhdb:isAboutDomain mhdb:use_of_consistency_of_positive_discipline ;
	mhdb:isAboutDomain mhdb:positive_involvement ;
	mhdb:isForInformant mhdb:self-report .

mhdb:Affective_Reactivity_Index-Parent_Report rdfs:label """Affective Reactivity Index - Parent Report"""@en ;
	rdf:type dcterms:source ;
	mhdb:hasAbbreviation mhdb:ARI-P ;
	rdfs:comment """The ARI-P is a concise scale for the dimensional assessment of irritability."""@en ;
	mhdb:takesMinutesToComplete "5-7"^^xsd:string ;
	mhdb:hasReferenceType disco:Questionnaire ;
	mhdb:usedByStudyOrClinic mhdb:Healthy_Brain_Network ;
	mhdb:isAboutDomain mhdb:oppositionality ;
	mhdb:isAboutDomain mhdb:aggression ;
	mhdb:isAboutDomain mhdb:personality_traits ;
	mhdb:isForInformant mhdb:parent-report .

mhdb:Alcohol_Use_Disorders_Identification_Test rdfs:label """Alcohol Use Disorders Identification Test"""@en ;
	rdf:type dcterms:source ;
	mhdb:hasAbbreviation mhdb:AUDIT ;
	rdfs:comment """The AUDIT is a simple, 10-item form developed by the World Health Organization to screen for problem or hazardous alcohol use in a clinical setting."""@en ;
	mhdb:takesMinutesToComplete "5"^^xsd:nonNegativeInteger ;
	mhdb:hasReferenceType disco:Questionnaire ;
	mhdb:usedByStudyOrClinic mhdb:Healthy_Brain_Network ;
	mhdb:isAboutDomain mhdb:substance_use ;
	mhdb:isAboutDomain mhdb:addiction ;
	mhdb:isForInformant mhdb:self-report .

mhdb:Barratt_Simplified_Measure_of_Social_Status rdfs:label """Barratt Simplified Measure of Social Status"""@en ;
	rdf:type dcterms:source ;
	mhdb:hasAbbreviation mhdb:BSMMS ;
	mhdb:hasReferenceType disco:Questionnaire ;
	mhdb:usedByStudyOrClinic mhdb:Healthy_Brain_Network ;
	mhdb:usedByStudyOrClinic mhdb:Nathan_Kline_Institute .

mhdb:Conners_ADHD_Rating_Scales-Self_Report_Short_Form rdfs:label """Conners ADHD Rating Scales - Self Report Short Form"""@en ;
	rdf:type dcterms:source ;
	rdfs:comment """The Conners ADHD Rating Scale is an instrument that uses self-report ratings to help assess attention deficit/hyperactivity disorder (ADHD) and evaluate problem behavior in children and adolescents."""@en ;
	mhdb:takesMinutesToComplete "10"^^xsd:nonNegativeInteger ;
	mhdb:hasReferenceType disco:Questionnaire ;
	mhdb:usedByStudyOrClinic mhdb:Healthy_Brain_Network ;
	mhdb:usedByStudyOrClinic mhdb:Nathan_Kline_Institute ;
	mhdb:isAboutDomain mhdb:oppositionality ;
	mhdb:isAboutDomain mhdb:social_interaction ;
	mhdb:isAboutDomain mhdb:cognitive_functioning ;
	mhdb:isAboutDomain mhdb:executive_functions ;
	mhdb:isAboutDomain mhdb:hyperactivity ;
	mhdb:isAboutDomain mhdb:attention ;
	mhdb:isAboutDomain mhdb:aggression ;
	mhdb:isForInformant mhdb:self-report ;
	dcterms:isReferencedBy mhdb:Conners_CK_2001_Conners_Rating_Scales-Revised_North_Tonawanda_NY_Multi-Health_Systems_Inc .

mhdb:Conners_ADHD_Adult_Rating_Scale-Self_Report_Short_Form rdfs:label """Conners ADHD Adult Rating Scale - Self Report Short Form"""@en ;
	rdf:type dcterms:source ;
	mhdb:hasAbbreviation mhdb:CAARS ;
	rdfs:comment """The Conners Adult ADHD Rating Scale is an instrument that uses self-report ratings to measure the presence and severity of ADHD symptoms."""@en ;
	mhdb:takesMinutesToComplete "10"^^xsd:nonNegativeInteger ;
	mhdb:hasReferenceType disco:Questionnaire ;
	mhdb:usedByStudyOrClinic mhdb:Healthy_Brain_Network ;
	mhdb:usedByStudyOrClinic mhdb:Nathan_Kline_Institute ;
	mhdb:isAboutDomain mhdb:oppositionality ;
	mhdb:isAboutDomain mhdb:social_interaction ;
	mhdb:isAboutDomain mhdb:cognitive_functioning ;
	mhdb:isAboutDomain mhdb:executive_functions ;
	mhdb:isAboutDomain mhdb:hyperactivity ;
	mhdb:isAboutDomain mhdb:attention ;
	mhdb:isAboutDomain mhdb:aggression ;
	mhdb:isForInformant mhdb:self-report ;
	mhdb:isForAgeGroup mhdb:adults ;
	dcterms:isReferencedBy mhdb:Conners_CK_Erhardt_D__Sparrow_E_1999_Conners_Adult_ADHD_Rating_Scales_Toronto_ON_Multi-Health_Systems_Inc .

mhdb:Childrens_Coping_Strategies_Checklist rdfs:label """Children's Coping Strategies Checklist"""@en ;
	rdf:type dcterms:source ;
	mhdb:hasAbbreviation mhdb:CCSC ;
	rdfs:comment """The Child Mind Institute Symptom Checker is used to assess general psychiatric symptoms of individuals."""@en ;
	mhdb:takesMinutesToComplete "5"^^xsd:nonNegativeInteger ;
	mhdb:hasReferenceType disco:Questionnaire ;
	mhdb:usedByStudyOrClinic mhdb:Healthy_Brain_Network ;
	mhdb:isAboutDomain mhdb:psychotic_behavior ;
	mhdb:isAboutDomain mhdb:behavior ;
	mhdb:isAboutDomain mhdb:atypical_behavior ;
	mhdb:isForInformant mhdb:parent-report ;
	mhdb:isForAgeGroup mhdb:children .

mhdb:Childrens_Depression_Inventory-Parent_Report rdfs:label """Children’s Depression Inventory - Parent Report"""@en ;
	rdf:type dcterms:source ;
	mhdb:hasAbbreviation mhdb:CDI-P ;
	rdfs:comment """The Children’s Depression Inventory is a 27 item, parent-report measure of symptoms of depression among children and adolescents. The CDI assesses a range of depressive symptoms, including disturbed mood, impaired hedonic capacity, vegetative functions, self-evaluation, and interpersonal behaviors."""@en ;
	mhdb:takesMinutesToComplete "15"^^xsd:nonNegativeInteger ;
	mhdb:hasReferenceType disco:Questionnaire ;
	mhdb:usedByStudyOrClinic mhdb:Healthy_Brain_Network ;
	mhdb:usedByStudyOrClinic mhdb:Nathan_Kline_Institute ;
	mhdb:isAboutDomain mhdb:depression ;
	mhdb:isAboutDomain mhdb:mood ;
	mhdb:isForInformant mhdb:parent-report ;
	mhdb:isForAgeGroup mhdb:children ;
	dcterms:isReferencedBy mhdb:Kovacs_M_1985_The_Childrens_Depression_Inventory_CDI_Psychopharmacology_Bulletin_214_995-998 .

mhdb:Childrens_Perception_of_Interparental_Conflict_Scale rdfs:label """Children's Perception of Interparental Conflict Scale"""@en ;
	rdf:type dcterms:source ;
	mhdb:hasAbbreviation mhdb:CPIC ;
	rdfs:comment """Guided by Grych and Fincham's theoretical framework for investigating the relation between interparental conflict and child adjustment, The Children's Perception of Interparental Conflict Scale (CPIC) was developed to assess children's views of several aspects of marital conflict."""@en ;
	mhdb:takesMinutesToComplete "10"^^xsd:nonNegativeInteger ;
	mhdb:hasReferenceType disco:Questionnaire ;
	mhdb:usedByStudyOrClinic mhdb:Healthy_Brain_Network ;
	mhdb:isAboutDomain mhdb:trauma ;
	mhdb:isAboutDomain mhdb:distress_tolerance ;
	mhdb:isForInformant mhdb:self-report ;
	dcterms:isReferencedBy mhdb:Grych_JH_Seid_M___Fincham_FD_1992_Assessing_marital_conflict_from_the_childs_perspective_The_Childrens_Perception_of_Interparental_Conflict_Scale_Child_Development_63_558-572_PMID_1600822 .

mhdb:Distress_Tolerance_Scale rdfs:label """Distress Tolerance Scale"""@en ;
	rdf:type dcterms:source ;
	mhdb:hasAbbreviation mhdb:DTS ;
	rdfs:comment """The DTS, a 15-item self-report questionnaire, measures emotional distress tolerance."""@en ;
	mhdb:takesMinutesToComplete "5"^^xsd:nonNegativeInteger ;
	mhdb:hasReferenceType disco:Questionnaire ;
	mhdb:usedByStudyOrClinic mhdb:Healthy_Brain_Network ;
	mhdb:isAboutDomain mhdb:distress_tolerance ;
	mhdb:isForInformant mhdb:parent-report ;
	dcterms:isReferencedBy mhdb:Simons__Gaher_2005_The_distress_tolerance_scale_development_and_validation_of_a_self-report_measure_Motivation_and_Emotion_292_83-102 .

mhdb:Edinburgh_Handedness_Questionnaire rdfs:label """Edinburgh Handedness Questionnaire"""@en ;
	rdf:type dcterms:source ;
	mhdb:hasAbbreviation mhdb:EHQ ;
	mhdb:hasReferenceType disco:Questionnaire ;
	mhdb:isForInformant mhdb:self-report .

mhdb:The_European_School_Survey_Project_on_Alcohol_and_Other_Drugs rdfs:label """The European School Survey Project on Alcohol and Other Drugs"""@en ;
	rdf:type dcterms:source ;
	mhdb:hasAbbreviation mhdb:ESPAD ;
	rdfs:comment """The ESPAD is an adaptive questionnaire. It consists of a 16-question drug and alcohol screening form and additional follow up questions only for substances that a participant endorses."""@en ;
	mhdb:takesMinutesToComplete "15"^^xsd:nonNegativeInteger ;
	mhdb:hasReferenceType disco:Questionnaire ;
	mhdb:usedByStudyOrClinic mhdb:Healthy_Brain_Network ;
	mhdb:isAboutDomain mhdb:substance_use ;
	mhdb:isAboutDomain mhdb:addiction ;
	mhdb:isForInformant mhdb:self-report ;
	dcterms:isReferencedBy mhdb:Hibell_B_Guttormsson_U_Ahlstrom_S_et_al_2012_The_2011_ESPAD_Report_substance_use_among_students_in_36_European_countries_The_Swedish_Council_for_Information_on_Alcohol_and_Other_Drugs_CAN_Stockholm_Sweden .

mhdb:Financial_Support_Questionnaire rdfs:label """Financial Support Questionnaire"""@en ;
	rdf:type dcterms:source ;
	mhdb:hasAbbreviation mhdb:FSQ ;
	mhdb:hasReferenceType disco:Questionnaire ;
	mhdb:usedByStudyOrClinic mhdb:Healthy_Brain_Network .

mhdb:Fagerstrom_Test_for_Nicotine_Dependence rdfs:label """Fagerstrom Test for Nicotine Dependence"""@en ;
	rdf:type dcterms:source ;
	mhdb:hasAbbreviation mhdb:FTND ;
	rdfs:comment """The FTND is a self-administered questionnaire that consists of 6 questions, and examines nicotine consumption and intake habits in those that smoke cigarettes. It is used as a screening instrument that assesses nicotine dependence in adults who are currently smokers or have been in the past two years. Level of nicotine dependence is scored on a scale from 0-10, with 0-2: very low dependence and 8-10: very high dependence."""@en ;
	mhdb:takesMinutesToComplete "5"^^xsd:nonNegativeInteger ;
	mhdb:hasReferenceType disco:Questionnaire ;
	mhdb:usedByStudyOrClinic mhdb:Healthy_Brain_Network ;
	mhdb:usedByStudyOrClinic mhdb:Nathan_Kline_Institute ;
	mhdb:isAboutDomain mhdb:substance_use ;
	mhdb:isAboutDomain mhdb:addiction ;
	mhdb:isForInformant mhdb:self-report ;
	dcterms:isReferencedBy mhdb:Heatherton_TF_Kozlowski_LT_Frecker_RC_Fagerstrom_KO_1991_The_Fagerstrom_Test_for_Nicotine_Dependence_A_revision_of_the_Fagerstrom_Tolerance_Questionnaire_British_Journal_of_Addictions_86_1119-27 .

mhdb:Modified_Fagerstrom_Tolerance_Questionnaire-Adolescents rdfs:label """Modified Fagerstrom Tolerance Questionnaire - Adolescents"""@en ;
	rdf:type dcterms:source ;
	mhdb:hasAbbreviation mhdb:FTQA ;
	rdfs:comment """The FTQA is a self-administered questionnaire consists of 7 questions, and is a modified version of the FTND that aims to assess nicotine tolerance in adolescents."""@en ;
	mhdb:takesMinutesToComplete "5"^^xsd:nonNegativeInteger ;
	mhdb:hasReferenceType disco:Questionnaire ;
	mhdb:usedByStudyOrClinic mhdb:Healthy_Brain_Network ;
	mhdb:usedByStudyOrClinic mhdb:Nathan_Kline_Institute ;
	mhdb:isAboutDomain mhdb:substance_use ;
	mhdb:isAboutDomain mhdb:addiction ;
	mhdb:isForInformant mhdb:self-report ;
	dcterms:isReferencedBy mhdb:Prokhorov_AV_Pallonen_UE_Fava_JL_Ding_L_Niaura_R_1996_Measuring_nicotine_dependence_among_high-risk_adolescent_smokers_Addict_Behav_21_1_117-127 .

mhdb:Internet_Addiction_Test rdfs:label """Internet Addiction Test"""@en ;
	rdf:type dcterms:source ;
	mhdb:hasAbbreviation mhdb:IAT ;
	rdfs:comment """The IAT is a 20-item scale that measures characteristics and behaviors associated with compulsive use of the Internet that include compulsivity, escapism, and dependency. Questions also assess problems related to addictive use in personal, occupational, and social functioning."""@en ;
	mhdb:takesMinutesToComplete "5-10"^^xsd:string ;
	mhdb:hasReferenceType disco:Questionnaire ;
	mhdb:usedByStudyOrClinic mhdb:Healthy_Brain_Network ;
	mhdb:isAboutDomain mhdb:substance_use ;
	mhdb:isAboutDomain mhdb:addiction ;
	mhdb:isForInformant mhdb:self-report ;
	dcterms:isReferencedBy mhdb:Young_K_S_1998_Internet_addiction_The_emergence_of_a_new_clinical_disorder_CyberPsychology_and_Behavior_13_237-244 .

mhdb:National_Institute_on_Drug_Abuse rdfs:label """National Institute on Drug Abuse"""@en ;
	rdf:type dcterms:source ;
	mhdb:hasAbbreviation mhdb:NIDA ;
	rdfs:comment """The NIDA Quick Screen and Assist is used to screen for substance use and severity over the lifetime and within the past year."""@en ;
	mhdb:takesMinutesToComplete "15"^^xsd:nonNegativeInteger ;
	mhdb:hasReferenceType disco:Questionnaire ;
	mhdb:usedByStudyOrClinic mhdb:Healthy_Brain_Network ;
	mhdb:isAboutDomain mhdb:substance_use ;
	mhdb:isAboutDomain mhdb:addiction ;
	mhdb:isForInformant mhdb:self-report ;
	dcterms:isReferencedBy mhdb:httpwwwdrugabusegovsitesdefaultfilespdfnmassistpdf .

mhdb:Negative_Life_Events_Questionnaire-Parent_Version rdfs:label """Negative Life Events Questionnaire - Parent Version"""@en ;
	rdf:type dcterms:source ;
	mhdb:hasAbbreviation mhdb:NLES-P ;
	rdfs:comment """The NLES-Parent focuses on family, community, and school-based stressors that children may be exposed to and are known to be related to negative physical and mental health outcomes. Parents are asked to rate whether the event occurred, whether the child was aware, and the child's level of resulting stress. Administration of this checklist includes the General Coping Efficacy sub-scale."""@en ;
	mhdb:takesMinutesToComplete "10"^^xsd:nonNegativeInteger ;
	mhdb:hasReferenceType disco:Questionnaire ;
	mhdb:usedByStudyOrClinic mhdb:Healthy_Brain_Network ;
	mhdb:isAboutDomain mhdb:trauma ;
	mhdb:isAboutDomain mhdb:distress_tolerance ;
	mhdb:isForInformant mhdb:parent-report ;
	dcterms:isReferencedBy mhdb:Sandler_IN_Wolchik_SA_Braver_SL__Fogas_B_1991_Stability_and_quality_of_life_events_and_psychological_symptomatology_in_children_of_divorce_American_Journal_of_Community_Psychology_194_501-520 .

mhdb:Negative_Life_Events_Questionnaire-Self_Report rdfs:label """Negative Life Events Questionnaire - Self Report"""@en ;
	rdf:type dcterms:source ;
	mhdb:hasAbbreviation mhdb:NLES-SR ;
	rdfs:comment """The NLES focuses on family, community, and school-based stressors that children may be exposed to and are known to be related to negative physical and mental health outcomes. Children are asked to rate whether the event occurred and their level of resulting stress."""@en ;
	mhdb:takesMinutesToComplete "10"^^xsd:nonNegativeInteger ;
	mhdb:hasReferenceType disco:Questionnaire ;
	mhdb:usedByStudyOrClinic mhdb:Healthy_Brain_Network ;
	mhdb:isAboutDomain mhdb:trauma ;
	mhdb:isAboutDomain mhdb:distress_tolerance ;
	mhdb:isForInformant mhdb:self-report ;
	dcterms:isReferencedBy mhdb:Sandler_IN_Wolchik_SA_Braver_SL__Fogas_B_1991_Stability_and_quality_of_life_events_and_psychological_symptomatology_in_children_of_divorce_American_Journal_of_Community_Psychology_194_501-520 .

mhdb:Physical_Activity_Questionnaire_for_Adolescents rdfs:label """Physical Activity Questionnaire for Adolescents"""@en ;
	rdf:type dcterms:source ;
	mhdb:hasAbbreviation mhdb:PAQ-A ;
	rdfs:comment """The PAQ-A (a slightly modified version of the PAQ-C with the “recess” item removed) is a self-administered, 7-day recall instrument. It was developed to assess general levels of physical activity for high school students in grades 9 to 12 and approximately 14 to 19 years of age. The PAQ-A can be administered in a classroom setting and provides a summary physical activity score derived from eight items, each scored on a 5-point scale."""@en ;
	mhdb:takesMinutesToComplete "5"^^xsd:nonNegativeInteger ;
	mhdb:hasReferenceType disco:Questionnaire ;
	mhdb:usedByStudyOrClinic mhdb:Healthy_Brain_Network ;
	mhdb:isForInformant mhdb:self-report ;
	mhdb:isForAgeGroup mhdb:adolescents ;
	dcterms:isReferencedBy mhdb:Kowalski_KC_Crocker_PR_Faulkner_RA_2007_Validation_of_the_Physical_Activity_Questionnaire_for_Older_Children_Pediatric_Exercise_Science_9_174-186 .

mhdb:Physical_Activity_Questionnaire_for_Older_Children rdfs:label """Physical Activity Questionnaire for Older Children"""@en ;
	rdf:type dcterms:source ;
	mhdb:hasAbbreviation mhdb:PAQ-C ;
	rdfs:comment """The Physical Activity Questionnaire for Children (PAQ-C) seeks information on children's participation in vigorous activities over the last 7 days. A checklist is used to determine if a child engages in physical activity during a given time period, such as the weekend or a weekday. No information is collected in regards to duration of participation, moderate or low intensity activities, or non-organized activities. An interviewer-administered 7-d recall questionnaire asks students to recall the time they spent sleeping, in moderate-intensity activities, and hard and very hard activities on each day of the previous week."""@en ;
	mhdb:takesMinutesToComplete "5"^^xsd:nonNegativeInteger ;
	mhdb:hasReferenceType disco:Questionnaire ;
	mhdb:usedByStudyOrClinic mhdb:Healthy_Brain_Network ;
	mhdb:isForInformant mhdb:self-report ;
	dcterms:isReferencedBy mhdb:Janz_K_F_Lutuchy_EM_Wenthe_P__Levy_SM_2008_Measuring_activity_in_children_and_adolescents_using_self-report_PAC-Q_and_PAQ-A_Medicine__Science_In_Sports__Exercise_404_767-772 .

mhdb:Parent-Child_Internet_Addiction_Test rdfs:label """Parent-Child Internet Addiction Test"""@en ;
	rdf:type dcterms:source ;
	mhdb:hasAbbreviation mhdb:PCIAT ;
	rdfs:comment """The PCIAT is a 20-item scale that measures characteristics and behaviors associated with compulsive use of the Internet that include compulsivity, escapism, and dependency. Questions also assess problems related to addictive use in personal, occupational, and social functioning."""@en ;
	mhdb:takesMinutesToComplete "5-10"^^xsd:string ;
	mhdb:hasReferenceType disco:Questionnaire ;
	mhdb:usedByStudyOrClinic mhdb:Healthy_Brain_Network ;
	mhdb:isAboutDomain mhdb:substance_use ;
	mhdb:isAboutDomain mhdb:addiction ;
	mhdb:isForInformant mhdb:parent-report ;
	dcterms:isReferencedBy mhdb:Young_K_S_1998_Internet_addiction_The_emergence_of_a_new_clinical_disorder_CyberPsychology_and_Behavior_13_237-244 .

mhdb:Peterson_Puberty_Scale rdfs:label """Peterson Puberty Scale"""@en ;
	rdf:type dcterms:source ;
	mhdb:hasAbbreviation mhdb:PPS ;
	rdfs:comment """The Peterson Puberty Scale is an adaptation of an interview-based puberty-rating scale by Petersen, and includes scores for each of five items rating physical development, an overall maturation measure, and a categorical maturation score. It is designed to be non-invasive, not requiring the use of pictures."""@en ;
	mhdb:takesMinutesToComplete "5"^^xsd:nonNegativeInteger ;
	mhdb:hasReferenceType disco:Questionnaire ;
	mhdb:usedByStudyOrClinic mhdb:Healthy_Brain_Network ;
	mhdb:isAboutDomain mhdb:background_information ;
	mhdb:isForInformant mhdb:self-report ;
	mhdb:isForInformant mhdb:parent-report ;
	dcterms:isReferencedBy mhdb:Petersen_A_Crockett_L_Richards_M__Boxer_A_1988_A_self-report_measure_of_pubertal_status_Reliability_validity_and_initial_norms_Journal_of_Youth_and_Adolescence_172_117-133 .

mhdb:Parenting_Stress_Index rdfs:label """Parenting Stress Index"""@en ;
	rdf:type dcterms:source ;
	mhdb:hasAbbreviation mhdb:PSI ;
	rdfs:comment """The PSITM is designed to evaluate the magnitude of stress in the parent-child system, focusing on three major domains of stress: 1) child characteristics, 2) parent characteristics, and 3) situational/demographic life stress."""@en ;
	mhdb:takesMinutesToComplete "15"^^xsd:nonNegativeInteger ;
	mhdb:hasReferenceType disco:Questionnaire ;
	mhdb:usedByStudyOrClinic mhdb:Healthy_Brain_Network ;
	mhdb:isAboutDomain mhdb:trauma ;
	mhdb:isAboutDomain mhdb:distress_tolerance ;
	mhdb:isForInformant mhdb:parent-report ;
	dcterms:isReferencedBy mhdb:Abidin_RR_2012_Parenting_stress_index_fourth_edition_PSI-4_Lutz_FL_Psychological_Assessment_Resources .

mhdb:Yale_Food_Addiction_Scale rdfs:label """Yale Food Addiction Scale"""@en ;
	rdf:type dcterms:source ;
	mhdb:hasAbbreviation mhdb:YFAS ;
	rdfs:comment """The YFAS is a measure that has been developed to identify those who are most likely to be exhibiting markers of substance dependence with the consumption of high fat/high sugar foods. This 25-item self-report measure includes mixed response categories (dichotomous and Likert-type format). A food addiction symptom (e.g., tolerance, withdrawal, loss of control) count can be obtained which is similar to the criteria for substance dependence of the DSM-IV-TR (American Psychiatric Association, 2000). Additionally, two items assess clinically significant impairment or distress from eating. Food addiction can be “diagnosed” when three symptoms and clinically significant impairment or distress are present."""@en ;
	mhdb:takesMinutesToComplete "10"^^xsd:nonNegativeInteger ;
	mhdb:hasReferenceType disco:Questionnaire ;
	mhdb:usedByStudyOrClinic mhdb:Healthy_Brain_Network ;
	mhdb:isAboutDomain mhdb:substance_use ;
	mhdb:isAboutDomain mhdb:eating ;
	mhdb:isAboutDomain mhdb:addiction ;
	mhdb:isForInformant mhdb:self-report ;
	dcterms:isReferencedBy mhdb:Gearhardt_AN_Corbin_WR__Brownell_KD_2009_Preliminary_validation_of_the_Yale_Food_Addiction_Scale_Appetite_52_430-436 .

mhdb:Multidimensional_Anxiety_Scale_for_Children_2nd_Edition-Parent_Report rdfs:label """Multidimensional Anxiety Scale for Children 2nd Edition - Parent Report"""@en ;
	rdf:type dcterms:source ;
	mhdb:hasAbbreviation mhdb:MASC-2-Parent ;
	rdfs:comment """The MASC is a normed 39-item self-report questionnaire that assesses anxiety in children and adolescents. It uses four basic scales (physical symptoms, harm avoidance, social anxiety, and separation/panic), one scale measuring total anxiety, and two additional indexes, anxiety disorder and inconsistency. Participants are asked to rate their own behavior on a 4-point scale: 0-Never true about me, 1-Rarely true about me, 2-Sometimes true about me, 3-Often true about me."""@en ;
	mhdb:hasReferenceType disco:Questionnaire ;
	mhdb:usedByStudyOrClinic mhdb:Healthy_Brain_Network ;
	mhdb:usedByStudyOrClinic mhdb:Nathan_Kline_Institute ;
	mhdb:isAboutDomain mhdb:anxiety ;
	mhdb:isAboutDomain mhdb:somatic_complaints ;
	mhdb:isForInformant mhdb:parent-report ;
	mhdb:isForAgeGroup mhdb:children ;
	dcterms:isReferencedBy mhdb:March_J_S_1998_Multi-dimensional_anxiety_scale_for_children_North_Tonawanda_NY_Multi_Health_Systems .

mhdb:Multidimensional_Anxiety_Scale_for_Children_2nd_Edition-Self_Report rdfs:label """Multidimensional Anxiety Scale for Children 2nd Edition - Self Report"""@en ;
	rdf:type dcterms:source ;
	mhdb:hasAbbreviation mhdb:MASC-2-Self ;
	rdfs:comment """The MASC is a normed 39-item self-report questionnaire that assesses anxiety in children and adolescents. It uses four basic scales (physical symptoms, harm avoidance, social anxiety, and separation/panic), one scale measuring total anxiety, and two additional indexes, anxiety disorder and inconsistency. Participants are asked to rate their own behavior on a 4-point scale: 0-Never true about me, 1-Rarely true about me, 2-Sometimes true about me, 3-Often true about me."""@en ;
	mhdb:hasReferenceType disco:Questionnaire ;
	mhdb:usedByStudyOrClinic mhdb:Healthy_Brain_Network ;
	mhdb:usedByStudyOrClinic mhdb:Nathan_Kline_Institute ;
	mhdb:isAboutDomain mhdb:anxiety ;
	mhdb:isAboutDomain mhdb:somatic_complaints ;
	mhdb:isForInformant mhdb:self-report ;
	mhdb:isForAgeGroup mhdb:children ;
	dcterms:isReferencedBy mhdb:March_J_S_1998_Multi-dimensional_anxiety_scale_for_children_North_Tonawanda_NY_Multi_Health_Systems .

mhdb:Behaviour_Rating_Inventory_of_Executive_Function-Preschool_Version rdfs:label """Behaviour Rating Inventory of Executive Function-Preschool Version"""@en ;
	rdf:type dcterms:source ;
	mhdb:hasAbbreviation mhdb:BRIEF-Preschool ;
	mhdb:hasReferenceType disco:Questionnaire ;
	mhdb:usedByStudyOrClinic mhdb:Child_Mind_Institute .

<https://www.who.int/classifications/icd/en/bluebook.pdf> rdfs:label """International Statistical Classification of Diseases and Related Health Problems of Mental and Behavioural Disorders Clinical descriptions and diagnostic guidelines"""@en ;
	rdf:type dcterms:source ;
	mhdb:hasAbbreviation mhdb:ICD-10 ;
	schema:WebSite <https://www.who.int/classifications/icd/en/bluebook.pdf> ;
	mhdb:hasReferenceType mhdb:nosology_manual .

mhdb:Ishihara_Color_Vision_Test rdfs:label """Ishihara Color Vision Test"""@en ;
	rdf:type dcterms:source ;
	mhdb:usedByStudyOrClinic mhdb:Healthy_Brain_Network .

mhdb:MATTER_Lab rdfs:label """MATTER Lab"""@en ;
	rdf:type dcterms:source ;
	mhdb:hasReferenceType schema:Person ;
	mhdb:usedByStudyOrClinic mhdb:Healthy_Brain_Network .

mhdb:Childrens_Global_Assessment_Scale rdfs:label """Children's Global Assessment Scale"""@en ;
	rdf:type dcterms:source ;
	mhdb:hasAbbreviation mhdb:CGAS ;
	rdfs:comment """The Children's Global Assessment Scale (CGAS) is a numeric scale used by mental health clinicians to rate the general functioning of youths under the age of 18. Scores range from 1 to 90 or 1 to 100, with high scores indicating better functioning."""@en ;
	mhdb:takesMinutesToComplete "5"^^xsd:nonNegativeInteger ;
	mhdb:hasReferenceType disco:Questionnaire ;
	mhdb:usedByStudyOrClinic mhdb:Healthy_Brain_Network ;
	mhdb:isAboutDomain mhdb:executive_functions ;
	mhdb:isAboutDomain mhdb:cognitive_functioning ;
	mhdb:isForInformant mhdb:self-report ;
	mhdb:isForAgeGroup mhdb:children ;
	dcterms:isReferencedBy mhdb:Shaffer_David_Gould_MS_Brasic_J_Ambrosini_P_Fisher_Prudence_Bird_Hector_Aluwahlia_S_1983_A_childrens_global_assessment_scale_CGAS_Archives_of_General_Psychiatry_40_122831 .

mhdb:Columbia_Impairment_Scale-Parent_Report_Version rdfs:label """Columbia Impairment Scale - Parent Report Version"""@en ;
	rdf:type dcterms:source ;
	mhdb:hasAbbreviation mhdb:CIS-P ;
	rdfs:comment """The CIS is a 13 item parent report scale that assesses global functioning in domains of interpersonal relations, psychopathology, school performance, use of leisure time; monitors progress after 6 months of treatment."""@en ;
	mhdb:takesMinutesToComplete "5"^^xsd:nonNegativeInteger ;
	mhdb:hasReferenceType disco:Questionnaire ;
	mhdb:usedByStudyOrClinic mhdb:Healthy_Brain_Network ;
	mhdb:isAboutDomain mhdb:general_impairment ;
	mhdb:isForInformant mhdb:parent-report ;
	dcterms:isReferencedBy mhdb:Bird_H_R_Shaffer_D_Fisher_P__Gould_M_S_1993_The_Columbia_Impairment_Scale_CIS_Pilot_findings_on_a_measure_of_global_impairment_for_children_and_adolescents_International_Journal_of_Methods_in_Psychiatric_Research .

mhdb:Extended_Strengths_and_Weaknesses_Assessment_of_Normal_Behavior rdfs:label """Extended Strengths and Weaknesses Assessment of Normal Behavior"""@en ;
	rdf:type dcterms:source ;
	mhdb:hasAbbreviation mhdb:E-SWAN ;
	rdfs:comment """The Extended Strengths and Weaknesses Assessment of Normal Behavior (E-SWAN) is a parent self-report instrument used to help assess multiple DSM Disorders and evaluate problem behavior in children and adolescents.  The disorders include Depression, Disruptive Mood Disregulation Disorder (DMDD), Social Anxiety, and Panic Disorder."""@en ;
	mhdb:takesMinutesToComplete "10"^^xsd:nonNegativeInteger ;
	mhdb:hasReferenceType disco:Questionnaire ;
	mhdb:usedByStudyOrClinic mhdb:Healthy_Brain_Network ;
	mhdb:isAboutDomain mhdb:depression ;
	mhdb:isAboutDomain mhdb:anxiety ;
	mhdb:isAboutDomain mhdb:psychotic_behavior ;
	mhdb:isAboutDomain mhdb:behavior ;
	mhdb:isAboutDomain mhdb:atypical_behavior ;
	mhdb:isAboutDomain mhdb:mood ;
	mhdb:isForInformant mhdb:parent-report .

mhdb:Food_Frequency_Questionnaire rdfs:label """Food Frequency Questionnaire"""@en ;
	rdf:type dcterms:source ;
	mhdb:hasAbbreviation mhdb:FFQ ;
	rdfs:comment """The Food Frequency Questionnaire (FFQ) is a screening tool designed to assess children's intake by food group, with outcomes measured in number of servings. The focus of these tools is on intake of fruit and fruit juices, vegetables, potatoes (including French fries), whole grains, meat/poultry/fish, dairy, legumes, saturated fat, \'added sugars\' (in sweetened cereals, soft drinks, and sweets), glycemic load and glycemic index. A secondary analysis produces estimates for intake of sugary beverages (both kcal and frequency). Individual portion sizes are asked."""@en ;
	mhdb:takesMinutesToComplete "10"^^xsd:nonNegativeInteger ;
	mhdb:hasReferenceType disco:Questionnaire ;
	mhdb:usedByStudyOrClinic mhdb:Healthy_Brain_Network ;
	mhdb:isAboutDomain mhdb:eating ;
	mhdb:isForInformant mhdb:self-report ;
	dcterms:isReferencedBy mhdb:Block_G_Hartman_AM_Dresser_CM_Carroll_MD_Gannon_J_Gardner_L_A_data-based_approach_to_diet_questionnaire_design_and_testing_Am_J_Epidemiol_1986_124453-469 .

mhdb:Peabody_Picture_Vocabulary_Test_Fourth_Edition rdfs:label """Peabody Picture Vocabulary Test, Fourth Edition"""@en ;
	rdf:type dcterms:source ;
	mhdb:hasAbbreviation mhdb:PPVT-4 ;
	rdfs:comment """The PPVT–4 scale is a norm-referenced, wide-range instrument for measuring the receptive (hearing) vocabulary of children and adults. It measures understanding of the spoken word in standard American English and thus assesses vocabulary acquisition."""@en ;
	mhdb:takesMinutesToComplete "10"^^xsd:nonNegativeInteger ;
	mhdb:usedByStudyOrClinic mhdb:Healthy_Brain_Network ;
	mhdb:isAboutDomain mhdb:learning ;
	mhdb:isAboutDomain mhdb:verbal_learning ;
	mhdb:isForAgeGroup mhdb:adults ;
	mhdb:isForAgeGroup mhdb:children ;
	dcterms:isReferencedBy mhdb:Dunn_L_M__Dunn_D_M_2007_PPVT-4_Peabody_picture_vocabulary_test_Pearson_Assessments .

mhdb:PhenX_School_Risk rdfs:label """PhenX School Risk"""@en ;
	rdf:type dcterms:source ;
	rdfs:comment """The PhenX School Risk measure can be used to identify specific school-related risk and protective factors that can predict adolescent (and later life) substance use and abuse."""@en ;
	mhdb:takesMinutesToComplete "1"^^xsd:nonNegativeInteger ;
	mhdb:hasReferenceType disco:Questionnaire ;
	mhdb:usedByStudyOrClinic mhdb:Healthy_Brain_Network ;
	mhdb:isAboutDomain mhdb:background_information ;
	mhdb:isAboutDomain mhdb:substance_use ;
	mhdb:isAboutDomain mhdb:addiction ;
	mhdb:isForInformant mhdb:self-report ;
	dcterms:isReferencedBy mhdb:Beyers_J_M_Toumbourou_J_W_Catalano_R_F_Arthur_M_W__Hawkins_J_D_2004_A_cross-national_comparison_of_risk_and_protective_factors_for_adolescent_substance_use_the_United_States_and_Australia_Journal_of_Adolescent_Health_351_3-16 ;
	dcterms:isReferencedBy mhdb:Hemphill_S_A_Heerde_J_A_Herrenkohl_T_I_Patton_G_C_Toumbourou_J_W__Catalano_R_F_2011_Risk_and_protective_factors_for_adolescent_substance_use_in_Washington_State_the_United_States_and_Victoria_Australia_A_longitudinal_study_Journal_of_Adolescent_Health_493_312-320 .

mhdb:PhenX_Neighborhood_Safety rdfs:label """PhenX Neighborhood Safety"""@en ;
	rdf:type dcterms:source ;
	rdfs:comment """The PhenX Neighborhood Safety measure is used to evaluate a respondent’s feelings toward neighborhood-level crime and safety. Studies show that neighborhood safety is relevant to a range of health outcomes, such as birth weight."""@en ;
	mhdb:takesMinutesToComplete "10"^^xsd:nonNegativeInteger ;
	mhdb:hasReferenceType disco:Questionnaire ;
	mhdb:usedByStudyOrClinic mhdb:Healthy_Brain_Network ;
	mhdb:isAboutDomain mhdb:background_information ;
	mhdb:isForInformant mhdb:parent-report ;
	dcterms:isReferencedBy mhdb:Mujahid_M_S_Diez_Roux_A_V_Morenoff_J_D__Raghunathan_T_2007_Assessing_the_measurement_properties_of_neighborhood_scales_From_psychometrics_to_ecometrics_American_Journal_of_Epidemiology_165_858-867 .

mhdb:Repetitive_Behavior_Scale-Revised rdfs:label """Repetitive Behavior Scale - Revised"""@en ;
	rdf:type dcterms:source ;
	mhdb:hasAbbreviation mhdb:RBS-R ;
	rdfs:comment """The RBS-R is a 44-item self-report questionnaire that is used to measure the breadth of repetitive behavior in children, adolescents, and adults with Autism Spectrum disorders. The RBS-R provides a quantitative, continuous measure of the full spectrum of repetitive behaviors. The RBS-R consists of six subscales including: Stereotyped Behavior, Self-injurious Behavior, Compulsive Behavior, Routine Behavior, Sameness Behavior, and Restricted Behavior, that have no overlap of item content."""@en ;
	mhdb:takesMinutesToComplete "15"^^xsd:nonNegativeInteger ;
	mhdb:hasReferenceType disco:Questionnaire ;
	mhdb:usedByStudyOrClinic mhdb:Healthy_Brain_Network ;
	mhdb:usedByStudyOrClinic mhdb:Nathan_Kline_Institute ;
	mhdb:isForInformant mhdb:parent-report ;
	mhdb:isForAgeGroup mhdb:adults ;
	dcterms:isReferencedBy mhdb:Lam_K_S_L_and_M_G_Aman_2007_The_Repetitive_Behavior_Scale-Revised_independent_validation_in_individuals_with_autism_spectrum_disorders_Journal_of_Autism_and_Developmental_Disorders_375_855-866 .

mhdb:Sleep_Disturbance_Scale_for_Children rdfs:label """Sleep Disturbance Scale for Children"""@en ;
	rdf:type dcterms:source ;
	mhdb:hasAbbreviation mhdb:SDSC ;
	rdfs:comment """The SDSC is a 27-item inventory rated on a 5 point Likert-type scale. The instrument’s purpose is to categorize sleep disorders in children. As well as giving an overall score the instrument uses five subdomains: disorders of initiating and maintaining sleep, sleep breathing disorders, disorders of arousal, sleep-wake transition disorders, disorders of excessive somnolence, and sleep hyperhidrosis."""@en ;
	mhdb:takesMinutesToComplete "5-10"^^xsd:string ;
	mhdb:hasReferenceType disco:Questionnaire ;
	mhdb:usedByStudyOrClinic mhdb:Healthy_Brain_Network ;
	mhdb:isAboutDomain mhdb:sleep ;
	mhdb:isForInformant mhdb:self-report ;
	mhdb:isForAgeGroup mhdb:children ;
	dcterms:isReferencedBy mhdb:Bruni_O_Ottavianio_S_Guidetti_V_Romoli_M_Innocenzi_M_Cortesi_F__Giannotti_F_1996_The_Sleep_Disturbance_Scale_for_Children_SDSC_Construction_and_validation_of_an_instrument_to_evaluate_sleep_disturbances_in_childhood_and_adolescence_J_Sleep_Rrs_5_251-261 .

mhdb:Social_Aptitudes_Scale rdfs:label """Social Aptitudes Scale"""@en ;
	rdf:type dcterms:source ;
	mhdb:hasAbbreviation mhdb:SAS ;
	rdfs:comment """The SAS is a 10-item parent report scale that assesses a child behaves in different social situations compared to other children of the same age. Items are rated from above to below average."""@en ;
	mhdb:takesMinutesToComplete "5"^^xsd:nonNegativeInteger ;
	mhdb:hasReferenceType disco:Questionnaire ;
	mhdb:usedByStudyOrClinic mhdb:Healthy_Brain_Network ;
	mhdb:isAboutDomain mhdb:social_interaction ;
	mhdb:isForInformant mhdb:parent-report ;
	dcterms:isReferencedBy mhdb:Liddle_Elizabeth_B_Martin_J_Batty_and_Robert_Goodman_The_social_aptitudes_scale_an_initial_validation_Social_psychiatry_and_psychiatric_epidemiology_446_2009_508-513 .

mhdb:Strengths_and_Difficulties_Questionnaire rdfs:label """Strengths and Difficulties Questionnaire"""@en ;
	rdf:type dcterms:source ;
	mhdb:hasAbbreviation mhdb:SDQ ;
	rdfs:comment """The SDQ is a brief behavioral screening questionnaire with 25 items on psychological attributes divided between 5 scales. The extended version includes an impact supplement that asks if the caregiver if participant has experienced a problem and the degree of chronicity, distress, social impairment, and burden to others. The questionnaire is administered during the initial telephone screen with the caregiver of a child or adolescent participant. For clinical assessment, SDQ helps to determine how the protocol assessments are completed and the professionals involved."""@en ;
	mhdb:takesMinutesToComplete "5"^^xsd:nonNegativeInteger ;
	mhdb:hasReferenceType disco:Questionnaire ;
	mhdb:usedByStudyOrClinic mhdb:Healthy_Brain_Network ;
	mhdb:isAboutDomain mhdb:depression ;
	mhdb:isAboutDomain mhdb:anxiety ;
	mhdb:isAboutDomain mhdb:social_interaction ;
	mhdb:isAboutDomain mhdb:cognitive_functioning ;
	mhdb:isAboutDomain mhdb:executive_functions ;
	mhdb:isAboutDomain mhdb:mood ;
	mhdb:isAboutDomain mhdb:hyperactivity ;
	mhdb:isAboutDomain mhdb:attention ;
	mhdb:isForInformant mhdb:caregiver-report ;
	dcterms:isReferencedBy mhdb:Goodman_et_al_2010_When_to_use_broader_internalising_and_externalising_subscales_instead_of_the_hypothesised_five_subscales_on_the_Strengths_and_Difficulties_Questionnaire_SDQ_data_from_British_parents_teachers_and_children_Journal_of_Abnormal_Child_Psychology_38_1179-1191 ;
	dcterms:isReferencedBy mhdb:Goodman_R_1997_The_Strengths_and_Difficulties_Questionnaire_A_Research_Note_Journal_of_Child_Psychology_and_Psychiatry38_581-586 ;
	dcterms:isReferencedBy mhdb:Goodman_R_1999_The_extended_version_of_the_Strengths_and_Difficulties_Questionnaire_as_a_guide_to_child_psychiatric_caseness_and_consequent_burden_Journal_of_Child_Psychology_and_Psychiatry_40_791-801 .

mhdb:Yale_Global_Tic_Severity_Scale rdfs:label """Yale Global Tic Severity Scale"""@en ;
	rdf:type dcterms:source ;
	mhdb:hasAbbreviation mhdb:Y-GTSS ;
	rdfs:comment """The Y-GTSS is a semi-structured clinician rated instrument that assesses the nature of motor and phonic tics, and is administered as part of the KSADS interview, if indicated."""@en ;
	mhdb:takesMinutesToComplete "10"^^xsd:nonNegativeInteger ;
	mhdb:hasReferenceType disco:Questionnaire ;
	mhdb:usedByStudyOrClinic mhdb:Healthy_Brain_Network ;
	mhdb:usedByStudyOrClinic mhdb:Nathan_Kline_Institute ;
	mhdb:isAboutDomain mhdb:psychotic_behavior ;
	mhdb:isAboutDomain mhdb:behavior ;
	mhdb:isAboutDomain mhdb:atypical_behavior ;
	mhdb:isAboutDomain mhdb:tics ;
	mhdb:isForInformant mhdb:self-report ;
	dcterms:isReferencedBy mhdb:Leckman_JF_Riddle_MA_Hardin_MT_Ort_SL_Swartz_KL_Stevenson_J_et_al_1989_The_Yale_Global_Tic_Severity_Scale_Initial_testing_of_a_clinician-rated_scale_of_tic_severity_Journal_of_the_American_Academy_of_Child_and_Adolescent_Psychiatry_28_566573 .

mhdb:WHO_Disability_Assessment_Schedule__Self_Report rdfs:label """WHO Disability Assessment Schedule – Self Report"""@en ;
	rdf:type dcterms:source ;
	mhdb:hasAbbreviation mhdb:WHODAS-SR ;
	rdfs:comment """The WHODAS is a generic assessment instrument for health and disability. It assesses function across domains of cognition, mobility, self-care, getting along, life activities, and participation."""@en ;
	mhdb:takesMinutesToComplete "5"^^xsd:nonNegativeInteger ;
	mhdb:hasReferenceType disco:Questionnaire ;
	mhdb:usedByStudyOrClinic mhdb:Healthy_Brain_Network ;
	mhdb:isAboutDomain mhdb:general_impairment ;
	mhdb:isForInformant mhdb:self-report ;
	dcterms:isReferencedBy mhdb:Gold_Liza_H_DSM-5_and_the_assessment_of_functioning_the_World_Health_Organization_Disability_Assessment_Schedule_20_WHODAS_20_Journal_of_the_American_Academy_of_Psychiatry_and_the_Law_Online_422_2014_173-181 .

mhdb:University_of_California_Los_Angeles_Trauma_Reactivity_Scale_for_DSM-5 rdfs:label """University of California Los Angeles Trauma Reactivity Scale for DSM-5"""@en ;
	rdf:type dcterms:source ;
	mhdb:hasAbbreviation mhdb:UCLA-DSM-5 ;
	rdfs:comment """The UCLA is a 31-item questionnaire used to assess PTSD symptoms. When answering the questions, the child should think about the traumatic event that is most bothersome to him/her currently and rate the frequency of symptoms in the past month."""@en ;
	mhdb:takesMinutesToComplete "15"^^xsd:nonNegativeInteger ;
	mhdb:hasReferenceType disco:Questionnaire ;
	mhdb:usedByStudyOrClinic mhdb:Healthy_Brain_Network ;
	mhdb:isAboutDomain mhdb:trauma ;
	mhdb:isAboutDomain mhdb:distress_tolerance ;
	mhdb:isForInformant mhdb:self-report ;
	dcterms:isReferencedBy mhdb:Steinberg_A_M_Brymer_M_J_Decker_K_B__Pynoos_R_S_2004_The_University_of_California_at_Los_Angeles_post-traumatic_stress_disorder_reaction_index_Current_psychiatry_reports_62_96-100 .

mhdb:Kiddie_Schedule_for_Affective_Disorders_and_Schizophrenia rdfs:label """Kiddie Schedule for Affective Disorders and Schizophrenia"""@en ;
	rdf:type dcterms:source ;
	mhdb:hasAbbreviation mhdb:K-SADS ;
	mhdb:usedByStudyOrClinic mhdb:Healthy_Brain_Network ;
	mhdb:isAboutDomain mhdb:psychotic_behavior .

mhdb:Vineland_Adaptive_Behavior_Scale-ParentCaregiver_Rating_Form rdfs:label """Vineland Adaptive Behavior Scale - Parent/Caregiver Rating Form"""@en ;
	rdf:type dcterms:source ;
	mhdb:usedByStudyOrClinic mhdb:Healthy_Brain_Network ;
	mhdb:isForInformant mhdb:parent-report ;
	mhdb:isForInformant mhdb:caregiver-report .

mhdb:Pregnancy_and_Birth_Questionnaire rdfs:label """Pregnancy and Birth Questionnaire"""@en ;
	rdf:type dcterms:source ;
	mhdb:hasAbbreviation mhdb:PBQ ;
	mhdb:hasReferenceType disco:Questionnaire ;
	mhdb:usedByStudyOrClinic mhdb:Healthy_Brain_Network .

mhdb:Yale-Brown_Obsessive_Compulsive_Scale rdfs:label """Yale-Brown Obsessive Compulsive Scale"""@en ;
	rdf:type dcterms:source ;
	mhdb:hasAbbreviation mhdb:Y-BOCS ;
	rdfs:comment """The Y-BOCS is a semi-structured clinician rated instrument to assess the severity of obsessive-compulsive disorder (OCD) symptoms that is administered as part of the KSADS interview, if indicated."""@en ;
	mhdb:hasReferenceType disco:Questionnaire ;
	mhdb:usedByStudyOrClinic mhdb:Healthy_Brain_Network ;
	mhdb:usedByStudyOrClinic mhdb:Nathan_Kline_Institute ;
	mhdb:isAboutDomain mhdb:psychotic_behavior ;
	mhdb:isAboutDomain mhdb:behavior ;
	mhdb:isAboutDomain mhdb:atypical_behavior ;
	mhdb:isForInformant mhdb:self-report ;
	dcterms:isReferencedBy mhdb:Storch_E_A_Larson_M_J_Goodman_W_K_Rasmussen_S_A_Price_L_H__Murphy_T_K_2010 .

mhdb:Young_Mania_Rating_Scale rdfs:label """Young Mania Rating Scale"""@en ;
	rdf:type dcterms:source ;
	mhdb:hasReferenceType disco:Questionnaire ;
	mhdb:usedByStudyOrClinic mhdb:Child_Mind_Institute ;
	mhdb:isAboutDomain mhdb:mania .

mhdb:The_Childrens_behavior_Questionnaire_Very_Short_Form rdfs:label """The Children's behavior Questionnaire (Very Short Form)"""@en ;
	rdf:type dcterms:source ;
	mhdb:hasAbbreviation mhdb:CBQ-VSF ;
	rdfs:comment """The CBQ-VSF is a 36-item informant-report questionnaire assessing temperament of children (ages 3 – 8). The questionnaire is designed to capture three broad dimensions: surgency/extraversion, negative affectivity, and effortful control. Informants are asked to rate their child based on how they feel that their child’s reaction is likely to be in a variety of situations. Responses are given on a 7-point scale ranging from 1 (extremely untrue of my child) to 7 (extremely true of my child). The questionnaire is designed to capture three broad dimensions: surgency/extraversion, negative affectivity, and effortful control. Participants are asked to rate how well the items describe their child on a 7-point scale: 1-extremely untrue of my child, 2-quite untrue, 3- slightly untrue, 4-neither true nor untrue, 5-slightly true, 6-quite true, 7-extremely true of my child."""@en ;
	mhdb:hasReferenceType disco:Questionnaire ;
	mhdb:usedByStudyOrClinic mhdb:Nathan_Kline_Institute ;
	mhdb:isAboutDomain mhdb:depression ;
	mhdb:isAboutDomain mhdb:impulsivity ;
	mhdb:isAboutDomain mhdb:anxiety ;
	mhdb:isAboutDomain mhdb:risk_taking ;
	mhdb:isAboutDomain mhdb:mood ;
	mhdb:isAboutDomain mhdb:hyperactivity ;
	mhdb:isAboutDomain mhdb:attention ;
	mhdb:isAboutDomain mhdb:personality_traits ;
	mhdb:isForInformant mhdb:parent-report ;
	dcterms:isReferencedBy mhdb:Putnam_S_P__Rothbart_M_K_2006_Development_of_short_and_very_short_forms_of_the_childrens_behavior_questionnaire_Journal_of_Personality_Assessment_871_102-112__Rothbart_M_K_Ahadi_S_A_Hershey_K_L__Fisher_P_2001_Investigations_of_temperament_at_three_to_seven_years_The_childrens_behavior_questionnaire_Child_Development_725_1394-1408 .

mhdb:Geriatric_Depression_Scale rdfs:label """Geriatric Depression Scale"""@en ;
	rdf:type dcterms:source ;
	mhdb:hasAbbreviation mhdb:GDS ;
	mhdb:hasReferenceType disco:Questionnaire ;
	mhdb:usedByStudyOrClinic mhdb:Nathan_Kline_Institute .

mhdb:Child_Eating_Behaviour_Questionnaire rdfs:label """Child Eating Behaviour Questionnaire"""@en ;
	rdf:type dcterms:source ;
	mhdb:hasAbbreviation mhdb:CEBQ ;
	rdfs:comment """The CEBQ is a 35-item informant-report questionnaire assessing eating style in children. Eating style is assessed on 8 scales (food responsiveness, enjoyment of food, emotional overeating, desire to drink, satiety responsiveness, slowness in eating, emotional undereating, and fussiness). Informants rate the frequency of their child’s behaviors and experiences on a 5-point scale: 1-never, 2-rarely, 3-sometimes, 4-often, 5-always."""@en ;
	mhdb:hasReferenceType disco:Questionnaire ;
	mhdb:usedByStudyOrClinic mhdb:Nathan_Kline_Institute ;
	mhdb:isAboutDomain mhdb:fussiness ;
	mhdb:isAboutDomain mhdb:slowness_in_eating ;
	mhdb:isAboutDomain mhdb:emotional_overeating ;
	mhdb:isAboutDomain mhdb:eating ;
	mhdb:isAboutDomain mhdb:desire_to_drink ;
	mhdb:isAboutDomain mhdb:enjoyment_of_food ;
	mhdb:isAboutDomain mhdb:food_responsiveness ;
	mhdb:isAboutDomain mhdb:satiety_responsiveness ;
	mhdb:isAboutDomain mhdb:emotional_undereating ;
	mhdb:isForInformant mhdb:parent-report ;
	mhdb:isForAgeGroup mhdb:children ;
	dcterms:isReferencedBy mhdb:Wardle_J_Guthrie_C_A_Sanderson_S__Rapoport_L_2001_Development_of_the_childrens_eating_behaviour_questionnaire_Journal_of_Child_Psychology_and_Psychiatry_4207_963-970 .

mhdb:The_Cambridge-Hopkins_Restless_Legs_Syndrome_Version_2 rdfs:label """The Cambridge-Hopkins Restless Legs Syndrome (Version 2)"""@en ;
	rdf:type dcterms:source ;
	mhdb:hasAbbreviation mhdb:CHRLS ;
	mhdb:hasReferenceType disco:Questionnaire ;
	mhdb:usedByStudyOrClinic mhdb:Nathan_Kline_Institute .

mhdb:Eating_Disorder_Examination_Questionnaire rdfs:label """Eating Disorder Examination Questionnaire"""@en ;
	rdf:type dcterms:source ;
	mhdb:hasAbbreviation mhdb:EDEQ ;
	rdfs:comment """The EDEQ is a 36-item self-report measure that is an adapted version of the Eating Disorder Examination (EDE). The measure is a comprehensive assessment of the specific psychopathology of eating disordered behavior, and asks participants to respond based on the past four weeks (28 days) only. Participants are asked to enter the number of days or times they have exhibited certain eating disordered thoughts or behaviors or asked to rate these on a 7-point scale of frequency in the past month: 0-no days, 1-1 to 5 days, 2-6 to 12 days, 3-13 to 15 days, 4-16 to 22 days, 5-23 to 27 days, 6-every day."""@en ;
	mhdb:hasReferenceType disco:Questionnaire ;
	mhdb:usedByStudyOrClinic mhdb:Nathan_Kline_Institute ;
	mhdb:isAboutDomain mhdb:eating ;
	mhdb:isAboutDomain mhdb:eating_disordered_behavior ;
	mhdb:isAboutDomain mhdb:eating_disordered_thoughts ;
	mhdb:isForInformant mhdb:self-report ;
	mhdb:isForAgeGroup mhdb:adults ;
	mhdb:isForAgeGroup mhdb:adolescents ;
	dcterms:isReferencedBy mhdb:Mond_J_M_Hay_P_J_Rodgers_B_Owen_C__Beumont_P_J_2004_Validity_of_the_eating_disorder_examination_questionnaire_EDE-Q_in_screening_for_eating_disorders_in_community_samples_Behaviour_Research_and_Therapy_425_551-67_Fairburn_C_G__Cooper_Z_1993_The_Eating_Disorder_Examination_twelfth_edition_In_C_G_Fairburn__G_T_Wilson_eds_Binge_Eating_Nature_Assessment_and_Treatment_pp_317-_360_New_York_Guilford_Press_1993 .

mhdb:Interpersonal_Reactivity_Index rdfs:label """Interpersonal Reactivity Index"""@en ;
	rdf:type dcterms:source ;
	mhdb:hasAbbreviation mhdb:IRI ;
	rdfs:comment """The IRI is a 28-item self- report, and is a well-validated multidimensional measure of empathic ability. Each item includes a statement about thoughts and feelings in a variety of situations, and participants are asked to indicate how well each statement describes them on a 5-point scale: 0-Does not describe me well to 4-Describes me very well."""@en ;
	mhdb:hasReferenceType disco:Questionnaire ;
	mhdb:usedByStudyOrClinic mhdb:Nathan_Kline_Institute ;
	mhdb:isAboutDomain mhdb:personality_traits ;
	mhdb:isForInformant mhdb:self-report ;
	dcterms:isReferencedBy mhdb:Davis_M_H_1983_Measuring_individual_differences_in_empathy_Evidence_for_a_multidimensional_approach_Journal_of_Personality_and_Social_Psychology_44_113-126 ;
	dcterms:isReferencedBy mhdb:Mark_H_Davis_1980_A_multidimensional_approach_to_individual_difference_in_empathy_JSAS_Catalog_of_Selected_Documents_in_Psychology_10_85 .

mhdb:The_21-Item_Peters_et_al_Delusions_Inventory rdfs:label """The 21-Item Peters et al. Delusions Inventory"""@en ;
	rdf:type dcterms:source ;
	mhdb:hasAbbreviation mhdb:PDI-21 ;
	rdfs:comment """The PDI-21 is a self-report designed to measure schizotypal traits and symptoms in the general population, using the Present State Examination as a template. The PDI-21 incorporates the multidimensionality of delusions, including measures of distress, preoccupation, and conviction."""@en ;
	mhdb:hasReferenceType disco:Questionnaire ;
	mhdb:usedByStudyOrClinic mhdb:Nathan_Kline_Institute ;
	mhdb:isAboutDomain mhdb:psychotic_behavior ;
	mhdb:isAboutDomain mhdb:behavior ;
	mhdb:isAboutDomain mhdb:atypical_behavior ;
	mhdb:isForInformant mhdb:self-report ;
	dcterms:isReferencedBy mhdb:Peters_E_R_Joseph_S_A__Garety_P_A_1999_Measurement_of_delusional_ideation_in_the_normal_population_Introducing_the_PDI_peters_et_al_Delusions_inventory_Schizophrenia_Bulletin_253_553-576 .

mhdb:Pittsburgh_Sleep_Quality_Index rdfs:label """Pittsburgh Sleep Quality Index"""@en ;
	rdf:type dcterms:source ;
	mhdb:hasAbbreviation mhdb:PSQI ;
	rdfs:comment """The PSQI is a 10-item self-report questionnaire that is designed to measure sleep quality in clinical populations, and assess usual sleep habits during the past one-month. This scale generates seven “component” scores: subjective sleep quality, sleep latency, sleep duration, habitual sleep efficiency, sleep disturbances, use of sleeping medication, and daytime dysfunction. Items 1-4 inquire about the amount of sleep and responses are recorded in free-text boxes. Items 5-10 inquire about specific sleep behaviors and quality, which are rated on 4-point scale."""@en ;
	mhdb:hasReferenceType disco:Questionnaire ;
	mhdb:usedByStudyOrClinic mhdb:Nathan_Kline_Institute ;
	mhdb:isAboutDomain mhdb:sleep ;
	mhdb:isAboutDomain mhdb:subjective_sleep_quality ;
	mhdb:isAboutDomain mhdb:daytime_dysfunction ;
	mhdb:isAboutDomain mhdb:sleep_disturbances ;
	mhdb:isAboutDomain mhdb:use_of_sleeping_medication ;
	mhdb:isAboutDomain mhdb:habitual_sleep_efficiency ;
	mhdb:isAboutDomain mhdb:sleep_duration ;
	mhdb:isAboutDomain mhdb:sleep_latency ;
	mhdb:isForInformant mhdb:self-report ;
	dcterms:isReferencedBy mhdb:BuysseDJ_ReynoldsCF_MonkTH_BermanSR__KupferDJ_1989_The_Pittsburgh_Sleep_Quality_Index_PSQI_A_new_instrument_for_psychiatric_research_and_practice_Psychiatry_Research_282_193-213 .

mhdb:Emotional_Regulation_Questionnaire rdfs:label """Emotional Regulation Questionnaire"""@en ;
	rdf:type dcterms:source ;
	mhdb:hasAbbreviation mhdb:ERQ ;
	rdfs:comment """The ERQ is a 10-item, self-administered, Likert scale questionnaire for adults that is designed to assess individual differences in the habitual use of two emotion regulation strategies: cognitive reappraisal and expressive suppression. Items are rated on a seven point scale: 1-Strongly Disagree, 4-Neutral, 7-Strongly Agree. The questionnaire provides scores for reappraisal and suppression."""@en ;
	mhdb:hasReferenceType disco:Questionnaire ;
	mhdb:usedByStudyOrClinic mhdb:Nathan_Kline_Institute ;
	mhdb:isAboutDomain mhdb:mood ;
	mhdb:isAboutDomain mhdb:depression ;
	mhdb:isAboutDomain mhdb:cognitive_reapprisal ;
	mhdb:isAboutDomain mhdb:expressive_suppression ;
	mhdb:isForAgeGroup mhdb:adults ;
	dcterms:isReferencedBy mhdb:Gross_JJ__John_OP_2003_Individual_differences_in_two_emotion_regulation_processes_Implications_for_affect_relationships_and_well-being_Journal_of_Personality_and_Social_Psychology_85_348-362 .

mhdb:The_Penn_State_Worry_Questionnaire rdfs:label """The Penn State Worry Questionnaire"""@en ;
	rdf:type dcterms:source ;
	mhdb:hasAbbreviation mhdb:PSWQ ;
	rdfs:comment """The PSWQ is a self-administered, 16-item, Likert-type scale designed to measure worry. It is considered by many to be the “gold-standard” for assessing worry. The items on the scale assess the occurrence, intrusiveness, pervasiveness, and other characterizing features of an individual’s experience with worry. The scale has been shown to identify worry, over and above anxiety and depression. Items are rated on a five-point scale: 1-Not at all typical of me to 5-Very typical of me. Possible range of scores is 16-80 with the algorithm of Total scores: 16-39Low Worry, 40-59 Moderate Worry, and 60-80 High Worry."""@en ;
	mhdb:hasReferenceType disco:Questionnaire ;
	mhdb:usedByStudyOrClinic mhdb:Nathan_Kline_Institute ;
	mhdb:isAboutDomain mhdb:anxiety ;
	mhdb:isAboutDomain mhdb:depression ;
	mhdb:isAboutDomain mhdb:mood ;
	dcterms:isReferencedBy mhdb:Meyer_TJ_Miller_ML_Metzger_RL_Borkovec_TD_1990_Development_and_validation_of_the_Penn_State_Worry_Questionnaire_Beh_Research_and_Therapy_28_487-495 .

mhdb:Ruminative_Responses_Scale rdfs:label """Ruminative Responses Scale"""@en ;
	rdf:type dcterms:source ;
	mhdb:hasAbbreviation mhdb:RRS ;
	rdfs:comment """The RRS is a revision of the original, longer Response Styles Questionnaire. The RRS was developed to more directly and reliably assess rumination that is related to, but not confounded by depression. The 22 items of the RRS measure two aspects of rumination, brooding and reflective pondering. Items are rated on a four-point scale: 1-Almost Never, 2-Sometimes, 3-Often, 4-Almost always. The questionnaire provides scores for the following scales: Brooding, Reflection, and Depression"""@en ;
	mhdb:hasReferenceType disco:Questionnaire ;
	mhdb:usedByStudyOrClinic mhdb:Nathan_Kline_Institute ;
	mhdb:isAboutDomain mhdb:depression ;
	mhdb:isAboutDomain mhdb:mood ;
	dcterms:isReferencedBy mhdb:Treynor_W_Gonzalez_R_Nolen-Hoeksema_S_2003_Rumination_Reconsidered_A_Psychometric_Analysis_Cognitive_Therapy_and_Research_273_247-259 .

mhdb:Short_Imaginal_Process_Inventory rdfs:label """Short Imaginal Process Inventory"""@en ;
	rdf:type dcterms:source ;
	mhdb:hasAbbreviation mhdb:SIPI ;
	rdfs:comment """The SIPI is a 45-item, self-administered, Likert scale questionnaire designed to measure aspects of daydreaming style and content, mental style, and general inner experience. Items are rated on a five-point scale: 1-Very true or strongly characteristic of me, 2-Moderately true or characteristic of me, 3-Neither particularly characteristic nor uncharacteristic of me, 4-Moderately untrue or uncharacteristic of me, 5-Definitely untrue or strongly uncharacteristic of me."""@en ;
	mhdb:hasReferenceType disco:Questionnaire ;
	mhdb:usedByStudyOrClinic mhdb:Nathan_Kline_Institute ;
	mhdb:isAboutDomain mhdb:hyperactivity ;
	mhdb:isAboutDomain mhdb:attention ;
	dcterms:isReferencedBy mhdb:Huba_G_J_Aneshensel_C_S_Singer_J_L_1981_Development_of_scales_for_three_second-order_factors_of_inner_experience_Multivariate_Behav_Res_16_181206 .

mhdb:Ohio_State_University_TBI_Identification_Method_Short_Form rdfs:label """Ohio State University TBI Identification Method Short Form"""@en ;
	rdf:type dcterms:source ;
	mhdb:hasAbbreviation mhdb:OSU_TBI-ID-SF ;
	mhdb:hasReferenceType disco:Questionnaire ;
	mhdb:usedByStudyOrClinic mhdb:Nathan_Kline_Institute .

mhdb:Vancouver_Index_of_Acculturation rdfs:label """Vancouver Index of Acculturation"""@en ;
	rdf:type dcterms:source ;
	mhdb:hasAbbreviation mhdb:VIA ;
	mhdb:hasReferenceType disco:Questionnaire ;
	mhdb:usedByStudyOrClinic mhdb:Adolescent_Brain_Cognitive_Development_Study .

mhdb:The_Hollingshead_Four_Factor_Index_of_Socioeconomic_Status rdfs:label """The Hollingshead Four Factor Index of Socioeconomic Status"""@en ;
	rdf:type dcterms:source ;
	mhdb:hasAbbreviation mhdb:SES-Adult ;
	rdfs:comment """The Hollingshead Four Factor Index of Socioeconomic Status is a survey designed to measure social status of an individual based on four domains: marital status, retired/employed status, educational attainment, and occupational prestige."""@en ;
	mhdb:hasReferenceType disco:Questionnaire ;
	mhdb:usedByStudyOrClinic mhdb:Nathan_Kline_Institute ;
	mhdb:isAboutDomain mhdb:social_status ;
	mhdb:isForInformant mhdb:self-report ;
	mhdb:isForAgeGroup mhdb:adults ;
	dcterms:isReferencedBy mhdb:Hollingshead_A_A_1975_Four-factor_index_of_social_status_Unpublished_manuscript_Yale_University_New_Haven_CT .

mhdb:Hollingshead_Socioeconomic_Status_Scale-Child_Version rdfs:label """Hollingshead Socioeconomic Status Scale-Child Version"""@en ;
	rdf:type dcterms:source ;
	mhdb:hasAbbreviation mhdb:SES-Child ;
	rdfs:comment """The Hollingshead Four Factor Index of Socioeconomic Status is a survey designed to measure social status of an individual based on four domains: marital status, retired/employed status, educational attainment, and occupational prestige."""@en ;
	mhdb:hasReferenceType disco:Questionnaire ;
	mhdb:usedByStudyOrClinic mhdb:Nathan_Kline_Institute ;
	mhdb:isAboutDomain mhdb:background_information ;
	mhdb:isForInformant mhdb:parent-report ;
	mhdb:isForAgeGroup mhdb:children ;
	dcterms:isReferencedBy mhdb:Hollingshead_A_A_1975_Four-factor_index_of_social_status_Unpublished_manuscript_Yale_University_New_Haven_CT .

mhdb:Medication_Form rdfs:label """Medication Form"""@en ;
	rdf:type dcterms:source ;
	mhdb:hasReferenceType disco:Questionnaire ;
	mhdb:usedByStudyOrClinic mhdb:Nathan_Kline_Institute .

mhdb:Medical_History-Adult rdfs:label """Medical History-Adult"""@en ;
	rdf:type dcterms:source ;
	mhdb:hasReferenceType disco:Questionnaire ;
	mhdb:usedByStudyOrClinic mhdb:Nathan_Kline_Institute ;
	mhdb:isForAgeGroup mhdb:adults .

mhdb:Sex-role_Identity_Scale rdfs:label """Sex-role Identity Scale"""@en ;
	rdf:type dcterms:source ;
	rdfs:comment """The Sex Role Identity Scale assesses an individual’s gender role characterization."""@en ;
	mhdb:hasReferenceType disco:Questionnaire ;
	mhdb:usedByStudyOrClinic mhdb:Nathan_Kline_Institute ;
	dcterms:isReferencedBy mhdb:Suggested_by_Dr_Theo_Sandfort_Adapted_from_Sex_Role_Identity_Scale_Journal_of_Personality_and_Social_Psychology_1979_Vol_37_No_10_1779-1789 .

mhdb:PhenX_Sexual_History rdfs:label """PhenX Sexual History"""@en ;
	rdf:type dcterms:source ;
	rdfs:comment """The PhenX provides an objective assessment of self-reported sexual behaviors."""@en ;
	mhdb:hasReferenceType disco:Questionnaire ;
	mhdb:usedByStudyOrClinic mhdb:Nathan_Kline_Institute ;
	mhdb:isAboutDomain mhdb:sex_and_gender ;
	mhdb:isForInformant mhdb:self-report ;
	mhdb:isForAgeGroup mhdb:adults ;
	mhdb:isForAgeGroup mhdb:adolescents .

mhdb:Sexual_Orientation_Scale rdfs:label """Sexual Orientation Scale"""@en ;
	rdf:type dcterms:source ;
	rdfs:comment """The Sexual Orientation Scale assesses self-reported sexual preference."""@en ;
	mhdb:hasReferenceType disco:Questionnaire ;
	mhdb:usedByStudyOrClinic mhdb:Nathan_Kline_Institute ;
	mhdb:isAboutDomain mhdb:sex_and_gender ;
	mhdb:isForInformant mhdb:self-report ;
	mhdb:isForAgeGroup mhdb:adults ;
	mhdb:isForAgeGroup mhdb:adolescents .

mhdb:Adult_ADHD_Clinical_Diagnostic_Scale rdfs:label """Adult ADHD Clinical Diagnostic Scale:"""@en ;
	rdfs:label """Adult ADHD Clinical Diagnostic Scale"""@en ;
	rdf:type dcterms:source ;
	mhdb:hasAbbreviation mhdb:ACDS ;
	mhdb:hasReferenceType disco:Questionnaire ;
	mhdb:usedByStudyOrClinic mhdb:Nathan_Kline_Institute ;
	mhdb:isForAgeGroup mhdb:adults .

mhdb:Behavior_Assessment_System_for_Children_Second_Edition_Ages_6-11 rdfs:label """Behavior Assessment System for Children, Second Edition (Ages 6-11)"""@en ;
	rdf:type dcterms:source ;
	mhdb:hasAbbreviation mhdb:BASC-2_Ages_6-11 ;
	rdfs:comment """The BASC-2 (6-11) a 160-item informant-report questionnaire assessing the adaptive and problem behaviors of children (ages 6 – 11) in the community and home setting. It provides scores for the following scales: anger control, bullying, developmental social disorders, emotional self-control, executive functioning, negative emotionality, and resiliency. Informants report on the child’s behavior in the last several months using a 4- point scale: 0-never, 1-sometimes, 2-often, 3-almost always."""@en ;
	mhdb:hasReferenceType disco:Questionnaire ;
	mhdb:usedByStudyOrClinic mhdb:Nathan_Kline_Institute ;
	mhdb:isAboutDomain mhdb:negative_emotionality ;
	mhdb:isAboutDomain mhdb:impulsivity ;
	mhdb:isAboutDomain mhdb:alerting_attention_Alerting_involves_a_change_in_mental_state_as_well_as_in_physiological_state_and_prepares_the_organism_for_fast_reactions_orienting_attention ;
	mhdb:isAboutDomain mhdb:anger_control ;
	mhdb:isAboutDomain mhdb:anxiety ;
	mhdb:isAboutDomain mhdb:social_interaction ;
	mhdb:isAboutDomain mhdb:mood ;
	mhdb:isAboutDomain mhdb:resiliency ;
	mhdb:isAboutDomain mhdb:behavior ;
	mhdb:isAboutDomain mhdb:atypical_behavior ;
	mhdb:isAboutDomain mhdb:emotional_self_control ;
	mhdb:isAboutDomain mhdb:hyperactivity ;
	mhdb:isAboutDomain mhdb:bullying ;
	mhdb:isAboutDomain mhdb:attention ;
	mhdb:isAboutDomain mhdb:aggression ;
	mhdb:isAboutDomain mhdb:personality_traits ;
	mhdb:isForInformant mhdb:parent-report ;
	mhdb:isForAgeGroup mhdb:children ;
	dcterms:isReferencedBy mhdb:Reynolds_C_R__Kamphaus_R_W_1992_BASC_Behavior_assessment_system_for_children_Manual_American_Guidance_Service_Incorporated .

mhdb:Behavior_Assessment_System_for_Children_Second_Edition_12-17 rdfs:label """Behavior Assessment System for Children, Second Edition 12-17"""@en ;
	rdf:type dcterms:source ;
	mhdb:hasAbbreviation mhdb:BASC-2_12-17 ;
	rdfs:comment """The BASC – 2 (12-17) is a 150-item informant-report questionnaire assessing the adaptive and problem behaviors of adolescents (ages 12 – 17) in the community and home setting. It provides scores for the following scales: anger control, bullying, developmental social disorders, emotional self-control, executive functioning, negative emotionality, and resiliency. Informants report on the adolescent’s behavior in the last several months using a 4- point scale: 0-never, 1-sometimes, 2-often, 3-almost always."""@en ;
	mhdb:hasReferenceType disco:Questionnaire ;
	mhdb:usedByStudyOrClinic mhdb:Nathan_Kline_Institute ;
	mhdb:isAboutDomain mhdb:negative_emotionality ;
	mhdb:isAboutDomain mhdb:impulsivity ;
	mhdb:isAboutDomain mhdb:alerting_attention_Alerting_involves_a_change_in_mental_state_as_well_as_in_physiological_state_and_prepares_the_organism_for_fast_reactions_orienting_attention ;
	mhdb:isAboutDomain mhdb:anger_control ;
	mhdb:isAboutDomain mhdb:anxiety ;
	mhdb:isAboutDomain mhdb:social_interaction ;
	mhdb:isAboutDomain mhdb:substance_use ;
	mhdb:isAboutDomain mhdb:mood ;
	mhdb:isAboutDomain mhdb:resiliency ;
	mhdb:isAboutDomain mhdb:behavior ;
	mhdb:isAboutDomain mhdb:emotional_self_control ;
	mhdb:isAboutDomain mhdb:hyperactivity ;
	mhdb:isAboutDomain mhdb:bullying ;
	mhdb:isAboutDomain mhdb:somatic_complaints ;
	mhdb:isAboutDomain mhdb:attention ;
	mhdb:isAboutDomain mhdb:aggression ;
	mhdb:isAboutDomain mhdb:personality_traits ;
	mhdb:isForInformant mhdb:parent-report ;
	dcterms:isReferencedBy mhdb:Reynolds_C_R__Kamphaus_R_W_1992_BASC_Behavior_assessment_system_for_children_Manual_American_Guidance_Service_Incorporated .

mhdb:Quantify_Meditation_Experience rdfs:label """Quantify Meditation Experience"""@en ;
	rdf:type dcterms:source ;
	mhdb:hasAbbreviation mhdb:QME ;
	mhdb:hasReferenceType disco:Questionnaire ;
	mhdb:usedByStudyOrClinic mhdb:Nathan_Kline_Institute .

mhdb:Perseverative_Thought_Questionnaire rdfs:label """Perseverative Thought Questionnaire"""@en ;
	rdf:type dcterms:source ;
	mhdb:hasAbbreviation mhdb:PTQ ;
	rdfs:comment """The PTQ is a self-administered, 15-item, Likert-type scale designed to measure the broad idea of repetitive negative thought. The items on the scale assess what are considered to be the core aspects of repetitive negative thought: 1) their repetitive and intrusive nature, 2) the perceived unproductive nature of these thoughts, and 3) the way in which this type of thinking captures mental capacity. Items are rated on a five-point scale: 0-Never, 1-Rarely, 2-Sometimes, 3-Often, 4-Almost Always."""@en ;
	mhdb:hasReferenceType disco:Questionnaire ;
	mhdb:usedByStudyOrClinic mhdb:Nathan_Kline_Institute ;
	mhdb:isAboutDomain mhdb:anxiety ;
	mhdb:isAboutDomain mhdb:depression ;
	mhdb:isAboutDomain mhdb:mood ;
	dcterms:isReferencedBy mhdb:Ehring_T_Zetsche_U_Weidacker_K_Wahl_K_Schonfeld_S__Ehlers_A_2011_The_Perseverative_Thinking_Questionnaire_PTQ_Validation_of_a_content-independent_measure_of_repetitive_negative_thinking_Journal_of_Behavior_Therapy_and_Experimental_Psychiatry_42_225-232 .

mhdb:Affect_Intensity_Measure rdfs:label """Affect Intensity Measure"""@en ;
	rdf:type dcterms:source ;
	mhdb:hasAbbreviation mhdb:AIM ;
	rdfs:comment """The AIM is a self-administered, 40-item, Likert scale questionnaire designed to measure the strength or weakness with which one experiences both positive and negative emotions. The questionnaire provides scores for the following scales: Negative Intensity, Positive Intensity, Negative Affectivity, and Positive Affectivity. Items are rated on a six-point scale: 1-Never, 2-Almost Never, 3-Occasionally, 4-Usually, 5-Almost Always, 6-Always."""@en ;
	mhdb:hasReferenceType disco:Questionnaire ;
	mhdb:usedByStudyOrClinic mhdb:Nathan_Kline_Institute ;
	mhdb:isAboutDomain mhdb:depression ;
	mhdb:isAboutDomain mhdb:positive_intensity ;
	mhdb:isAboutDomain mhdb:positive_affectivity ;
	mhdb:isAboutDomain mhdb:negative_affectivity ;
	mhdb:isAboutDomain mhdb:negative_intensity ;
	mhdb:isAboutDomain mhdb:mood ;
	dcterms:isReferencedBy mhdb:Larsen_RJ_Diener_E_Emmons_RA_1986_Affect_intensity_and_reactions_to_daily_life_events_Journal_of_Personality_and_Social_Psychology_51_803814 .

mhdb:2011_Middle_School_Youth_Risk_Behavior_Survey rdfs:label """2011 Middle School Youth Risk Behavior Survey"""@en ;
	rdf:type dcterms:source ;
	mhdb:hasAbbreviation mhdb:YRBS-MS ;
	rdfs:comment """The YRBS-MS is a 45-item self-report questionnaire developed by the Center for Disease Control and Prevention (CDC), used to measure risky behavior in teens and young adults. The focus of the YRBS is to determine incidence and prevalence of specific behaviors in six areas that contribute to leading causes of morbidity and mortality in adolescents and adults. These six areas include: unintentional and intentional injuries; tobacco use; alcohol and other drug use; sexual behaviors that contribute to unintended pregnancy and STD; dietary behaviors that result in disease; and physical inactivity. Behaviors are rated on a multiple-choice response format."""@en ;
	mhdb:hasReferenceType disco:Questionnaire ;
	mhdb:usedByStudyOrClinic mhdb:Nathan_Kline_Institute ;
	mhdb:isAboutDomain mhdb:unintentional_and_intentional_injuries ;
	mhdb:isAboutDomain mhdb:depression ;
	mhdb:isAboutDomain mhdb:impulsivity ;
	mhdb:isAboutDomain mhdb:alerting_attention_Alerting_involves_a_change_in_mental_state_as_well_as_in_physiological_state_and_prepares_the_organism_for_fast_reactions_orienting_attention ;
	mhdb:isAboutDomain mhdb:substance_use ;
	mhdb:isAboutDomain mhdb:eating ;
	mhdb:isAboutDomain mhdb:risk_taking ;
	mhdb:isAboutDomain mhdb:mood ;
	mhdb:isForInformant mhdb:self-report ;
	mhdb:isForAgeGroup mhdb:children ;
	mhdb:isForAgeGroup mhdb:adolescents ;
	dcterms:isReferencedBy mhdb:Larsen_RJ_Diener_E_Emmons_RA_1986_Affect_intensity_and_reactions_to_daily_life_events_Journal_of_Personality_and_Social_Psychology_51_803814 .

mhdb:2011_High_School_Youth_Risk_Behavior_Survey rdfs:label """2011 High School Youth Risk Behavior Survey"""@en ;
	rdf:type dcterms:source ;
	mhdb:hasAbbreviation mhdb:YRBS-HS ;
	rdfs:comment """The YRBS-HS is a 79-item self-report questionnaire developed by the Center for Disease Control and Prevention (CDC), used to measure risky behavior in teens and young adults. The focus of the YRBS is to determine incidence and prevalence of specific behaviors in six areas that contribute to leading causes of morbidity and mortality in adolescents and adults. These six areas include: unintentional and intentional injuries; tobacco use; alcohol and other drug use; sexual behaviors that contribute to unintended pregnancy and STD; dietary behaviors that result in disease; and physical inactivity. Behaviors are rated on a multiple-choice response format."""@en ;
	mhdb:hasReferenceType disco:Questionnaire ;
	mhdb:usedByStudyOrClinic mhdb:Nathan_Kline_Institute ;
	mhdb:isAboutDomain mhdb:unintentional_and_intentional_injuries ;
	mhdb:isAboutDomain mhdb:depression ;
	mhdb:isAboutDomain mhdb:impulsivity ;
	mhdb:isAboutDomain mhdb:alerting_attention_Alerting_involves_a_change_in_mental_state_as_well_as_in_physiological_state_and_prepares_the_organism_for_fast_reactions_orienting_attention ;
	mhdb:isAboutDomain mhdb:eating ;
	mhdb:isAboutDomain mhdb:risk_taking ;
	mhdb:isAboutDomain mhdb:mood ;
	mhdb:isForInformant mhdb:self-report ;
	mhdb:isForAgeGroup mhdb:adolescents ;
	dcterms:isReferencedBy mhdb:Methodology_of_the_Youth_Risk_Behavior_Surveillance_System_MMWR_200453RR-12113 .

mhdb:UPPS-P_Impulsive_Behavior_Scale rdfs:label """UPPS-P Impulsive Behavior Scale"""@en ;
	rdf:type dcterms:source ;
	mhdb:hasAbbreviation mhdb:UPPS-P ;
	rdfs:comment """The UPPS-P is a 59-item self-report that assesses five subscales (urgency, premeditation, perseverance, sensation seeking, and positive urgency) that are used to measure five distinct dimensions of impulse behavior in adolescents and adults (ages 12 and older). It is designed to measure impulsivity across dimensions of the Four Factor Model of personality: Premeditation (lack of), Urgency, Sensation Seeking, Perseverance (lack of).  The Scale is not considered a measure of trait impulsivity, rather, the scales reflect distinct personality traits that lead to impulsive-type behavior. Participants are asked to consider acts/incidents during the last 6 months when rating their behavior and attitudes on a 4-point scale, in which 1-Agree strongly, 2-Agree some, 3-Disagree some, 4-Disagree strongly."""@en ;
	mhdb:hasReferenceType disco:Questionnaire ;
	mhdb:usedByStudyOrClinic mhdb:Nathan_Kline_Institute ;
	mhdb:isAboutDomain mhdb:impulsivity ;
	mhdb:isAboutDomain mhdb:alerting_attention_Alerting_involves_a_change_in_mental_state_as_well_as_in_physiological_state_and_prepares_the_organism_for_fast_reactions_orienting_attention ;
	mhdb:isAboutDomain mhdb:perseverance ;
	mhdb:isAboutDomain mhdb:urgency ;
	mhdb:isAboutDomain mhdb:premeditation ;
	mhdb:isAboutDomain mhdb:sensation_seeking ;
	mhdb:isAboutDomain mhdb:risk_taking ;
	mhdb:isForInformant mhdb:self-report ;
	mhdb:isForAgeGroup mhdb:adults ;
	dcterms:isReferencedBy mhdb:Whiteside_S_P_and_D_R_Lynam_2001_The_Five_Factor_Model_and_impulsivity_using_a_structural_model_of_personality_to_understand_impulsivity_Personality_and_Individual_Differences_304_669-689 ;
	dcterms:isReferencedBy mhdb:Whiteside_SP_Lynam_DR_Miller_JD_Reynolds_SK_2005_Validation_of_the_UPPS_impulsive_behaviour_scale_a_four-factor_model_of_impulsivity_European_Journal_of_Personality_19559-574 .

mhdb:University_of_California_at_Los_Angeles_Posttraumatic_Stress_Disorder_Reaction_Index_for_DSM-4_child_version-ages_7-12 rdfs:label """University of California at Los Angeles Posttraumatic Stress Disorder Reaction Index for DSM-4 (child version-ages 7-12):"""@en ;
	rdf:type dcterms:source ;
	rdfs:comment """The UCLA-Youth PTSD index for DSM-IV is a 48-item self report used to screen both for exposure to traumatic events and for all DSM-IV PTSD symptoms in school age children and adolescents (ages 7-12) who report traumatic stress experiences. These instruments are meant to serve as brief screening tools to provide information regarding trauma exposure and PTSD symptoms."""@en ;
	mhdb:hasReferenceType disco:Questionnaire ;
	mhdb:usedByStudyOrClinic mhdb:Nathan_Kline_Institute ;
	mhdb:isAboutDomain mhdb:trauma ;
	mhdb:isForInformant mhdb:self-report ;
	dcterms:isReferencedBy mhdb:Pynoos_Rodriguez_Steinberg_Stuber__FrederickC_1998_UCLA_PTSD_Index_for_DSM-IV_Unpublished_Manual .

mhdb:University_of_California_at_Los_Angeles_Posttraumatic_Stress_Disorder_Reaction_Index_for_DSM-4_Parent_version rdfs:label """University of California at Los Angeles Posttraumatic Stress Disorder Reaction Index for DSM-4 (Parent version):"""@en ;
	rdf:type dcterms:source ;
	rdfs:comment """The UCLA-Parent PTSD index for DSM-IV is a 48-item parent report used to screen both for exposure to traumatic events and for all DSM-IV PTSD symptoms in school age children and adolescents (ages 7-12) who report traumatic stress experiences. These instruments are meant to serve as brief screening tools to provide information regarding trauma exposure and PTSD symptoms."""@en ;
	mhdb:hasReferenceType disco:Questionnaire ;
	mhdb:usedByStudyOrClinic mhdb:Nathan_Kline_Institute ;
	mhdb:isAboutDomain mhdb:trauma ;
	mhdb:isForInformant mhdb:parent-report ;
	mhdb:isForAgeGroup mhdb:children ;
	dcterms:isReferencedBy mhdb:Pynoos_Rodriguez_Steinberg_Stuber__FrederickC_1998_UCLA_PTSD_Index_for_DSM-IV_Unpublished_Manual .

mhdb:Trauma_Symptom_Checklist_for_Children rdfs:label """Trauma Symptom Checklist for Children"""@en ;
	rdf:type dcterms:source ;
	mhdb:hasAbbreviation mhdb:TSC-C ;
	rdfs:comment """The TSC-C is a 54-item self-report inventory assessing posttraumatic stress in children (ages 8 -17) who have experienced traumatic events such as physical or sexual abuse, major loss, natural disaster, or violence. The following clinical scales are assessed: Anxiety, Depression, Anger, Posttraumatic Stress, Dissociation, and Sexual Concerns. Child participants are asked to rate the frequency of certain thoughts and behaviors on a 4-point scale: 0-Never 1-Sometimes, 2-Lots of the time, 3-Almost all the time."""@en ;
	mhdb:hasReferenceType disco:Questionnaire ;
	mhdb:usedByStudyOrClinic mhdb:Nathan_Kline_Institute ;
	mhdb:isAboutDomain mhdb:trauma ;
	mhdb:isForInformant mhdb:self-report ;
	mhdb:isForAgeGroup mhdb:children ;
	dcterms:isReferencedBy mhdb:Briere_J_1996_Trauma_Symptom_Checklist_for_Children_TSCC_Professional_Manual_Odessa_FL_Psychological_Assessment_Resources .

mhdb:Social_Networking_Questionnaire rdfs:label """Social Networking Questionnaire"""@en ;
	rdf:type dcterms:source ;
	rdfs:comment """The Social Networking Questionnaire assesses social interactions and supports."""@en ;
	mhdb:hasReferenceType disco:Questionnaire ;
	mhdb:usedByStudyOrClinic mhdb:Nathan_Kline_Institute ;
	mhdb:isAboutDomain mhdb:social_interaction ;
	mhdb:isForInformant mhdb:self-report ;
	mhdb:isForAgeGroup mhdb:adults ;
	dcterms:isReferencedBy mhdb:Adapted_from_Holtzman_et_al_2004_Social_Network_Characteristics_and_Cognition_in_Middle-Aged_and_Older_Adults_JOG_Psych_Sci_596_278-284 .

mhdb:Nathan_Kline_Institute_Satisfaction_Survey-Child rdfs:label """Nathan Kline Institute Satisfaction Survey-Child"""@en ;
	rdf:type dcterms:source ;
	mhdb:hasReferenceType disco:Questionnaire ;
	mhdb:usedByStudyOrClinic mhdb:Nathan_Kline_Institute .

mhdb:Nathan_Kline_Institute_Participant_Satisfaction_Survey-Adult rdfs:label """Nathan Kline Institute Participant Satisfaction Survey-Adult"""@en ;
	rdf:type dcterms:source ;
	mhdb:hasReferenceType disco:Questionnaire ;
	mhdb:usedByStudyOrClinic mhdb:Nathan_Kline_Institute ;
	mhdb:isForAgeGroup mhdb:adults .

mhdb:NEO_Five_Factor_Inventory-3 rdfs:label """NEO Five Factor Inventory - 3"""@en ;
	rdf:type dcterms:source ;
	mhdb:hasAbbreviation mhdb:NEO-FFI-3 ;
	rdfs:comment """The NEO-FFI-3 is a 60-item psychological personality inventory that assesses based on the five-factor model: Openness to Experience, Conscientiousness, Extraversion, Agreeableness, and Neuroticism. Participants are asked to select the response that best represents their opinion on a 5-point scale: 0-Strongly Agree, 1-Agree, 2-Neutral, 3-Disagree, 4-Strongly Disagree."""@en ;
	mhdb:hasReferenceType disco:Questionnaire ;
	mhdb:usedByStudyOrClinic mhdb:Nathan_Kline_Institute ;
	mhdb:isAboutDomain mhdb:anxiety ;
	mhdb:isAboutDomain mhdb:personality_traits ;
	mhdb:isForInformant mhdb:self-report ;
	dcterms:isReferencedBy mhdb:Mccrae_R_R__Costa_P_T_February_2004_A_contemplated_revision_of_the_NEO_Five-Factor_Inventory_Personality_and_Individual_Differences_363_587596 .

mhdb:International_Physical_Activity_Questionnaire_Ages_15-69 rdfs:label """International Physical Activity Questionnaire (Ages 15-69)"""@en ;
	rdf:type dcterms:source ;
	mhdb:hasAbbreviation mhdb:IPAQ ;
	rdfs:comment """The purpose of the International Physical Activity Questionnaires (IPAQ) is to provide a set of well-developed instruments that can be used internationally to obtain comparable estimates of physical activity. This questionnaire asks the participant about time spent being physically active in the last 7 days, and includes activities that are done at work, as part of house and yard work, getting from place to place, and in spare time for recreation, exercise, and sport. The participant is asked about time spent in vigorous physical activities (referring to activities that take hard physical effort and make you breathe much harder than normal) and moderate activities (referring to activities that take moderate physical effort and make you breathe somewhat harder than normal). The participant is asked to indicate how many days in the last week were spent in either vigorous or moderate activities as part of each aspect of their lives, and further asked to indicate how much time is spend on those activities each day (in hours and minutes)."""@en ;
	mhdb:hasReferenceType disco:Questionnaire ;
	mhdb:usedByStudyOrClinic mhdb:Nathan_Kline_Institute ;
	mhdb:isForInformant mhdb:self-report ;
	dcterms:isReferencedBy mhdb:Craig_CL_et_al_2003_International_Physical_activity_questionnaire_12-country_reliability_and_validity_Medicine_and_Science_in_Sports__Exercise_358_1381-1395 .

mhdb:Domain-Specific_Risk-Taking_Adult_Scale-Risk_Taking_2006 rdfs:label """Domain-Specific Risk-Taking (Adult) Scale - Risk Taking (2006)"""@en ;
	rdf:type dcterms:source ;
	mhdb:hasAbbreviation mhdb:DOSPERT ;
	rdfs:comment """The DOSPERT is a 90-item self-report that assesses risk taking in five content domains: financial decisions (separately for investing versus gambling), health/safety, recreational, ethical, and social decisions. First, participants rate the likelihood that they would engage in domain-specific risky activities on a 7-point scale: 1-Extremely unlikely, 2-Moderately unlikely, 3-Somewhat unlikely, 4-Not sure, 5-Somewhat likely, 6-Moderately likely, 7-Extremely Likely. Next, participants rate the perceived riskiness of these activities on a 7-point scale: 1-Not at all risky, 2-Sligthly risky, 3-Somewhat risky, 4-Moderately risky, 5-Risky, 6-Very risky, 7-Extremely risky. Finally, participants rate the expected benefits of each activity on a 7-point scale: 1-No benefits at all, 4-Moderate benefits, 7-Great benefits."""@en ;
	mhdb:hasReferenceType disco:Questionnaire ;
	mhdb:usedByStudyOrClinic mhdb:Nathan_Kline_Institute ;
	mhdb:isAboutDomain mhdb:risk_taking ;
	mhdb:isAboutDomain mhdb:impulsivity ;
	mhdb:isForInformant mhdb:self-report ;
	mhdb:isForAgeGroup mhdb:adults ;
	dcterms:isReferencedBy mhdb:Blais_AR__Weber_EU_2006_A_Domain-Specific_Risk-Taking_DOSPERT_scale_for_adult_populations_Judgment_and_Decision_Making_1_33-47 .

mhdb:The_Cognitive_Failures_Questionnaire rdfs:label """The Cognitive Failures Questionnaire"""@en ;
	rdf:type dcterms:source ;
	mhdb:hasAbbreviation mhdb:CFQ ;
	rdfs:comment """The CFQ is a 25-item self-report questionnaire assessing failures in perception, memory, and motor function in the completion of everyday tasks in the past 6 months. Individuals are asked to rate the frequency experiences and behaviors on a 5-point scale: 0-Never, 1-Very rarely, 2-Ocassionally, 3-Quite often, 4-Very often."""@en ;
	mhdb:hasReferenceType disco:Questionnaire ;
	mhdb:usedByStudyOrClinic mhdb:Nathan_Kline_Institute ;
	mhdb:isForInformant mhdb:self-report ;
	mhdb:isForAgeGroup mhdb:adults ;
	mhdb:isForAgeGroup mhdb:adolescents ;
	dcterms:isReferencedBy mhdb:Broadbent_D_E_Cooper_P_F_FitzGerald_P__Parkes_K_R_1982_The_cognitive_failures_questionnaire_CFQ_and_its_correlates_British_Journal_of_Clinical_Psychology_211_1-16 .

mhdb:Three_Factor_Eating_Questionnaire rdfs:label """Three Factor Eating Questionnaire"""@en ;
	rdf:type dcterms:source ;
	mhdb:hasAbbreviation mhdb:TFEQ ;
	rdfs:comment """The TFEQ is a 51-item self-report questionnaire designed for adolescents and adults (ages 12 and up). This assessment is designed to measure 3 dimensions of human eating behavior: cognitive restraint of eating (Factor I - 20 items), disinhibition (Factor II – 16 items), and hunger (Factor III - 15 items). The minimum score for factors I-II-III is therefore 0-0-0, and maximum possible score is 20-16-15. Part I includes items 1-36 and are rated either 1-True or 0-False. Part II includes items 37-51 and is rated on a 4-point scale with the exception of item 50, which is rated on a 6-point scale."""@en ;
	mhdb:hasReferenceType disco:Questionnaire ;
	mhdb:usedByStudyOrClinic mhdb:Nathan_Kline_Institute ;
	mhdb:isAboutDomain mhdb:hunger ;
	mhdb:isAboutDomain mhdb:eating ;
	mhdb:isAboutDomain mhdb:disinhibition ;
	mhdb:isAboutDomain mhdb:cognitive_restraint_of_eating ;
	mhdb:isForInformant mhdb:self-report ;
	mhdb:isForAgeGroup mhdb:adults ;
	dcterms:isReferencedBy mhdb:Stunkard_A_J__Messick_S_1985_The_three-factor_eating_questionnaire_to_measure_dietary_restraint_disinhibition_and_hunger_Journal_of_Psychosomatic_Research_29_7183 .

mhdb:Comprehensive_Addiction_Severity_Index_for_Adolescents rdfs:label """Comprehensive Addiction Severity Index for Adolescents"""@en ;
	rdf:type dcterms:source ;
	mhdb:hasAbbreviation mhdb:CASI-A ;
	mhdb:hasReferenceType disco:Questionnaire ;
	mhdb:usedByStudyOrClinic mhdb:Nathan_Kline_Institute .

mhdb:Adult_Temperament_Questionnaire rdfs:label """Adult Temperament Questionnaire"""@en ;
	rdf:type dcterms:source ;
	mhdb:hasAbbreviation mhdb:ATQ ;
	rdfs:comment """The ATQ short form is a 77-item self-report questionnaire for adults (ages 18 and over) assessing constructs of temperament and personality. The measure includes constructs of effortful control, negative affect, extraversion/surgency, and orienting sensitivity. Participants are asked to rate how well the items describe them on a 7-point scale: 1-extremely untrue, 2-quite untrue, 3-slightly true, 4-neither true or false, 5-slightly true, 6-quite true, 7-extremely true."""@en ;
	mhdb:hasReferenceType disco:Questionnaire ;
	mhdb:usedByStudyOrClinic mhdb:Nathan_Kline_Institute ;
	mhdb:isAboutDomain mhdb:depression ;
	mhdb:isAboutDomain mhdb:impulsivity ;
	mhdb:isAboutDomain mhdb:alerting_attention_Alerting_involves_a_change_in_mental_state_as_well_as_in_physiological_state_and_prepares_the_organism_for_fast_reactions_orienting_attention ;
	mhdb:isAboutDomain mhdb:social_interaction ;
	mhdb:isAboutDomain mhdb:anxiety ;
	mhdb:isAboutDomain mhdb:risk_taking ;
	mhdb:isAboutDomain mhdb:mood ;
	mhdb:isAboutDomain mhdb:hyperactivity ;
	mhdb:isAboutDomain mhdb:attention ;
	mhdb:isAboutDomain mhdb:personality_traits ;
	mhdb:isForInformant mhdb:self-report ;
	mhdb:isForAgeGroup mhdb:adults ;
	dcterms:isReferencedBy mhdb:Evans_DE__Rothbart_MK_2007_Development_of_a_model_for_adult_temperament_Journal_of_Research_in_Personality_41_868-888 .

mhdb:Early_Adolescent_Temperament_Questionnaire-Revised_Parent_Report rdfs:label """Early Adolescent Temperament Questionnaire - Revised Parent Report"""@en ;
	rdf:type dcterms:source ;
	mhdb:hasAbbreviation mhdb:EATQ-R ;
	rdfs:comment """The EATQ-R (Parent Report) is a 62-item assessment of temperament and behavior in children and adolescents (ages 9 to 15 years old). The following scales are included: activation control, affiliation, attention, fear, frustration, high-intensity pleasure, inhibitory control, shyness, and aggression and depressive mood. Parents are asked to rate how true the characteristics and behaviors are of their child on a 5-point scale: 1-Almost always untrue, 2-Usually untrue, 3-Sometimes true, sometimes untrue, 4-Usually true, 5-Almost always true."""@en ;
	mhdb:hasReferenceType disco:Questionnaire ;
	mhdb:usedByStudyOrClinic mhdb:Nathan_Kline_Institute ;
	mhdb:isAboutDomain mhdb:attention ;
	mhdb:isAboutDomain mhdb:activation_control ;
	mhdb:isAboutDomain mhdb:oppositionality ;
	mhdb:isAboutDomain mhdb:affiliation ;
	mhdb:isAboutDomain mhdb:shyness ;
	mhdb:isAboutDomain mhdb:depression ;
	mhdb:isAboutDomain mhdb:high-intensity_pleasure ;
	mhdb:isAboutDomain mhdb:anxiety ;
	mhdb:isAboutDomain mhdb:social_interaction ;
	mhdb:isAboutDomain mhdb:frustration ;
	mhdb:isAboutDomain mhdb:mood ;
	mhdb:isAboutDomain mhdb:hyperactivity ;
	mhdb:isAboutDomain mhdb:inhibitory_control ;
	mhdb:isAboutDomain mhdb:aggression ;
	mhdb:isForInformant mhdb:parent-report ;
	mhdb:isForAgeGroup mhdb:children ;
	dcterms:isReferencedBy mhdb:Ellis_L_K_2002_Individual_differences_and_adolescent_psychological_development_Unpublished_doctoral_dissertation_University_of_Oregon ;
	dcterms:isReferencedBy mhdb:Ellis_L_K__Rothbart_M_K_2001_April_Revision_of_the_Early_Adolescent_Temperament_Questionnaire_Poster_presented_at_the_biennial_meeting_of_the_Society_for_Research_in_Child_Development_Minneapolis_MN ;
	dcterms:isReferencedBy mhdb:Capaldi_D_M__Rothbart_M_K_1992_Development_and_validation_of_an_early_adolescent_temperament_measure_Journal_of_Early_Adolescence_122_153-173 .

mhdb:Older_Adult_Self_Report rdfs:label """Older Adult Self Report"""@en ;
	rdf:type dcterms:source ;
	mhdb:hasAbbreviation mhdb:OASR ;
	rdfs:comment """The OASR is a 127-item self-administered instrument designed for older adults (ages 60-90) that examines diverse aspects of adaptive functioning and problems. Participants are asked to review a list of items that describe people, and select the best answer to describe themselves over the past two months on a 3-point scale: 0-Not true, 1-Somewhat or Sometimes True, 2-Very True or Often True. The questionnaire provides scores for the following syndrome scales: anxious/depressed, worries, somatic complaints, functional impairment, memory/cognition problems, thought problems, and irritable/disinhibited. The questionnaire provides scores for the following DSM-oriented scales: depressive problems, anxiety problems, somatic problems, dementia problems, psychotic problems, and antisocial personality problems. Additionally, the questionnaire asks about their use of tobacco, alcohol, and drugs."""@en ;
	mhdb:hasReferenceType disco:Questionnaire ;
	mhdb:usedByStudyOrClinic mhdb:Nathan_Kline_Institute ;
	mhdb:isAboutDomain mhdb:oppositionality ;
	mhdb:isAboutDomain mhdb:depression ;
	mhdb:isAboutDomain mhdb:cognitive_functioning ;
	mhdb:isAboutDomain mhdb:distractability ;
	mhdb:isAboutDomain mhdb:memorycognition_problems ;
	mhdb:isAboutDomain mhdb:behavior ;
	mhdb:isAboutDomain mhdb:thought_problems ;
	mhdb:isAboutDomain mhdb:atypical_behavior ;
	mhdb:isAboutDomain mhdb:mood ;
	mhdb:isAboutDomain mhdb:somatic_complaints ;
	mhdb:isAboutDomain mhdb:functional_impairment ;
	mhdb:isAboutDomain mhdb:aggression ;
	mhdb:isForInformant mhdb:self-report ;
	mhdb:isForAgeGroup mhdb:adults ;
	dcterms:isReferencedBy mhdb:Achenbach_T_M_Newhouse_PA__Rescorla_L_A_2004_Manual_for_the_ASEBA_Older_Adult_Forms__Profiles_Burlington_VT_University_of_Vermont_Research_Center_for_Children_Youth__Families .

mhdb:Trauma_Symptom_Checklist_for_Adults rdfs:label """Trauma Symptom Checklist for Adults"""@en ;
	rdf:type dcterms:source ;
	mhdb:hasAbbreviation mhdb:TSC-40 ;
	rdfs:comment """The TSC-40 is a 40-item self-report that evaluates symptomology in adults (ages 18 and older) associated with childhood or adult traumatic experiences. The TSC-40 consists of six subscales: Anxiety, Depression, Dissociation, Sexual Abuse Trauma Index (SATI), Sexual Problems, and Sleep Disturbance, and includes a Total Score as well. Each symptom item is rated according to it’s frequency of occurrence over the past two months using a 4-point scale: 0-Never, to 3-Often."""@en ;
	mhdb:hasReferenceType disco:Questionnaire ;
	mhdb:usedByStudyOrClinic mhdb:Nathan_Kline_Institute ;
	mhdb:isAboutDomain mhdb:sleep_disturbances ;
	mhdb:isAboutDomain mhdb:trauma ;
	mhdb:isForInformant mhdb:self-report ;
	mhdb:isForAgeGroup mhdb:adults ;
	dcterms:isReferencedBy mhdb:Briere_J_N__Runtz_M_G_1989_The_Trauma_Symptom_Checklist_TSC-33_early_data_on_a_new_scale_Journal_of_Interpersonal_Violence_4_151-163 ;
	dcterms:isReferencedBy mhdb:Elliot_D_M__Briere_J_1992_Sexual_abuse_trauma_among_professional_women_Validating_the_Trauma_Symptom_Checklist__40_TSC-40_Child_Abuse__Neglect_16_391-398 .

mhdb:Demographics rdfs:label """Demographics"""@en ;
	rdf:type dcterms:source ;
	mhdb:hasReferenceType disco:Questionnaire ;
	mhdb:usedByStudyOrClinic mhdb:Healthy_Brain_Network ;
	mhdb:usedByStudyOrClinic mhdb:Nathan_Kline_Institute .

mhdb:Selective_Mutism_Questionnaire rdfs:label """Selective Mutism Questionnaire"""@en ;
	rdf:type dcterms:source ;
	mhdb:hasAbbreviation mhdb:SMQ ;
	mhdb:hasReferenceType disco:Questionnaire ;
	mhdb:usedByStudyOrClinic mhdb:Child_Mind_Institute .

mhdb:Beck_Anxiety_Inventory rdfs:label """Beck Anxiety Inventory"""@en ;
	rdf:type dcterms:source ;
	mhdb:hasReferenceType disco:Questionnaire ;
	mhdb:usedByStudyOrClinic mhdb:Child_Mind_Institute .

mhdb:Social_Responsiveness_Scale-2_Pre-School rdfs:label """Social Responsiveness Scale-2 Pre-School"""@en ;
	rdf:type dcterms:source ;
	mhdb:hasAbbreviation mhdb:SRS-P ;
	mhdb:hasReferenceType disco:Questionnaire ;
	mhdb:usedByStudyOrClinic mhdb:Healthy_Brain_Network .

mhdb:Inventory_of_Callous_and_Unemotional_Traits___Youth_Self_Report rdfs:label """Inventory of Callous and Unemotional Traits  – Youth Self Report"""@en ;
	rdf:type dcterms:source ;
	mhdb:hasAbbreviation mhdb:ICU-SR ;
	rdfs:comment """The Inventory of Callous-Unemotional Traits (ICU) is a 24-item questionnaire designed to provide a comprehensive assessment of callous and unemotional traits.  These traits have proven to be important for designating a distinct subgroup group of antisocial and aggressive youth. The ICU has three subscales:  Callousness, Uncaring, and Unemotional. Adolescent participants are asked to indicate how well each statement describes them on a 4-point scale: 0-Not true at all, 1-Somewhat true, 2-Very true, 3-Definitely true."""@en ;
	mhdb:takesMinutesToComplete "10-15"^^xsd:string ;
	mhdb:hasReferenceType disco:Questionnaire ;
	mhdb:usedByStudyOrClinic mhdb:Healthy_Brain_Network ;
	mhdb:usedByStudyOrClinic mhdb:Nathan_Kline_Institute ;
	mhdb:isAboutDomain mhdb:personality_traits ;
	mhdb:isForInformant mhdb:self-report ;
	dcterms:isReferencedBy mhdb:Essau_CA_Sasagawa_S__Frick_PJ_2006_Callous-unemotional_traits_in_a_community_sample_of_adolescents_Assessment_132_454-469 .

mhdb:Child_Behavior_Checklist_for_Ages_6-18-Parent rdfs:label """Child Behavior Checklist for Ages 6-18 - Parent"""@en ;
	rdf:type dcterms:source ;
	rdfs:comment """The CBCL is a 113-item informant-report questionnaire assessing behavioral competency and behavioral problems in children (ages 6 – 18) within the past six months. The following syndrome scales are assessed: anxious/depressed, withdrawn/depressed, somatic complains, social problems, thought problems, rule-breaking behavior, and aggressive behavior. The following DSM-oriented scales are assessed: affective problems, anxiety problems, somatic problems, attention deficit/hyperactivity problems, oppositional defiant problems, and conduct problems. Additionally, there are 20 social competency items used to obtain parents’ reports of the amount and quality of their child’s participation in sports, hobbies, games, activities, organizations, jobs and chores, friendships, how well the child gets along with others and plays and works by him/herself, and school functioning. Behaviors are rated on a 3-point scale: 0-Not true (as far as you know), 1-Somewhat or sometimes true, 2-Very true or often true."""@en ;
	mhdb:hasReferenceType disco:Questionnaire ;
	mhdb:usedByStudyOrClinic mhdb:Nathan_Kline_Institute ;
	mhdb:isForInformant mhdb:parent-report ;
	dcterms:isReferencedBy mhdb:Achenbach_T_M_1991_Integrative_Guide_to_the_1991_CBCL4-18_YSR_and_TRF_Profiles_Burlington_VT_University_of_Vermont_Department_of_Psychology .

mhdb:Pediatric_Symptom_Checklist_Youth_Report rdfs:label """Pediatric Symptom Checklist Youth Report"""@en ;
	rdf:type dcterms:source ;
	mhdb:hasAbbreviation mhdb:Y-PSC .

mhdb:Community_Assessment_of_Psychotic_Experiences_CAPE-42 rdfs:label """Community Assessment of Psychotic Experiences (CAPE-42)"""@en ;
	rdf:type dcterms:source .

mhdb:The_CRAFFT_Screening_Interview rdfs:label """The CRAFFT Screening Interview"""@en ;
	rdf:type dcterms:source .

mhdb:Patient_Health_Questionnaire_Modified_for_Teens rdfs:label """Patient Health Questionnaire Modified for Teens"""@en ;
	rdf:type dcterms:source ;
	mhdb:hasAbbreviation mhdb:PHQ-9_Modified .

mhdb:Child_Behaviour_Checklist_Ages_6-17_Parent_Report_Form rdfs:label """Child Behaviour Checklist (Ages 6-17) Parent Report Form"""@en ;
	rdf:type dcterms:source ;
	mhdb:hasAbbreviation mhdb:CBCL_Parent_Report_Form_Ages_6-17 ;
	mhdb:isForInformant mhdb:parent-report .

mhdb:Positive_and_Negative_Affect_Schedule rdfs:label """Positive and Negative Affect Schedule"""@en ;
	rdf:type dcterms:source ;
	mhdb:hasAbbreviation mhdb:PANAS .

mhdb:Childhood_Traumatic_Events_Scale rdfs:label """Childhood Traumatic Events Scale"""@en ;
	rdf:type dcterms:source ;
	mhdb:hasAbbreviation mhdb:CTQ .

mhdb:Recent_Traumatic_Events_Scale rdfs:label """Recent Traumatic Events Scale"""@en ;
	rdf:type dcterms:source ;
	mhdb:hasAbbreviation mhdb:RTES .

mhdb:httpswwwnaturecomarticlessrep13865 rdfs:label """<https://www.nature.com/articles/srep13865>"""@en ;
	rdf:type dcterms:source ;
	fabio:hasPubMedId mhdb:26353920 .

mhdb:httpsieeexploreieeeorgdocument8438678 rdfs:label """<https://ieeexplore.ieee.org/document/8438678>"""@en ;
	rdf:type dcterms:source .

mhdb:httpswwwncbinlmnihgovpubmedtermmindlight rdfs:label """<https://www.ncbi.nlm.nih.gov/pubmed/?term=mindlight>"""@en ;
	rdf:type dcterms:source .

mhdb:httpswwwncbinlmnihgovpmcarticlesPMC3983066 rdfs:label """<https://www.ncbi.nlm.nih.gov/pmc/articles/PMC3983066/>"""@en ;
	rdf:type dcterms:source ;
	fabio:hasPubMedId mhdb:24005416 .

mhdb:httpwwwcellcomneuronfulltextS0896-62731400954-4_returnURLhttp3A2F2Flinkinghubelseviercom2Fretrieve2Fpii2FS08966273140095443Fshowall3Dtrue rdfs:label """<http://www.cell.com/neuron/fulltext/S0896-6273(14)00954-4?_returnURL=http%3A%2F%2Flinkinghub.elsevier.com%2Fretrieve%2Fpii%2FS0896627314009544%3Fshowall%3Dtrue>"""@en ;
	rdf:type dcterms:source ;
	fabio:hasPubMedId mhdb:25467987 .

mhdb:httpwwwjaacapcomarticleS0890-85671631262-Xabstract rdfs:label """<http://www.jaacap.com/article/S0890-8567(16)31262-X/abstract>"""@en ;
	rdf:type dcterms:source .

mhdb:httpspeerjcomarticles38 rdfs:label """<https://peerj.com/articles/38/>"""@en ;
	rdf:type dcterms:source ;
	fabio:hasPubMedId mhdb:23638374 .

mhdb:httpsstatic1squarespacecomstatic540e15d2e4b0271ac53fa946t540e2d66e4b0424a81411d241410215270990hedmanDissertationpdf rdfs:label """<https://static1.squarespace.com/static/540e15d2e4b0271ac53fa946/t/540e2d66e4b0424a81411d24/1410215270990/hedmanDissertation.pdf>"""@en ;
	rdf:type dcterms:source .

mhdb:httpeduakcjaeufilespdf137pdf rdfs:label """<http://eduakcja.eu/files/pdf/137.pdf>"""@en ;
	rdf:type dcterms:source .

mhdb:httpswwwnaturecomarticlessrep31107 rdfs:label """<https://www.nature.com/articles/srep31107>"""@en ;
	rdf:type dcterms:source ;
	fabio:hasPubMedId mhdb:27553971 .

mhdb:httpstmsciencemagorgcontent8366366ra165 rdfs:label """<http://stm.sciencemag.org/content/8/366/366ra165>"""@en ;
	rdf:type dcterms:source ;
	fabio:hasPubMedId mhdb:27881826 .

mhdb:httpdlacmorgcitationcfmid2971344 rdfs:label """<http://dl.acm.org/citation.cfm?id=2971344>"""@en ;
	rdf:type dcterms:source .

mhdb:httpswwwncbinlmnihgovpmcarticlesPMC5371917 rdfs:label """<https://www.ncbi.nlm.nih.gov/pmc/articles/PMC5371917/>"""@en ;
	rdf:type dcterms:source ;
	fabio:hasPubMedId mhdb:28264474 .

mhdb:httpswwwresearchgatenetpublication262534139_Automatic_Ingestion_Monitor_A_Novel_Wearable_Device_for_Monitoring_of_Ingestive_Behavior rdfs:label """<https://www.researchgate.net/publication/262534139_Automatic_Ingestion_Monitor_A_Novel_Wearable_Device_for_Monitoring_of_Ingestive_Behavior>"""@en ;
	rdf:type dcterms:source ;
	fabio:hasPubMedId mhdb:24845288 .

mhdb:httpswwwresearchgatenetpublication263311930_SmartStep_A_Fully_Integrated_Low-Power_Insole_Monitorevprf_high rdfs:label """<https://www.researchgate.net/publication/263311930_SmartStep_A_Fully_Integrated_Low-Power_Insole_Monitor?ev=prf_high>"""@en ;
	rdf:type dcterms:source .

mhdb:httpieeexploreieeeorgdocument7039196 rdfs:label """<http://ieeexplore.ieee.org/document/7039196/>"""@en ;
	rdf:type dcterms:source .

mhdb:httpswwwncbinlmnihgovpmcarticlesPMC4775094 rdfs:label """<https://www.ncbi.nlm.nih.gov/pmc/articles/PMC4775094/>"""@en ;
	rdf:type dcterms:source ;
	fabio:hasPubMedId mhdb:4775094 ;
	fabio:hasPubMedId mhdb:25677414 ;
	mhdb:hasReferenceType mhdb:research_paper ;
	mhdb:isAboutDomain mhdb:behavior .

mhdb:httpswwwncbinlmnihgovpmcarticlesPMC3360842 rdfs:label """<https://www.ncbi.nlm.nih.gov/pmc/articles/PMC3360842/>"""@en ;
	rdf:type dcterms:source ;
	fabio:hasPubMedId mhdb:21769705 .

mhdb:httpscapmhbiomedcentralcomarticles101186s13034-015-0076-1 rdfs:label """<https://capmh.biomedcentral.com/articles/10.1186/s13034-015-0076-1>"""@en ;
	rdf:type dcterms:source ;
	fabio:hasPubMedId mhdb:26361496 .

mhdb:httpslinkspringercomchapter101007978-3-319-07227-2_35 rdfs:label """<https://link.springer.com/chapter/10.1007/978-3-319-07227-2_35>"""@en ;
	rdf:type dcterms:source .

mhdb:httpswwwgooglecomsearchqAPreliminaryExaminationofRestingStateFunctionalConnectivityCorrelatesofMotorActivityoqAPreliminaryExaminationofRestingStateFunctionalConnectivityCorrelatesofMotorActivityaqschrome69i57j69i64l3999j0j9sourceidchromeieUTF-8 rdfs:label """<https://www.google.com/search?q=A+Preliminary+Examination+of+Resting+State+Functional+Connectivity+Correlates+of+Motor+Activity&oq=A+Preliminary+Examination+of+Resting+State+Functional+Connectivity+Correlates+of+Motor+Activity&aqs=chrome..69i57j69i64l3.999j0j9&sourceid=chrome&ie=UTF-8>"""@en ;
	rdf:type dcterms:source .

mhdb:httpictuscedupubsAn20innovative20ADHD20assessment20system20using20virtual20realitypdf rdfs:label """<http://ict.usc.edu/pubs/An%20innovative%20ADHD%20assessment%20system%20using%20virtual%20reality.pdf>"""@en ;
	rdf:type dcterms:source .

mhdb:httpswwwncbinlmnihgovpmcarticlesPMC3709861 rdfs:label """<https://www.ncbi.nlm.nih.gov/pmc/articles/PMC3709861/>"""@en ;
	rdf:type dcterms:source ;
	fabio:hasPubMedId mhdb:21454386 .

mhdb:httpwebeecsumichedubavejaPapersPriori_ICASSP_finalpdf rdfs:label """<http://web.eecs.umich.edu/~baveja/Papers/Priori_ICASSP_final.pdf>"""@en ;
	rdf:type dcterms:source ;
	fabio:hasPubMedId mhdb:27630535 .

mhdb:httpswwwncbinlmnihgovpubmed28368138 rdfs:label """<https://www.ncbi.nlm.nih.gov/pubmed/28368138>"""@en ;
	rdf:type dcterms:source ;
	fabio:hasPubMedId mhdb:28368138 .

mhdb:httpswwwresearchgatenetpublication280587665_Daily_electronic_self-monitoring_in_bipolar_disorder_using_smartphones-The_MONARCA_i_trial_A_randomized_placebo-controlled_single-blind_parallel_group_trial rdfs:label """<https://www.researchgate.net/publication/280587665_Daily_electronic_self-monitoring_in_bipolar_disorder_using_smartphones_-_The_MONARCA_i_trial_A_randomized_placebo-controlled_single-blind_parallel_group_trial>"""@en ;
	rdf:type dcterms:source ;
	fabio:hasPubMedId mhdb:26220802 .

mhdb:httpwwwjmirorg20173e62 rdfs:label """<http://www.jmir.org/2017/3/e62/>"""@en ;
	rdf:type dcterms:source ;
	fabio:hasPubMedId mhdb:28258049 .

mhdb:httpptlsysvirginiaeduptlsitesdefaultfilessensus-previewpdf rdfs:label """<http://ptl.sys.virginia.edu/ptl/sites/default/files/sensus-preview.pdf>"""@en ;
	rdf:type dcterms:source .

mhdb:httpwwwcshujiacildaphnapapersKliperEtal_2015pdf rdfs:label """<http://www.cs.huji.ac.il/~daphna/papers/KliperEtal_2015.pdf>"""@en ;
	rdf:type dcterms:source .

mhdb:httpwwwcshujiacildaphnapapersVinokurovEtal_2015pdf rdfs:label """<http://www.cs.huji.ac.il/~daphna/papers/VinokurovEtal_2015.pdf>"""@en ;
	rdf:type dcterms:source .

mhdb:httpswwwncbinlmnihgovpubmed28070783 rdfs:label """<https://www.ncbi.nlm.nih.gov/pubmed/28070783>"""@en ;
	rdf:type dcterms:source ;
	fabio:hasPubMedId mhdb:28070783 ;
	mhdb:hasReferenceType mhdb:research_paper .

mhdb:httpwwwdifculpttjvgamctrocasfilesartigo_w4apdf rdfs:label """<http://www.di.fc.ul.pt/~tjvg/amc/trocas/files/artigo_w4a.pdf>"""@en ;
	rdf:type dcterms:source .

mhdb:httpswwwcenterforautismresearchorgsitesdefaultfilesA20Smartphone20Application-minjpg rdfs:label """<https://www.centerforautismresearch.org/sites/default/files/A%20Smartphone%20Application-min.jpg>"""@en ;
	rdf:type dcterms:source .

mhdb:httppaccscornelledupubsPervasiveHealth_BeWellpdf rdfs:label """<http://pac.cs.cornell.edu/pubs/PervasiveHealth_BeWell.pdf>"""@en ;
	rdf:type dcterms:source .

mhdb:httppaccscornelledupubsubicomp2012_StressSensepdf rdfs:label """<http://pac.cs.cornell.edu/pubs/ubicomp2012_StressSense.pdf>"""@en ;
	rdf:type dcterms:source .

mhdb:httpswwwmc10inccomhubfsClinical20feasibility20of20a20wearable20conformable20sensor20patch20to20monitor20motor20symptoms20in20ParkinsonE28099s20diseasepdft1509466322363 rdfs:label """<https://www.mc10inc.com/hubfs/Clinical%20feasibility%20of%20a%20wearable,%20conformable%20sensor%20patch%20to%20monitor%20motor%20symptoms%20in%20Parkinson%E2%80%99s%20disease.pdf?t=1509466322363>"""@en ;
	rdf:type dcterms:source ;
	fabio:hasPubMedId mhdb:30635244 .

mhdb:httpieeexploreieeeorgdocument8103797reloadtrue rdfs:label """<http://ieeexplore.ieee.org/document/8103797/?reload=true>"""@en ;
	rdf:type dcterms:source .

mhdb:httpwwwvisukyeducheungdocIMFAR2013_posterpdf rdfs:label """<http://www.vis.uky.edu/~cheung/doc/IMFAR2013_poster.pdf>"""@en ;
	rdf:type dcterms:source .

mhdb:httpwwwthelancetcomjournalslanpsyarticlePIIS2215-03661400091-1abstract rdfs:label """<http://www.thelancet.com/journals/lanpsy/article/PIIS2215-0366(14)00091-1/abstract>"""@en ;
	rdf:type dcterms:source ;
	fabio:hasPubMedId mhdb:26359749 ;
	mhdb:hasReferenceType mhdb:research_paper ;
	mhdb:isAboutDomain mhdb:social_interaction ;
	mhdb:isAboutDomain mhdb:sensory_skills .

mhdb:httpslinkspringercomarticle1010072Fs10803-015-2375-z rdfs:label """<https://link.springer.com/article/10.1007%2Fs10803-015-2375-z>"""@en ;
	rdf:type dcterms:source ;
	fabio:hasPubMedId mhdb:25636679 ;
	mhdb:hasReferenceType mhdb:research_paper ;
	mhdb:isAboutDomain mhdb:behavior .

mhdb:httpslinkspringercomarticle1010072Fs10803-015-2374-0 rdfs:label """<https://link.springer.com/article/10.1007%2Fs10803-015-2374-0>"""@en ;
	rdf:type dcterms:source ;
	fabio:hasPubMedId mhdb:25643864 ;
	mhdb:hasReferenceType mhdb:research_paper ;
	mhdb:isAboutDomain mhdb:social_interaction ;
	mhdb:isAboutDomain mhdb:emotion_recognition .

mhdb:httpslinkspringercomarticle1010072Fs10803-015-2377-x rdfs:label """<https://link.springer.com/article/10.1007%2Fs10803-015-2377-x>"""@en ;
	rdf:type dcterms:source ;
	fabio:hasPubMedId mhdb:25643865 ;
	mhdb:hasReferenceType mhdb:research_paper ;
	mhdb:isAboutDomain mhdb:communication .

mhdb:httpslinkspringercomarticle1010072Fs10803-014-2267-7 rdfs:label """<https://link.springer.com/article/10.1007%2Fs10803-014-2267-7>"""@en ;
	rdf:type dcterms:source ;
	fabio:hasPubMedId mhdb:25308197 ;
	mhdb:hasReferenceType mhdb:research_paper ;
	mhdb:isAboutDomain mhdb:social_interaction .

mhdb:httpswwwnaturecomarticles479033aepdfreferrer_access_tokenTovdQ3yrkkPxhlS1q-u2dtRgN0jAjWel9jnR3ZoTv0NRfQuZoINlfS4UdPGInJA0lxpOxbmV32aRjGzS4GI63gD8Rz7x7eTs0ag_3c8eigw_nJCQjnJeai2dSGknBIp2KqMHvLERkvkAxATS21Qzvb58TCC-YF3qXLN0oSmILu83Dtracking_referrerwwwmedscapecom rdfs:label """<https://www.nature.com/articles/479033a.epdf?referrer_access_token=TovdQ3yrkkPxhlS1q-u2dtRgN0jAjWel9jnR3ZoTv0NRfQuZoINlfS4UdPGInJA0lxpOxbmV32aRjGzS4GI63gD8Rz7x7eTs0ag_3c8eigw_nJCQjnJeai2dSGknBIp2KqMHvLERkvkAxATS21Qzvb58TCC-YF3qXLN0oSmILu8%3D&tracking_referrer=www.medscape.com>"""@en ;
	rdf:type dcterms:source .

mhdb:httpswwwnaturecomarticless41598-017-18902-w rdfs:label """<https://www.nature.com/articles/s41598-017-18902-w>"""@en ;
	rdf:type dcterms:source ;
	fabio:hasPubMedId mhdb:29330487 ;
	mhdb:hasReferenceType mhdb:research_paper ;
	mhdb:isAboutDomain mhdb:motor_skills .

mhdb:httpswwwncbinlmnihgovpubmed25474637 rdfs:label """<https://www.ncbi.nlm.nih.gov/pubmed/25474637>"""@en ;
	rdf:type dcterms:source ;
	fabio:hasPubMedId mhdb:25474637 ;
	mhdb:hasReferenceType mhdb:research_paper ;
	mhdb:isAboutDomain mhdb:social_interaction .

mhdb:httpswwwncbinlmnihgovpubmed25385366 rdfs:label """<https://www.ncbi.nlm.nih.gov/pubmed/25385366>"""@en ;
	rdf:type dcterms:source ;
	fabio:hasPubMedId mhdb:25385366 ;
	mhdb:hasReferenceType mhdb:research_paper .

mhdb:httpswwwncbinlmnihgovpmcarticlesPMC4554774 rdfs:label """<https://www.ncbi.nlm.nih.gov/pmc/articles/PMC4554774/>"""@en ;
	rdf:type dcterms:source ;
	fabio:hasPubMedId mhdb:25931290 ;
	mhdb:hasReferenceType mhdb:research_paper ;
	mhdb:isAboutDomain mhdb:sensory_skills .

mhdb:httpsjamanetworkcomjournalsjamafullarticle2275445 rdfs:label """<https://jamanetwork.com/journals/jama/fullarticle/2275445>"""@en ;
	rdf:type dcterms:source ;
	fabio:hasPubMedId mhdb:25898050 ;
	mhdb:hasReferenceType mhdb:research_paper ;
	mhdb:isAboutDomain mhdb:behavior .

mhdb:httpswwwncbinlmnihgovpubmed15360800 rdfs:label """<https://www.ncbi.nlm.nih.gov/pubmed/15360800>"""@en ;
	rdf:type dcterms:source ;
	fabio:hasPubMedId mhdb:15360800 .

mhdb:httpswwwhindawicomjournalsaurt2014935686 rdfs:label """<https://www.hindawi.com/journals/aurt/2014/935686/>"""@en ;
	rdf:type dcterms:source ;
	fabio:hasPubMedId mhdb:25045536 .

mhdb:httpswwwncbinlmnihgovpmcarticlesPMC4526946 rdfs:label """<https://www.ncbi.nlm.nih.gov/pmc/articles/PMC4526946/>"""@en ;
	rdf:type dcterms:source ;
	fabio:hasPubMedId mhdb:26085230 .

mhdb:httpswwwncbinlmnihgovpmcarticlesPMC5046013 rdfs:label """<https://www.ncbi.nlm.nih.gov/pmc/articles/PMC5046013/>"""@en ;
	rdf:type dcterms:source ;
	fabio:hasPubMedId mhdb:27721995 ;
	mhdb:hasReferenceType mhdb:research_paper ;
	mhdb:isAboutDomain mhdb:sensory_skills .

mhdb:httpswwwsciencedirectcomsciencearticlepiiS0747563216303089 rdfs:label """<https://www.sciencedirect.com/science/article/pii/S0747563216303089>"""@en ;
	rdf:type dcterms:source .

mhdb:httpslinkspringercomarticle101007s10209-016-0521-9 rdfs:label """<https://link.springer.com/article/10.1007/s10209-016-0521-9>"""@en ;
	rdf:type dcterms:source .

mhdb:httpwwwtocureautismorgsitesdefaultfilespdfv06i03p128pdf rdfs:label """<http://www.tocureautism.org/sites/default/files/pdf/v06i03p128.pdf>"""@en ;
	rdf:type dcterms:source .

mhdb:httpswwwnaturecomarticlesnature12715 rdfs:label """<https://www.nature.com/articles/nature12715>"""@en ;
	rdf:type dcterms:source ;
	fabio:hasPubMedId mhdb:24196715 .

mhdb:httpswwwnaturecomarticless41598-017-13053-4WTfeed_namesubjects_autism-spectrum-disorders rdfs:label """<https://www.nature.com/articles/s41598-017-13053-4?WT.feed_name=subjects_autism-spectrum-disorders>"""@en ;
	rdf:type dcterms:source ;
	fabio:hasPubMedId mhdb:29051506 ;
	mhdb:hasReferenceType mhdb:research_paper .

mhdb:httpswwwresearchgatenetpublication220947735_DANTE_A_Video_Based_Annotation_Tool_for_Smart_Environments rdfs:label """<https://www.researchgate.net/publication/220947735_DANTE_A_Video_Based_Annotation_Tool_for_Smart_Environments>"""@en ;
	rdf:type dcterms:source .

mhdb:httpswwweralibedacukhandle184214193 rdfs:label """<https://www.era.lib.ed.ac.uk/handle/1842/14193>"""@en ;
	rdf:type dcterms:source .

mhdb:httpethesesbhamacuk69775Mademtzi16PhDpdf rdfs:label """<http://etheses.bham.ac.uk/6977/5/Mademtzi16PhD.pdf>"""@en ;
	rdf:type dcterms:source .

mhdb:httpswwwresearchgatenetpublication266078731_Pictogram_Room_Natural_Interaction_Technologies_to_Aid_in_the_Development_of_Children_with_Autism rdfs:label """<https://www.researchgate.net/publication/266078731_Pictogram_Room_Natural_Interaction_Technologies_to_Aid_in_the_Development_of_Children_with_Autism>"""@en ;
	rdf:type dcterms:source .

mhdb:httpsoroopenacuk438621Stefan_Kreitmayer_PhD_Thesis_2014pdf rdfs:label """<https://oro.open.ac.uk/43862/1/Stefan_Kreitmayer_PhD_Thesis_2014.pdf>"""@en ;
	rdf:type dcterms:source .

mhdb:httpswwwncbinlmnihgovpmcarticlesPMC5591836 rdfs:label """<https://www.ncbi.nlm.nih.gov/pmc/articles/PMC5591836/>"""@en ;
	rdf:type dcterms:source ;
	fabio:hasPubMedId mhdb:28928701 .

mhdb:httpswwwresearchgatenetpublication301798675_Tablet-Based_Activity_Schedule_in_Mainstream_Environment_for_Children_with_Autism_and_Children_with_ID rdfs:label """<https://www.researchgate.net/publication/301798675_Tablet-Based_Activity_Schedule_in_Mainstream_Environment_for_Children_with_Autism_and_Children_with_ID>"""@en ;
	rdf:type dcterms:source .

mhdb:httpswwwncbinlmnihgovpmcarticlesPMC4094670 rdfs:label """<https://www.ncbi.nlm.nih.gov/pmc/articles/PMC4094670/>"""@en ;
	rdf:type dcterms:source ;
	fabio:hasPubMedId mhdb:25018866 .

mhdb:httpswwwresearchgatenetpublication268129484_Seeing_the_Doctor_without_Fear_Systematic_Desensitization_for_Medical_Visits_in_ASD rdfs:label """<https://www.researchgate.net/publication/268129484_Seeing_the_Doctor_without_Fear_Systematic_Desensitization_for_Medical_Visits_in_ASD>"""@en ;
	rdf:type dcterms:source .

mhdb:httpswwwsciencedirectcomsciencearticlepiiS0891422217300562 rdfs:label """<https://www.sciencedirect.com/science/article/pii/S0891422217300562>"""@en ;
	rdf:type dcterms:source ;
	fabio:hasPubMedId mhdb:28327383 .

mhdb:httpswwwfrontiersinorgarticles103389fpsyt201600070full rdfs:label """<https://www.frontiersin.org/articles/10.3389/fpsyt.2016.00070/full>"""@en ;
	rdf:type dcterms:source ;
	fabio:hasPubMedId mhdb:27199777 .

mhdb:httponlinelibrarywileycomdoi101111jcpp12354abstractsystemMessageWileyOnlineLibraryismigratingtoanewplatformpoweredbyAtypon2CtheleadingproviderofscholarlypublishingplatformsThenewWileyOnlineLibrarywillbemigratedovertheweekendofMarch17and18YoushouldnotexperienceanyissuesorlossofaccessduringthistimeFormoreinformation2Cpleasevisitourmigrationpage3Ahttp3A2F2Fwwwwileyactualcom2FWOLMigration2F rdfs:label """<http://onlinelibrary.wiley.com/doi/10.1111/jcpp.12354/abstract?systemMessage=Wiley+Online+Library+is+migrating+to+a+new+platform+powered+by+Atypon%2C+the+leading+provider+of+scholarly+publishing+platforms.+The+new+Wiley+Online+Library+will+be+migrated+over+the+weekend+of+March+17+and+18.You+should+not+experience+any+issues+or+loss+of+access+during+this+time.+For+more+information%2C+please+visit+our+migration+page%3A++http%3A%2F%2Fwww.wileyactual.com%2FWOLMigration%2F>"""@en ;
	rdf:type dcterms:source ;
	fabio:hasPubMedId mhdb:25346345 ;
	mhdb:hasReferenceType mhdb:research_paper ;
	mhdb:isAboutDomain mhdb:communication ;
	mhdb:isAboutDomain mhdb:sensory_skills .

mhdb:httpswwwncbinlmnihgovpubmed21454386 rdfs:label """<https://www.ncbi.nlm.nih.gov/pubmed/21454386>"""@en ;
	rdf:type dcterms:source ;
	fabio:hasPubMedId mhdb:21454386 ;
	mhdb:isAboutDomain mhdb:behavior .

mhdb:httpsonlinelibrarywileycomdoiabs101002aur1667 rdfs:label """<https://onlinelibrary.wiley.com/doi/abs/10.1002/aur.1667>"""@en ;
	rdf:type dcterms:source ;
	fabio:hasPubMedId mhdb:27459107 ;
	mhdb:hasReferenceType mhdb:research_paper ;
	mhdb:isAboutDomain mhdb:communication .

mhdb:httpswwwncbinlmnihgovpubmed23366211 rdfs:label """<https://www.ncbi.nlm.nih.gov/pubmed/23366211>"""@en ;
	rdf:type dcterms:source ;
	fabio:hasPubMedId mhdb:23366211 ;
	mhdb:hasReferenceType mhdb:research_paper ;
	mhdb:isAboutDomain mhdb:behavior .

mhdb:httpswwwsciencedirectcomsciencearticlepiiS0165168417303705 rdfs:label """<https://www.sciencedirect.com/science/article/pii/S0165168417303705>"""@en ;
	rdf:type dcterms:source ;
	mhdb:hasReferenceType mhdb:research_paper ;
	mhdb:isAboutDomain mhdb:motor_skills ;
	mhdb:isAboutDomain mhdb:behavior .

mhdb:httpsfilesericedgovfulltextED577783pdf rdfs:label """<https://files.eric.ed.gov/fulltext/ED577783.pdf>"""@en ;
	rdf:type dcterms:source .

mhdb:httpswwwncbinlmnihgovpmcarticlesPMC3808497 rdfs:label """<https://www.ncbi.nlm.nih.gov/pmc/articles/PMC3808497/>"""@en ;
	rdf:type dcterms:source ;
	fabio:hasPubMedId mhdb:23661504 ;
	mhdb:hasReferenceType mhdb:research_paper ;
	mhdb:isAboutDomain mhdb:communication .

mhdb:httpswwwomicsonlineorgopen-accessmental-imagery-therapy-for-autism-mita--an-early-interventioncomputerized-brain-training-program-for-children-with-asd-2165-7890-1000153pdf rdfs:label """<https://www.omicsonline.org/open-access/mental-imagery-therapy-for-autism-mita--an-early-interventioncomputerized-brain-training-program-for-children-with-asd-2165-7890-1000153.pdf>"""@en ;
	rdf:type dcterms:source .

mhdb:httpsiruiowaeducgiviewcontentcgiarticle1600contextetd rdfs:label """<https://ir.uiowa.edu/cgi/viewcontent.cgi?article=1600&context=etd>"""@en ;
	rdf:type dcterms:source .

mhdb:httpwwwijaictcomissue12ijaict202015041204pdf rdfs:label """<http://www.ijaict.com/issue12/ijaict%202015041204.pdf>"""@en ;
	rdf:type dcterms:source ;
	mhdb:hasReferenceType mhdb:research_paper ;
	mhdb:isAboutDomain mhdb:communication .

mhdb:httpjournalfrontiersinorgarticle103389frobt201700031full rdfs:label """<http://journal.frontiersin.org/article/10.3389/frobt.2017.00031/full>"""@en ;
	rdf:type dcterms:source .

mhdb:httpsgroupscsailmiteduslspublications2017TukaAlHanai_aaai-17pdf rdfs:label """<https://groups.csail.mit.edu/sls/publications/2017/TukaAlHanai_aaai-17.pdf>"""@en ;
	rdf:type dcterms:source ;
	mhdb:isAboutDomain mhdb:behavior .

mhdb:httpsacademicoupcomscanarticle843781623776 rdfs:label """<https://academic.oup.com/scan/article/8/4/378/1623776>"""@en ;
	rdf:type dcterms:source ;
	fabio:hasPubMedId mhdb:22267520 ;
	mhdb:hasReferenceType mhdb:research_paper ;
	mhdb:isAboutDomain mhdb:motor_skills .

mhdb:httpsacademicoupcomcercorarticle26627051754257 rdfs:label """<https://academic.oup.com/cercor/article/26/6/2705/1754257>"""@en ;
	rdf:type dcterms:source ;
	fabio:hasPubMedId mhdb:26048952 ;
	mhdb:hasReferenceType mhdb:research_paper ;
	mhdb:isAboutDomain mhdb:motor_skills .

mhdb:httpciteseerxistpsueduviewdocdownloaddoi1011604562reprep1typepdf rdfs:label """<http://citeseerx.ist.psu.edu/viewdoc/download?doi=10.1.1.60.4562&rep=rep1&type=pdf>"""@en ;
	rdf:type dcterms:source ;
	fabio:hasPubMedId mhdb:16688391 .

mhdb:httpsaffectmediamitedupdfs10Fletcher_etal_TITBpdf rdfs:label """<https://affect.media.mit.edu/pdfs/10.Fletcher_etal_TITB.pdf>"""@en ;
	rdf:type dcterms:source ;
	fabio:hasPubMedId mhdb:20064760 .

mhdb:httpspdfssemanticscholarorge2d8dbf198dc4b3f9028d351785fd5381c8898b8pdf rdfs:label """<https://pdfs.semanticscholar.org/e2d8/dbf198dc4b3f9028d351785fd5381c8898b8.pdf>"""@en ;
	rdf:type dcterms:source .

mhdb:httpciteseerxistpsueduviewdocdownloaddoi1011558492reprep1typepdf rdfs:label """<http://citeseerx.ist.psu.edu/viewdoc/download?doi=10.1.1.55.8492&rep=rep1&type=pdf>"""@en ;
	rdf:type dcterms:source .

mhdb:httpwwwmdpicom2073-431X614 rdfs:label """<http://www.mdpi.com/2073-431X/6/1/4>"""@en ;
	rdf:type dcterms:source .

mhdb:httpwwwpnasorgcontent982011818 rdfs:label """<http://www.pnas.org/content/98/20/11818>"""@en ;
	rdf:type dcterms:source ;
	fabio:hasPubMedId mhdb:11573015 ;
	mhdb:hasReferenceType mhdb:research_paper ;
	mhdb:isAboutDomain mhdb:motivation ;
	mhdb:isAboutDomain mhdb:reward ;
	mhdb:isAboutDomain mhdb:arousal ;
	mhdb:isAboutDomain mhdb:emotion .

mhdb:httpswwwjaacaporgarticleS0890-85670960384-1fulltext rdfs:label """<https://www.jaacap.org/article/S0890-8567(09)60384-1/fulltext>"""@en ;
	rdf:type dcterms:source ;
	fabio:hasPubMedId mhdb:11314561 .

mhdb:httpwwwvokicomsiteapp rdfs:label """<http://www.voki.com/site/app>"""@en ;
	rdf:type dcterms:source .

mhdb:httpswwwncbinlmnihgovpmcarticlesPMC6169783 rdfs:label """<https://www.ncbi.nlm.nih.gov/pmc/articles/PMC6169783/>"""@en ;
	rdf:type dcterms:source ;
	fabio:hasPubMedId mhdb:28661072 .

mhdb:httpslinkspringercomchapter101007978-3-319-32270-4_7 rdfs:label """<https://link.springer.com/chapter/10.1007/978-3-319-32270-4_7>"""@en ;
	rdf:type dcterms:source ;
	mhdb:hasReferenceType mhdb:research_paper ;
	mhdb:isAboutDomain mhdb:motor_skills .

mhdb:httpslinkspringercomchapter101007978-3-319-32270-4_6 rdfs:label """<https://link.springer.com/chapter/10.1007/978-3-319-32270-4_6>"""@en ;
	rdf:type dcterms:source ;
	mhdb:hasReferenceType mhdb:research_paper ;
	mhdb:isAboutDomain mhdb:communication .

mhdb:httpslinkspringercomchapter101007978-3-319-32270-4_8 rdfs:label """<https://link.springer.com/chapter/10.1007/978-3-319-32270-4_8>"""@en ;
	rdf:type dcterms:source ;
	mhdb:hasReferenceType mhdb:research_paper .

mhdb:Achenbach_T_M_1991_Integrative_Guide_to_the_1991_CBCL4-18_YSR_and_TRF_Profiles_Burlington_VT_University_of_Vermont_Department_of_Psychology rdfs:label """Achenbach, T. M. (1991). Integrative Guide to the 1991 CBCL/4-18, YSR, and TRF Profiles. Burlington, VT: University of Vermont, Department of Psychology."""@en ;
	rdf:type dcterms:source .

mhdb:Achenbach_T_Rescorla_L_2003_Manual_for_the_ASEBA_Adult_Forms__Profiles_Burlington_VT_University_of_Vermont_Research_Center_for_Children_Youth_and_Families rdfs:label """Achenbach T., Rescorla, L. (2003). Manual for the ASEBA Adult Forms & Profiles. Burlington, VT: University of Vermont, Research Center for Children, Youth, and Families."""@en ;
	rdf:type dcterms:source .

mhdb:Achenbach_T_M_1991_Manual_for_the_Youth_Self-Report_and_1991_profile_Burlington_VT_University_of_Vermont_Department_of_Psychiatry rdfs:label """Achenbach, T. M. (1991). Manual for the Youth Self-Report and 1991 profile. Burlington, VT: University of Vermont, Department of Psychiatry."""@en ;
	rdf:type dcterms:source .

mhdb:Achenbach_T_M_Newhouse_PA__Rescorla_L_A_2004_Manual_for_the_ASEBA_Older_Adult_Forms__Profiles_Burlington_VT_University_of_Vermont_Research_Center_for_Children_Youth__Families rdfs:label """Achenbach, T. M., Newhouse, P.A., & Rescorla, L. A. (2004). Manual for the ASEBA Older Adult Forms & Profiles. Burlington, VT: University of Vermont, Research Center for Children, Youth, & Families."""@en ;
	rdf:type dcterms:source .

mhdb:Storch_E_A_Larson_M_J_Goodman_W_K_Rasmussen_S_A_Price_L_H__Murphy_T_K_2010 rdfs:label """Storch, E. A., Larson, M. J., Goodman, W. K., Rasmussen, S. A., Price, L. H., & Murphy, T. K. (2010)."""@en ;
	rdf:type dcterms:source ;
	fabio:hasPubMedId mhdb:20471199 .

mhdb:Development_and_Psychometric_Evaluation_of_the_Yale-Brown_Obsessive-Compulsive_ScaleSecond_Edition_Psychological_Assessment_222_223-232 rdfs:label """Development and Psychometric Evaluation of the Yale-Brown Obsessive-Compulsive Scale—Second Edition. Psychological Assessment, 22(2), 223-232."""@en ;
	rdf:type dcterms:source .

mhdb:Birmaher_B_Brent_D_A_Chiappetta_L_Bridge_J_Monga_S__Baugher_M_1999 rdfs:label """Birmaher, B., Brent, D. A., Chiappetta, L., Bridge, J., Monga, S., & Baugher, M. (1999)."""@en ;
	rdf:type dcterms:source ;
	fabio:hasPubMedId mhdb:10517055 .

mhdb:Psychometric_properties_of_the_Screen_for_Child_Anxiety_Related_Emotional_Disorders_SCARED_a_replication_study_Journal_of_the_American_Academy_of_Child_and_Adolescent_Psychiatry_3810_1230-1236 rdfs:label """Psychometric properties of the Screen for Child Anxiety Related Emotional Disorders (SCARED): a replication study. Journal of the American Academy of Child and Adolescent Psychiatry, 38(10), 1230-1236."""@en ;
	rdf:type dcterms:source ;
	fabio:hasPubMedId mhdb:10517055 .

mhdb:Posner_K_Brown_GK_Stanley_B_Brent_DA_Yershova_KV_Oquendo_MA_Currier_GW_Melvin_G_Greenhill_L_Shen_S__Mann_JJ_The_Columbia-Suicide_Severity_Rating_Scale_Initial_Validity_and_Internal_Consistency_Findings_From_Three_Multisite_Studies_With_Adolescents_and_Adults_American_Journal_of_Psychiatry_2011_1681266-1277 rdfs:label """Posner, K., Brown, G.K., Stanley, B., Brent, D.A., Yershova, K.V., Oquendo, M.A., Currier, G.W., Melvin, G., Greenhill, L., Shen, S., & Mann, J.J., The Columbia-Suicide Severity Rating Scale: Initial Validity and Internal Consistency Findings From Three Multisite Studies With Adolescents and Adults American Journal of Psychiatry, 2011; 168:1266-1277."""@en ;
	rdf:type dcterms:source ;
	fabio:hasPubMedId mhdb:22193671 .

mhdb:Kovacs_M_1985_The_Childrens_Depression_Inventory_CDI_Psychopharmacology_Bulletin_214_995-998 rdfs:label """Kovacs, M. (1985). The Children's Depression, Inventory (CDI). Psychopharmacology Bulletin, 21(4), 995-998."""@en ;
	rdf:type dcterms:source .

mhdb:Spielberger_C_D_Gorsuch_RL_and_Lushene_RE_1970_Manual_for_the_State-Trait_Anxiety_Inventory_Palo_Alto_CA_Consulting_Psychologists_Press rdfs:label """Spielberger, C. D., Gorsuch, R.L., and Lushene. R.E. (1970). Manual for the State-Trait Anxiety Inventory. Palo Alto, CA: Consulting Psychologists Press"""@en ;
	rdf:type dcterms:source .

mhdb:Angold_A_Costello_E_J_Messer_S_C_Pickles_A_Winder_F__Silver_D_1995_The_development_of_a_short_questionnaire_for_use_in_epidemiological_studies_of_depression_in_children_and_adolescents_International_Journal_of_Methods_in_Psychiatric_Research_5_237-249 rdfs:label """Angold, A., Costello, E. J., Messer, S. C., Pickles, A., Winder, F., & Silver, D. (1995) The development of a short questionnaire for use in epidemiological studies of depression in children and adolescents. International Journal of Methods in Psychiatric Research, 5, 237 - 249."""@en ;
	rdf:type dcterms:source .

mhdb:Swanson_J_Schuck_S_Mann_M_Carlson_C_Hartman_K_Sergeant_J____McCleary_R_2001_The_SWAN_rating_scale rdfs:label """Swanson, J., Schuck, S., Mann, M., Carlson, C., Hartman, K., Sergeant, J., . . . McCleary, R. (2001). The SWAN rating scale."""@en ;
	rdf:type dcterms:source ;
	fabio:hasPubMedId mhdb:26504617 .

mhdb:Essau_CA_Sasagawa_S__Frick_PJ_2006_Callous-unemotional_traits_in_a_community_sample_of_adolescents_Assessment_132_454-469 rdfs:label """Essau, C.A., Sasagawa, S., & Frick, P.J. (2006). Callous-unemotional traits in a community sample of adolescents. Assessment, 132, 454-469."""@en ;
	rdf:type dcterms:source .

mhdb:Chandler_S_Charman_T_Baird_G_et_al_2007_Validation_of_the_Social_Communication_Questionnaire_in_a_population_cohort_of_children_with_autism_spectrum_disorders_Journal_of_the_American_Academy_of_Child_and_Adolescent_Psychiatry_46_1324_-1332 rdfs:label """Chandler, S., Charman, T., Baird, G., et al (2007). Validation of the Social Communication Questionnaire in a population cohort of children with autism spectrum disorders. Journal of the American Academy of Child and Adolescent Psychiatry, 46, 1324 -1332."""@en ;
	rdf:type dcterms:source .

mhdb:Constantino_JN_Davis_SA_Todd_RD_Schindler_MK_Gross_MM_Brophy_SL_et_al_2003_Validation_of_a_brief_quantitative_measure_of_autistic_traits_comparison_of_the_Social_Responsiveness_Scale_with_the_Autism_Diagnostic_Interview-Revised_Journal_of_Autism_Developmental_Disorders_33_427-433 rdfs:label """Constantino, J.N., Davis, S.A., Todd, R.D., Schindler M.K., Gross, M.M., Brophy, S.L., et al. (2003). Validation of a brief quantitative measure of autistic traits: comparison of the Social Responsiveness Scale with the Autism Diagnostic Interview-Revised. Journal of Autism Developmental Disorders. 33, 427-433."""@en ;
	rdf:type dcterms:source ;
	fabio:hasPubMedId mhdb:12959421 .

mhdb:Bird_H_R_Shaffer_D_Fisher_P__Gould_M_S_1993_The_Columbia_Impairment_Scale_CIS_Pilot_findings_on_a_measure_of_global_impairment_for_children_and_adolescents_International_Journal_of_Methods_in_Psychiatric_Research rdfs:label """Bird, H. R., Shaffer, D., Fisher, P., & Gould, M. S. (1993). The Columbia Impairment Scale (CIS): Pilot findings on a measure of global impairment for children and adolescents. International Journal of Methods in Psychiatric Research."""@en ;
	rdf:type dcterms:source .

mhdb:Gold_Liza_H_DSM-5_and_the_assessment_of_functioning_the_World_Health_Organization_Disability_Assessment_Schedule_20_WHODAS_20_Journal_of_the_American_Academy_of_Psychiatry_and_the_Law_Online_422_2014_173-181 rdfs:label """Gold, Liza H. \'DSM-5 and the assessment of functioning: the World Health Organization Disability Assessment Schedule 2.0 (WHODAS 2.0).\' Journal of the American Academy of Psychiatry and the Law Online 42.2 (2014): 173-181."""@en ;
	rdf:type dcterms:source ;
	fabio:hasPubMedId mhdb:24986344 .

mhdb:Felitti_VJ_Anda_RF_Nordenberg_D_et_al_Relationship_of_childhood_abuse_and_household_dysfunction_to_many_of_the_leading_causes_of_death_in_adults_The_adverse_childhood_experiences_ACE_study_Am_J_Prev_Med_199814245--58_PMID_9635069 rdfs:label """Felitti VJ, Anda RF, Nordenberg D, et al. Relationship of childhood abuse and household dysfunction to many of the leading causes of death in adults. The adverse childhood experiences (ACE) study. Am J Prev Med 1998;14:245--58. PMID: 9635069"""@en ;
	rdf:type dcterms:source ;
	fabio:hasPubMedId mhdb:9635069 .

mhdb:Conners_CK_2001_Conners_Rating_Scales-Revised_North_Tonawanda_NY_Multi-Health_Systems_Inc rdfs:label """Conners, C.K. (2001). Conners’ Rating Scales-Revised. North Tonawanda, NY: Multi-Health Systems, Inc."""@en ;
	rdf:type dcterms:source .

mhdb:Conners_CK_Erhardt_D__Sparrow_E_1999_Conners_Adult_ADHD_Rating_Scales_Toronto_ON_Multi-Health_Systems_Inc rdfs:label """Conners, C.K., Erhardt, D., & Sparrow, E. (1999). Conners’ Adult ADHD Rating Scales. Toronto, ON: Multi-Health Systems, Inc."""@en ;
	rdf:type dcterms:source .

mhdb:Grych_JH_Seid_M___Fincham_FD_1992_Assessing_marital_conflict_from_the_childs_perspective_The_Childrens_Perception_of_Interparental_Conflict_Scale_Child_Development_63_558-572_PMID_1600822 rdfs:label """Grych, J.H., Seid, M. , & Fincham, F.D. (1992). Assessing marital conflict from the child's perspective: The Children's Perception of Interparental Conflict Scale. Child Development, 63, 558-572. PMID: 1600822"""@en ;
	rdf:type dcterms:source ;
	fabio:hasPubMedId mhdb:1600822 .

mhdb:Simons__Gaher_2005_The_distress_tolerance_scale_development_and_validation_of_a_self-report_measure_Motivation_and_Emotion_292_83-102 rdfs:label """Simons & Gaher. (2005) The distress tolerance scale: development and validation of a self-report measure. Motivation and Emotion, 29(2), 83-102."""@en ;
	rdf:type dcterms:source .

mhdb:Hibell_B_Guttormsson_U_Ahlstrom_S_et_al_2012_The_2011_ESPAD_Report_substance_use_among_students_in_36_European_countries_The_Swedish_Council_for_Information_on_Alcohol_and_Other_Drugs_CAN_Stockholm_Sweden rdfs:label """Hibell, B., Guttormsson, U., Ahlstrom, S., et al. (2012), The 2011 ESPAD Report: substance use among students in 36 European countries. The Swedish Council for Information on Alcohol and Other Drugs (CAN), Stockholm, Sweden."""@en ;
	rdf:type dcterms:source .

mhdb:Heatherton_TF_Kozlowski_LT_Frecker_RC_Fagerstrom_KO_1991_The_Fagerstrom_Test_for_Nicotine_Dependence_A_revision_of_the_Fagerstrom_Tolerance_Questionnaire_British_Journal_of_Addictions_86_1119-27 rdfs:label """Heatherton TF, Kozlowski LT, Frecker RC, Fagerstrom KO (1991). The Fagerstrom Test for Nicotine Dependence: A revision of the Fagerstrom Tolerance Questionnaire. British Journal of Addictions, 86, 1119-27."""@en ;
	rdf:type dcterms:source ;
	fabio:hasPubMedId mhdb:1932883 .

mhdb:Prokhorov_AV_Pallonen_UE_Fava_JL_Ding_L_Niaura_R_1996_Measuring_nicotine_dependence_among_high-risk_adolescent_smokers_Addict_Behav_21_1_117-127 rdfs:label """Prokhorov, A.V., Pallonen, U.E., Fava, J.L., Ding, L., Niaura, R. (1996). Measuring nicotine dependence among high-risk adolescent smokers. Addict Behav, 21 (1), 117-127."""@en ;
	rdf:type dcterms:source ;
	fabio:hasPubMedId mhdb:8729713 .

mhdb:Young_K_S_1998_Internet_addiction_The_emergence_of_a_new_clinical_disorder_CyberPsychology_and_Behavior_13_237-244 rdfs:label """Young, K. S. (1998) Internet addiction: The emergence of a new clinical disorder. CyberPsychology and Behavior, 1(3), 237-244."""@en ;
	rdf:type dcterms:source .

mhdb:httpwwwdrugabusegovsitesdefaultfilespdfnmassistpdf rdfs:label """<http://www.drugabuse.gov/sites/default/files/pdf/nmassist.pdf.>"""@en ;
	rdf:type dcterms:source .

mhdb:Sandler_IN_Wolchik_SA_Braver_SL__Fogas_B_1991_Stability_and_quality_of_life_events_and_psychological_symptomatology_in_children_of_divorce_American_Journal_of_Community_Psychology_194_501-520 rdfs:label """Sandler, I.N., Wolchik, S.A., Braver, S.L. & Fogas, B. (1991). Stability and quality of life events and psychological symptomatology in children of divorce. American Journal of Community Psychology, 19(4), 501-520."""@en ;
	rdf:type dcterms:source ;
	fabio:hasPubMedId mhdb:1755433 .

mhdb:Kowalski_KC_Crocker_PR_Faulkner_RA_2007_Validation_of_the_Physical_Activity_Questionnaire_for_Older_Children_Pediatric_Exercise_Science_9_174-186 rdfs:label """Kowalski, K.C., Crocker, P.R., Faulkner, R.A. (2007). Validation of the Physical Activity Questionnaire for Older Children. Pediatric Exercise Science, 9, 174-186"""@en ;
	rdf:type dcterms:source .

mhdb:Janz_K_F_Lutuchy_EM_Wenthe_P__Levy_SM_2008_Measuring_activity_in_children_and_adolescents_using_self-report_PAC-Q_and_PAQ-A_Medicine__Science_In_Sports__Exercise_404_767-772 rdfs:label """Janz, K. F., Lutuchy, E.M., Wenthe, P. & Levy, S.M. (2008). Measuring activity in children and adolescents using self-report: PAC-Q and PAQ-A. Medicine & Science In Sports & Exercise, 40(4), 767-772."""@en ;
	rdf:type dcterms:source ;
	fabio:hasPubMedId mhdb:18317366 .

mhdb:Petersen_A_Crockett_L_Richards_M__Boxer_A_1988_A_self-report_measure_of_pubertal_status_Reliability_validity_and_initial_norms_Journal_of_Youth_and_Adolescence_172_117-133 rdfs:label """Petersen, A., Crockett, L., Richards, M., & Boxer, A. (1988). \'A self-report measure of pubertal status: Reliability, validity, and initial norms.\' Journal of Youth and Adolescence, 17(2), 117-133."""@en ;
	rdf:type dcterms:source ;
	fabio:hasPubMedId mhdb:24277579 .

mhdb:Abidin_RR_2012_Parenting_stress_index_fourth_edition_PSI-4_Lutz_FL_Psychological_Assessment_Resources rdfs:label """Abidin, R.R. (2012). Parenting stress index, fourth edition (PSI-4). Lutz, FL: Psychological Assessment Resources."""@en ;
	rdf:type dcterms:source .

mhdb:Gearhardt_AN_Corbin_WR__Brownell_KD_2009_Preliminary_validation_of_the_Yale_Food_Addiction_Scale_Appetite_52_430-436 rdfs:label """Gearhardt, A.N., Corbin, W.R., & Brownell, K.D. (2009). Preliminary validation of the Yale Food Addiction Scale. Appetite, 52, 430-436."""@en ;
	rdf:type dcterms:source ;
	fabio:hasPubMedId mhdb:19121351 .

mhdb:March_J_S_1998_Multi-dimensional_anxiety_scale_for_children_North_Tonawanda_NY_Multi_Health_Systems rdfs:label """March, J. S. (1998). Multi-dimensional anxiety scale for children. North Tonawanda, NY: Multi Health Systems."""@en ;
	rdf:type dcterms:source .

mhdb:Shaffer_David_Gould_MS_Brasic_J_Ambrosini_P_Fisher_Prudence_Bird_Hector_Aluwahlia_S_1983_A_childrens_global_assessment_scale_CGAS_Archives_of_General_Psychiatry_40_122831 rdfs:label """Shaffer, David; Gould, M.S.; Brasic, J.; Ambrosini, P.; Fisher, Prudence; Bird, Hector; Aluwahlia, S. (1983). \'A children's global assessment scale (CGAS)\'. Archives of General Psychiatry. 40: 1228–31"""@en ;
	rdf:type dcterms:source .

mhdb:Block_G_Hartman_AM_Dresser_CM_Carroll_MD_Gannon_J_Gardner_L_A_data-based_approach_to_diet_questionnaire_design_and_testing_Am_J_Epidemiol_1986_124453-469 rdfs:label """Block G, Hartman AM, Dresser CM, Carroll MD, Gannon J, Gardner L. A data-based approach to diet questionnaire design and testing. Am J Epidemiol 1986; 124:453-469."""@en ;
	rdf:type dcterms:source ;
	fabio:hasPubMedId mhdb:3740045 .

mhdb:Dunn_L_M__Dunn_D_M_2007_PPVT-4_Peabody_picture_vocabulary_test_Pearson_Assessments rdfs:label """Dunn, L. M., & Dunn, D. M. (2007). PPVT-4: Peabody picture vocabulary test. Pearson Assessments."""@en ;
	rdf:type dcterms:source .

mhdb:Hemphill_S_A_Heerde_J_A_Herrenkohl_T_I_Patton_G_C_Toumbourou_J_W__Catalano_R_F_2011_Risk_and_protective_factors_for_adolescent_substance_use_in_Washington_State_the_United_States_and_Victoria_Australia_A_longitudinal_study_Journal_of_Adolescent_Health_493_312-320 rdfs:label """Hemphill, S. A., Heerde, J. A., Herrenkohl, T. I., Patton, G. C., Toumbourou, J. W., & Catalano, R. F. (2011). Risk and protective factors for adolescent substance use in Washington State, the United States and Victoria, Australia: A longitudinal study. Journal of Adolescent Health, 49(3), 312-320."""@en ;
	rdf:type dcterms:source ;
	fabio:hasPubMedId mhdb:21856525 .

mhdb:Beyers_J_M_Toumbourou_J_W_Catalano_R_F_Arthur_M_W__Hawkins_J_D_2004_A_cross-national_comparison_of_risk_and_protective_factors_for_adolescent_substance_use_the_United_States_and_Australia_Journal_of_Adolescent_Health_351_3-16 rdfs:label """Beyers, J. M., Toumbourou, J. W., Catalano, R. F., Arthur, M. W., & Hawkins, J. D. (2004). A cross-national comparison of risk and protective factors for adolescent substance use: the United States and Australia. Journal of Adolescent Health, 35(1), 3-16."""@en ;
	rdf:type dcterms:source ;
	fabio:hasPubMedId mhdb:15193569 .

mhdb:Mujahid_M_S_Diez_Roux_A_V_Morenoff_J_D__Raghunathan_T_2007_Assessing_the_measurement_properties_of_neighborhood_scales_From_psychometrics_to_ecometrics_American_Journal_of_Epidemiology_165_858-867 rdfs:label """Mujahid, M. S., Diez Roux, A. V., Morenoff, J. D., & Raghunathan, T. (2007). Assessing the measurement properties of neighborhood scales: From psychometrics to ecometrics. American Journal of Epidemiology, 165, 858-867."""@en ;
	rdf:type dcterms:source .

mhdb:Lam_K_S_L_and_M_G_Aman_2007_The_Repetitive_Behavior_Scale-Revised_independent_validation_in_individuals_with_autism_spectrum_disorders_Journal_of_Autism_and_Developmental_Disorders_375_855-866 rdfs:label """Lam, K. S. L. and M. G. Aman (2007). The Repetitive Behavior Scale-Revised: independent validation in individuals with autism spectrum disorders. Journal of Autism and Developmental Disorders, 37(5): 855-866."""@en ;
	rdf:type dcterms:source ;
	fabio:hasPubMedId mhdb:17048092 .

mhdb:Bruni_O_Ottavianio_S_Guidetti_V_Romoli_M_Innocenzi_M_Cortesi_F__Giannotti_F_1996_The_Sleep_Disturbance_Scale_for_Children_SDSC_Construction_and_validation_of_an_instrument_to_evaluate_sleep_disturbances_in_childhood_and_adolescence_J_Sleep_Rrs_5_251-261 rdfs:label """Bruni, O., Ottavianio, S., Guidetti, V., Romoli, M., Innocenzi, M., Cortesi, F., & Giannotti, F. (1996). The Sleep Disturbance Scale for Children (SDSC): Construction and validation of an instrument to evaluate sleep disturbances in childhood and adolescence. J. Sleep Rrs, 5, 251-261."""@en ;
	rdf:type dcterms:source ;
	fabio:hasPubMedId mhdb:9065877 .

mhdb:Liddle_Elizabeth_B_Martin_J_Batty_and_Robert_Goodman_The_social_aptitudes_scale_an_initial_validation_Social_psychiatry_and_psychiatric_epidemiology_446_2009_508-513 rdfs:label """Liddle, Elizabeth B., Martin J. Batty, and Robert Goodman. \'The social aptitudes scale: an initial validation.\' Social psychiatry and psychiatric epidemiology 44.6 (2009): 508-513."""@en ;
	rdf:type dcterms:source ;
	fabio:hasPubMedId mhdb:18979221 .

mhdb:Goodman_R_1997_The_Strengths_and_Difficulties_Questionnaire_A_Research_Note_Journal_of_Child_Psychology_and_Psychiatry38_581-586 rdfs:label """Goodman, R. 1997. The Strengths and Difficulties Questionnaire: A Research Note. Journal of Child Psychology and Psychiatry,38, 581-586."""@en ;
	rdf:type dcterms:source ;
	fabio:hasPubMedId mhdb:9255702 .

mhdb:Goodman_R_1999_The_extended_version_of_the_Strengths_and_Difficulties_Questionnaire_as_a_guide_to_child_psychiatric_caseness_and_consequent_burden_Journal_of_Child_Psychology_and_Psychiatry_40_791-801 rdfs:label """Goodman, R. 1999. The extended version of the Strengths and Difficulties Questionnaire as a guide to child psychiatric caseness and consequent burden. Journal of Child Psychology and Psychiatry, 40, 791-801."""@en ;
	rdf:type dcterms:source ;
	fabio:hasPubMedId mhdb:10433412 .

mhdb:Goodman_et_al_2010_When_to_use_broader_internalising_and_externalising_subscales_instead_of_the_hypothesised_five_subscales_on_the_Strengths_and_Difficulties_Questionnaire_SDQ_data_from_British_parents_teachers_and_children_Journal_of_Abnormal_Child_Psychology_38_1179-1191 rdfs:label """Goodman et al. 2010. When to use broader internalising and externalising subscales instead of the hypothesised five subscales on the Strengths and Difficulties Questionnaire (SDQ): data from British parents, teachers and children. Journal of Abnormal Child Psychology, 38, 1179-1191."""@en ;
	rdf:type dcterms:source ;
	fabio:hasPubMedId mhdb:20623175 .

mhdb:Leckman_JF_Riddle_MA_Hardin_MT_Ort_SL_Swartz_KL_Stevenson_J_et_al_1989_The_Yale_Global_Tic_Severity_Scale_Initial_testing_of_a_clinician-rated_scale_of_tic_severity_Journal_of_the_American_Academy_of_Child_and_Adolescent_Psychiatry_28_566573 rdfs:label """Leckman J.F., Riddle M.A., Hardin M.T., Ort S.L., Swartz K.L., Stevenson J., et al. (1989). The Yale Global Tic Severity Scale: Initial testing of a clinician-rated scale of tic severity. Journal of the American Academy of Child and Adolescent Psychiatry. 28, 566–573."""@en ;
	rdf:type dcterms:source ;
	fabio:hasPubMedId mhdb:2768151 .

mhdb:Steinberg_A_M_Brymer_M_J_Decker_K_B__Pynoos_R_S_2004_The_University_of_California_at_Los_Angeles_post-traumatic_stress_disorder_reaction_index_Current_psychiatry_reports_62_96-100 rdfs:label """Steinberg, A. M., Brymer, M. J., Decker, K. B., & Pynoos, R. S. (2004). The University of California at Los Angeles post-traumatic stress disorder reaction index. Current psychiatry reports, 6(2), 96-100."""@en ;
	rdf:type dcterms:source ;
	fabio:hasPubMedId mhdb:15038911 .

mhdb:Putnam_S_P__Rothbart_M_K_2006_Development_of_short_and_very_short_forms_of_the_childrens_behavior_questionnaire_Journal_of_Personality_Assessment_871_102-112__Rothbart_M_K_Ahadi_S_A_Hershey_K_L__Fisher_P_2001_Investigations_of_temperament_at_three_to_seven_years_The_childrens_behavior_questionnaire_Child_Development_725_1394-1408 rdfs:label """Putnam, S. P., & Rothbart, M. K. (2006). Development of short and very short forms of the children’s behavior questionnaire. Journal of Personality Assessment, 87(1), 102-112. , Rothbart, M. K., Ahadi, S. A., Hershey, K. L., & Fisher, P. (2001). Investigations of temperament at three to seven years: The children’s behavior questionnaire. Child Development, 72(5), 1394-1408."""@en ;
	rdf:type dcterms:source ;
	fabio:hasPubMedId mhdb:16856791__11699677 .

mhdb:Wardle_J_Guthrie_C_A_Sanderson_S__Rapoport_L_2001_Development_of_the_childrens_eating_behaviour_questionnaire_Journal_of_Child_Psychology_and_Psychiatry_4207_963-970 rdfs:label """Wardle, J., Guthrie, C. A., Sanderson, S., & Rapoport, L. (2001). Development of the children’s eating behaviour questionnaire. Journal of Child Psychology and Psychiatry, 42(07), 963-970."""@en ;
	rdf:type dcterms:source ;
	fabio:hasPubMedId mhdb:11693591 .

mhdb:Mond_J_M_Hay_P_J_Rodgers_B_Owen_C__Beumont_P_J_2004_Validity_of_the_eating_disorder_examination_questionnaire_EDE-Q_in_screening_for_eating_disorders_in_community_samples_Behaviour_Research_and_Therapy_425_551-67_Fairburn_C_G__Cooper_Z_1993_The_Eating_Disorder_Examination_twelfth_edition_In_C_G_Fairburn__G_T_Wilson_eds_Binge_Eating_Nature_Assessment_and_Treatment_pp_317-_360_New_York_Guilford_Press_1993 rdfs:label """Mond, J. M., Hay, P. J., Rodgers, B., Owen, C., & Beumont, P. J. (2004). Validity of the eating disorder examination questionnaire (EDE-Q) in screening for eating disorders in community samples. Behaviour Research and Therapy, 42(5), 551-67. Fairburn C. G., & Cooper, Z. (1993). The Eating Disorder Examination (twelfth edition). In: C. G. Fairburn & G. T. Wilson (eds.). Binge Eating: Nature, Assessment and Treatment. (pp. 317- 360). New York: Guilford Press, 1993."""@en ;
	rdf:type dcterms:source ;
	fabio:hasPubMedId mhdb:15033501 .

mhdb:Davis_M_H_1983_Measuring_individual_differences_in_empathy_Evidence_for_a_multidimensional_approach_Journal_of_Personality_and_Social_Psychology_44_113-126 rdfs:label """Davis, M. H. (1983). Measuring individual differences in empathy: Evidence for a multidimensional approach. Journal of Personality and Social Psychology, 44, 113-126."""@en ;
	rdf:type dcterms:source .

mhdb:Mark_H_Davis_1980_A_multidimensional_approach_to_individual_difference_in_empathy_JSAS_Catalog_of_Selected_Documents_in_Psychology_10_85 rdfs:label """Mark H. Davis, 1980. A multidimensional approach to individual difference in empathy. JSAS Catalog of Selected Documents in Psychology, 10, 85."""@en ;
	rdf:type dcterms:source .

mhdb:Peters_E_R_Joseph_S_A__Garety_P_A_1999_Measurement_of_delusional_ideation_in_the_normal_population_Introducing_the_PDI_peters_et_al_Delusions_inventory_Schizophrenia_Bulletin_253_553-576 rdfs:label """Peters, E. R., Joseph, S. A., & Garety, P. A. (1999). Measurement of delusional ideation in the normal population: Introducing the PDI (peters et al. Delusions inventory). Schizophrenia Bulletin, 25(3), 553-576."""@en ;
	rdf:type dcterms:source ;
	fabio:hasPubMedId mhdb:10478789 .

mhdb:BuysseDJ_ReynoldsCF_MonkTH_BermanSR__KupferDJ_1989_The_Pittsburgh_Sleep_Quality_Index_PSQI_A_new_instrument_for_psychiatric_research_and_practice_Psychiatry_Research_282_193-213 rdfs:label """Buysse,D.J., Reynolds,C.F., Monk,T.H., Berman,S.R., & Kupfer,D.J. (1989). The Pittsburgh Sleep Quality Index (PSQI): A new instrument for psychiatric research and practice. Psychiatry Research, 28(2), 193-213."""@en ;
	rdf:type dcterms:source ;
	fabio:hasPubMedId mhdb:2748771 .

mhdb:Gross_JJ__John_OP_2003_Individual_differences_in_two_emotion_regulation_processes_Implications_for_affect_relationships_and_well-being_Journal_of_Personality_and_Social_Psychology_85_348-362 rdfs:label """Gross, J.J., & John, O.P. (2003). Individual differences in two emotion regulation processes: Implications for affect, relationships, and well-being. Journal of Personality and Social Psychology, 85, 348-362."""@en ;
	rdf:type dcterms:source ;
	fabio:hasPubMedId mhdb:12916575 .

mhdb:Meyer_TJ_Miller_ML_Metzger_RL_Borkovec_TD_1990_Development_and_validation_of_the_Penn_State_Worry_Questionnaire_Beh_Research_and_Therapy_28_487-495 rdfs:label """Meyer TJ, Miller ML, Metzger RL, Borkovec TD (1990). Development and validation of the Penn State Worry Questionnaire. Beh Research and Therapy, 28, 487-495."""@en ;
	rdf:type dcterms:source ;
	fabio:hasPubMedId mhdb:2076086 .

mhdb:Treynor_W_Gonzalez_R_Nolen-Hoeksema_S_2003_Rumination_Reconsidered_A_Psychometric_Analysis_Cognitive_Therapy_and_Research_273_247-259 rdfs:label """Treynor, W.; Gonzalez, R.; Nolen-Hoeksema, S. (2003). Rumination Reconsidered: A Psychometric Analysis. Cognitive Therapy and Research, 27(3), 247-259"""@en ;
	rdf:type dcterms:source .

mhdb:Huba_G_J_Aneshensel_C_S_Singer_J_L_1981_Development_of_scales_for_three_second-order_factors_of_inner_experience_Multivariate_Behav_Res_16_181206 rdfs:label """Huba G. J., Aneshensel C. S., Singer J. L. (1981). Development of scales for three second-order factors of inner experience. Multivariate Behav. Res. 16 181–206"""@en ;
	rdf:type dcterms:source ;
	fabio:hasPubMedId mhdb:26825422 .

mhdb:Hollingshead_A_A_1975_Four-factor_index_of_social_status_Unpublished_manuscript_Yale_University_New_Haven_CT rdfs:label """Hollingshead, A. A. (1975). Four-factor index of social status. Unpublished manuscript, Yale University, New Haven, CT."""@en ;
	rdf:type dcterms:source .

mhdb:Suggested_by_Dr_Theo_Sandfort_Adapted_from_Sex_Role_Identity_Scale_Journal_of_Personality_and_Social_Psychology_1979_Vol_37_No_10_1779-1789 rdfs:label """Suggested by Dr. Theo Sandfort. Adapted from: Sex Role Identity Scale. Journal of Personality and Social Psychology. 1979, Vol. 37, No. 10, 1779-1789."""@en ;
	rdf:type dcterms:source .

mhdb:Reynolds_C_R__Kamphaus_R_W_1992_BASC_Behavior_assessment_system_for_children_Manual_American_Guidance_Service_Incorporated rdfs:label """Reynolds, C. R., & Kamphaus, R. W. (1992). BASC: Behavior assessment system for children: Manual. American Guidance Service, Incorporated."""@en ;
	rdf:type dcterms:source .

mhdb:Ehring_T_Zetsche_U_Weidacker_K_Wahl_K_Schonfeld_S__Ehlers_A_2011_The_Perseverative_Thinking_Questionnaire_PTQ_Validation_of_a_content-independent_measure_of_repetitive_negative_thinking_Journal_of_Behavior_Therapy_and_Experimental_Psychiatry_42_225-232 rdfs:label """Ehring, T., Zetsche, U., Weidacker, K., Wahl, K., Schonfeld, S., & Ehlers, A. (2011). The Perseverative Thinking Questionnaire (PTQ): Validation of a content-independent measure of repetitive negative thinking. Journal of Behavior Therapy and Experimental Psychiatry, 42, 225-232."""@en ;
	rdf:type dcterms:source ;
	fabio:hasPubMedId mhdb:21315886 .

mhdb:Larsen_RJ_Diener_E_Emmons_RA_1986_Affect_intensity_and_reactions_to_daily_life_events_Journal_of_Personality_and_Social_Psychology_51_803814 rdfs:label """Larsen RJ.; Diener E.; Emmons RA. (1986) Affect intensity and reactions to daily life events. Journal of Personality and Social Psychology, 51, 803–814."""@en ;
	rdf:type dcterms:source ;
	fabio:hasPubMedId mhdb:16673624 .

mhdb:Methodology_of_the_Youth_Risk_Behavior_Surveillance_System_MMWR_200453RR-12113 rdfs:label """Methodology of the Youth Risk Behavior Surveillance System. MMWR 2004;53(RR-12):1–13."""@en ;
	rdf:type dcterms:source .

mhdb:Whiteside_S_P_and_D_R_Lynam_2001_The_Five_Factor_Model_and_impulsivity_using_a_structural_model_of_personality_to_understand_impulsivity_Personality_and_Individual_Differences_304_669-689 rdfs:label """Whiteside, S. P. and D. R. Lynam (2001). The Five Factor Model and impulsivity: using a structural model of personality to understand impulsivity. Personality and Individual Differences, 30(4): 669-689."""@en ;
	rdf:type dcterms:source .

mhdb:Whiteside_SP_Lynam_DR_Miller_JD_Reynolds_SK_2005_Validation_of_the_UPPS_impulsive_behaviour_scale_a_four-factor_model_of_impulsivity_European_Journal_of_Personality_19559-574 rdfs:label """Whiteside SP, Lynam DR, Miller JD, Reynolds SK. (2005). Validation of the UPPS impulsive behaviour scale: a four-factor model of impulsivity. European Journal of Personality. 19:559-574."""@en ;
	rdf:type dcterms:source .

mhdb:Pynoos_Rodriguez_Steinberg_Stuber__FrederickC_1998_UCLA_PTSD_Index_for_DSM-IV_Unpublished_Manual rdfs:label """Pynoos, Rodriguez, Steinberg, Stuber, & Frederick,C. (1998). UCLA PTSD Index for DSM-IV. Unpublished Manual."""@en ;
	rdf:type dcterms:source .

mhdb:Briere_J_1996_Trauma_Symptom_Checklist_for_Children_TSCC_Professional_Manual_Odessa_FL_Psychological_Assessment_Resources rdfs:label """Briere, J. (1996). Trauma Symptom Checklist for Children (TSCC) Professional Manual. Odessa, FL: Psychological Assessment Resources."""@en ;
	rdf:type dcterms:source .

mhdb:Adapted_from_Holtzman_et_al_2004_Social_Network_Characteristics_and_Cognition_in_Middle-Aged_and_Older_Adults_JOG_Psych_Sci_596_278-284 rdfs:label """Adapted from: Holtzman, et al., (2004). Social Network Characteristics and Cognition in Middle-Aged and Older Adults, JOG, Psych Sci. 59(6), 278-284"""@en ;
	rdf:type dcterms:source ;
	fabio:hasPubMedId mhdb:15576855 .

mhdb:Mccrae_R_R__Costa_P_T_February_2004_A_contemplated_revision_of_the_NEO_Five-Factor_Inventory_Personality_and_Individual_Differences_363_587596 rdfs:label """Mccrae, R. R., & Costa, P. T. (February 2004). “A contemplated revision of the NEO Five-Factor Inventory”. Personality and Individual Differences 36(3), 587–596."""@en ;
	rdf:type dcterms:source .

mhdb:Craig_CL_et_al_2003_International_Physical_activity_questionnaire_12-country_reliability_and_validity_Medicine_and_Science_in_Sports__Exercise_358_1381-1395 rdfs:label """Craig, C.L., et al. (2003). International Physical activity questionnaire: 12-country reliability and validity. Medicine and Science in Sports & Exercise, 35(8), 1381-1395."""@en ;
	rdf:type dcterms:source ;
	fabio:hasPubMedId mhdb:12900694 .

mhdb:Blais_AR__Weber_EU_2006_A_Domain-Specific_Risk-Taking_DOSPERT_scale_for_adult_populations_Judgment_and_Decision_Making_1_33-47 rdfs:label """Blais, A.R., & Weber, E.U. (2006) A Domain-Specific Risk-Taking (DOSPERT) scale for adult populations. Judgment and Decision Making, 1, 33-47."""@en ;
	rdf:type dcterms:source .

mhdb:Broadbent_D_E_Cooper_P_F_FitzGerald_P__Parkes_K_R_1982_The_cognitive_failures_questionnaire_CFQ_and_its_correlates_British_Journal_of_Clinical_Psychology_211_1-16 rdfs:label """Broadbent, D. E., Cooper, P. F., FitzGerald, P., & Parkes, K. R. (1982). The cognitive failures questionnaire (CFQ) and its correlates. British Journal of Clinical Psychology, 21(1), 1-16."""@en ;
	rdf:type dcterms:source ;
	fabio:hasPubMedId mhdb:7126941 .

mhdb:Rast_P_Zimprich_D_Van_Boxtel_M__Jolles_J_2009_Factor_structure_and_measurement_invariance_of_the_cognitive_failures_questionnaire_across_the_adult_life_span_Assessment_162_145-58 rdfs:label """Rast, P., Zimprich, D., Van Boxtel, M., & Jolles, J. (2009). Factor structure and measurement invariance of the cognitive failures questionnaire across the adult life span. Assessment, 16(2), 145-58."""@en ;
	rdf:type dcterms:source ;
	fabio:hasPubMedId mhdb:19066391 .

mhdb:Stunkard_A_J__Messick_S_1985_The_three-factor_eating_questionnaire_to_measure_dietary_restraint_disinhibition_and_hunger_Journal_of_Psychosomatic_Research_29_7183 rdfs:label """Stunkard, A. J. & Messick, S. (1985). The three-factor eating questionnaire to measure dietary restraint, disinhibition, and hunger. Journal of Psychosomatic Research, 29: 71–83."""@en ;
	rdf:type dcterms:source ;
	fabio:hasPubMedId mhdb:3981480 .

mhdb:Evans_DE__Rothbart_MK_2007_Development_of_a_model_for_adult_temperament_Journal_of_Research_in_Personality_41_868-888 rdfs:label """Evans, D.E., & Rothbart, M.K. (2007). Development of a model for adult temperament. Journal of Research in Personality, 41, 868-888."""@en ;
	rdf:type dcterms:source .

mhdb:Ellis_L_K__Rothbart_M_K_2001_April_Revision_of_the_Early_Adolescent_Temperament_Questionnaire_Poster_presented_at_the_biennial_meeting_of_the_Society_for_Research_in_Child_Development_Minneapolis_MN rdfs:label """Ellis, L. K., & Rothbart, M. K. (2001, April). Revision of the Early Adolescent Temperament Questionnaire. Poster presented at the biennial meeting of the Society for Research in Child Development, Minneapolis, MN."""@en ;
	rdf:type dcterms:source .

mhdb:Capaldi_D_M__Rothbart_M_K_1992_Development_and_validation_of_an_early_adolescent_temperament_measure_Journal_of_Early_Adolescence_122_153-173 rdfs:label """Capaldi, D. M., & Rothbart, M. K. (1992). Development and validation of an early adolescent temperament measure. Journal of Early Adolescence, 12(2), 153-173."""@en ;
	rdf:type dcterms:source .

mhdb:Ellis_L_K_2002_Individual_differences_and_adolescent_psychological_development_Unpublished_doctoral_dissertation_University_of_Oregon rdfs:label """Ellis, L. K. (2002). Individual differences and adolescent psychological development. Unpublished doctoral dissertation, University of Oregon."""@en ;
	rdf:type dcterms:source .

mhdb:Elliot_D_M__Briere_J_1992_Sexual_abuse_trauma_among_professional_women_Validating_the_Trauma_Symptom_Checklist__40_TSC-40_Child_Abuse__Neglect_16_391-398 rdfs:label """Elliot, D. M. & Briere, J. (1992). Sexual abuse trauma among professional women: Validating the Trauma Symptom Checklist – 40 (TSC-40). Child Abuse & Neglect, 16, 391-398."""@en ;
	rdf:type dcterms:source ;
	fabio:hasPubMedId mhdb:1617473 .

mhdb:Briere_J_N__Runtz_M_G_1989_The_Trauma_Symptom_Checklist_TSC-33_early_data_on_a_new_scale_Journal_of_Interpersonal_Violence_4_151-163 rdfs:label """Briere, J. N., & Runtz, M. G. (1989). The Trauma Symptom Checklist (TSC-33): early data on a new scale. Journal of Interpersonal Violence, 4, 151-163."""@en ;
	rdf:type dcterms:source .

<http://shura.shu.ac.uk/7164/> rdfs:label """A treatise on language methods and language-games in autism"""@en ;
	rdf:type dcterms:source ;
	schema:WebSite <http://shura.shu.ac.uk/7164/> ;
	mhdb:hasReferenceType bibo:Thesis ;
	mhdb:isAboutDomain mhdb:communication .

mhdb:Using_concurrent_operants_to_evaluate_perseverate_conversations_in_children_and_adults_with_aspergers rdfs:label """Using concurrent operants to evaluate perseverate conversations in children and adults with aspergers"""@en ;
	rdf:type dcterms:source ;
	mhdb:hasReferenceType bibo:Thesis ;
	mhdb:isAboutDomain mhdb:communication ;
	dcterms:isReferencedBy mhdb:httpsiruiowaeducgiviewcontentcgiarticle1600contextetd .

mhdb:The_Proloquo2go_App_in_reducing_echolalia_in_autism rdfs:label """The Proloquo2go App in reducing echolalia in autism"""@en ;
	rdf:type dcterms:source ;
	mhdb:hasReferenceType bibo:Thesis ;
	mhdb:isAboutDomain mhdb:communication ;
	dcterms:isReferencedBy mhdb:httpsfilesericedgovfulltextED577783pdf .

mhdb:httpslinkspringercomchapter101007978-3-319-09767-1_3 rdfs:label """<https://link.springer.com/chapter/10.1007/978-3-319-09767-1_3>"""@en ;
	rdf:type dcterms:source ;
	mhdb:hasReferenceType mhdb:research_paper .

mhdb:httpsresearchvunlenpublicationsreliability-and-validity-of-the-interactive-drawing-test-a-measur rdfs:label """<https://research.vu.nl/en/publications/reliability-and-validity-of-the-interactive-drawing-test-a-measur>"""@en ;
	rdf:type dcterms:source ;
	mhdb:hasReferenceType mhdb:research_paper .

mhdb:httpswwwncbinlmnihgovpubmed29939367 rdfs:label """<https://www.ncbi.nlm.nih.gov/pubmed/29939367>"""@en ;
	rdf:type dcterms:source ;
	fabio:hasPubMedId mhdb:29939367 .

mhdb:httpswwwncbinlmnihgovpmcarticlesPMC5726304 rdfs:label """<https://www.ncbi.nlm.nih.gov/pmc/articles/PMC5726304/>"""@en ;
	rdf:type dcterms:source ;
	fabio:hasPubMedId mhdb:29188853 .

mhdb:nosology_manual rdfs:label """\'\'\'nosology manual\'\'\'@en"""@en ;
	rdf:type mhdb:ReferenceType ;
	rdfs:subClassOf mhdb:manual .

disco:Questionnaire rdfs:label """\'\'\'disco:Questionnaire\'\'\'@en"""@en ;
	rdf:type mhdb:ReferenceType ;
	rdfs:subClassOf schema:CreativeWork .

mhdb:questionnaire_manual rdfs:label """\'\'\'questionnaire manual\'\'\'@en"""@en ;
	rdf:type mhdb:ReferenceType ;
	rdfs:subClassOf mhdb:manual .

schema:WebSite rdfs:label """\'\'\'schema:WebSite\'\'\'@en"""@en ;
	rdf:type mhdb:ReferenceType .

schema:Person rdfs:label """\'\'\'schema:Person\'\'\'@en"""@en ;
	rdf:type mhdb:ReferenceType .

mhdb:manual rdfs:label """\'\'\'manual\'\'\'@en"""@en ;
	rdf:type mhdb:ReferenceType ;
	rdfs:subClassOf schema:CreativeWork .

mhdb:research_paper rdfs:label """\'\'\'research paper\'\'\'@en"""@en ;
	rdf:type mhdb:ReferenceType .

bibo:Thesis rdfs:label """\'\'\'bibo:Thesis\'\'\'@en"""@en ;
	rdf:type mhdb:ReferenceType .
